@prefix : <https://raw.githubusercontent.com/AbsVahter/trpgontologies/main/gumshoe/cthulhu_confidential/PELGOC01.ttl#> .
@prefix owl: <http://www.w3.org/2002/07/owl#> .
@prefix rdf: <http://www.w3.org/1999/02/22-rdf-syntax-ns#> .
@prefix xml: <http://www.w3.org/XML/1998/namespace> .
@prefix xsd: <http://www.w3.org/2001/XMLSchema#> .
@prefix rdfs: <http://www.w3.org/2000/01/rdf-schema#> .
@prefix sche: <http://schema.org/> .
@prefix bbo: <https://raw.githubusercontent.com/AbsVahter/trpgontologies/main/_basic/BasicBookOnto.ttl#> .
@prefix pzo2101: <https://raw.githubusercontent.com/AbsVahter/trpgontologies/main/pathfinder/2ed/pzo2101.owl#> .
@base <https://raw.githubusercontent.com/AbsVahter/trpgontologies/main/gumshoe/cthulhu_confidential/PELGOC01.ttl#> .

<https://raw.githubusercontent.com/AbsVahter/trpgontologies/main/gumshoe/cthulhu_confidential/PELGOC01.ttl#> rdf:type owl:Ontology ;
                                                                                                             owl:imports bbo: .

#################################################################
#    Annotation properties
#################################################################

###  http://schema.org/image
sche:image rdf:type owl:AnnotationProperty .


#################################################################
#    Object Properties
#################################################################

###  https://raw.githubusercontent.com/AbsVahter/trpgontologies/main/gumshoe/cthulhu_confidential/PELGOC01.ttl#advance
:advance rdf:type owl:ObjectProperty ;
         rdfs:domain :Challenge ;
         rdfs:range :Gamerule ;
         rdfs:comment "Succeeding especially well. This might grant you an Edge card, or allow you extra leverage in the situation at hand." ;
         rdfs:label "Advance outcome" ;
         rdfs:seeAlso pzo2101:checkCriticalSuccess .


###  https://raw.githubusercontent.com/AbsVahter/trpgontologies/main/gumshoe/cthulhu_confidential/PELGOC01.ttl#hold
:hold rdf:type owl:ObjectProperty ;
      rdfs:domain :Challenge ;
      rdfs:range :Gamerule ;
      rdfs:comment "generally leaves you no worse off than you were before, or allows you to move forward, though without additional benefit" ;
      rdfs:label "Hold outcome" ;
      rdfs:seeAlso pzo2101:checkFailure ,
                   pzo2101:checkSuccess .


###  https://raw.githubusercontent.com/AbsVahter/trpgontologies/main/gumshoe/cthulhu_confidential/PELGOC01.ttl#setback
:setback rdf:type owl:ObjectProperty ;
         rdfs:domain :Challenge ;
         rdfs:range :Gamerule ;
         rdfs:comment "Worsening your situation. It may saddle you with a Problem card. Or it might simply make your immediate dilemma worse in some way." ;
         rdfs:label "Setback outcome" ;
         rdfs:seeAlso pzo2101:checkCriticalFailure .


###  https://raw.githubusercontent.com/AbsVahter/trpgontologies/main/gumshoe/cthulhu_confidential/PELGOC01.ttl#uses
:uses rdf:type owl:ObjectProperty ;
      rdfs:domain :Gamerule ;
      rdfs:range owl:Thing ;
      rdfs:label "uses" ;
      rdfs:seeAlso pzo2101:uses .


#################################################################
#    Data properties
#################################################################

###  https://raw.githubusercontent.com/AbsVahter/trpgontologies/main/gumshoe/cthulhu_confidential/PELGOC01.ttl#application
:application rdf:type owl:DatatypeProperty ;
             rdfs:domain owl:Thing ;
             rdfs:range xsd:string ;
             rdfs:label "example of using" .


###  https://raw.githubusercontent.com/AbsVahter/trpgontologies/main/gumshoe/cthulhu_confidential/PELGOC01.ttl#calculations
:calculations rdf:type owl:DatatypeProperty ;
              rdfs:domain :Gamerule ;
              rdfs:range xsd:string ;
              rdfs:label "calculations" ;
              rdfs:seeAlso pzo2101:calculations .


#################################################################
#    Classes
#################################################################

###  https://raw.githubusercontent.com/AbsVahter/trpgontologies/main/gumshoe/cthulhu_confidential/PELGOC01.ttl#AcademicAbility
:AcademicAbility rdf:type owl:Class ;
                 rdfs:subClassOf :InvestigativeAbility ;
                 rdfs:label "Academic ability" .


###  https://raw.githubusercontent.com/AbsVahter/trpgontologies/main/gumshoe/cthulhu_confidential/PELGOC01.ttl#Art


###  https://raw.githubusercontent.com/AbsVahter/trpgontologies/main/gumshoe/cthulhu_confidential/PELGOC01.ttl#Challenge
:Challenge rdf:type owl:Class ;
           rdfs:subClassOf :Test ;
           rdfs:comment "Challenges occur in situations where degrees of success or failure can send the story into different possible branches, each of them interesting in its own way." ,
                        "Sometimes you know that you’ll get what you want, but you are only determining the costs of success" ,
                        "examples: fixing the car before the yokel with the rifle gets back, running away from a creature that surges out of the La Brea tar pits, sneaking backstage at the nightclub" ;
           rdfs:label "Challenge" ;
           rdfs:seeAlso pzo2101:SkillCheck .


###  https://raw.githubusercontent.com/AbsVahter/trpgontologies/main/gumshoe/cthulhu_confidential/PELGOC01.ttl#Characteristic
:Characteristic rdf:type owl:Class ;
                rdfs:label "Characteristic" ;
                rdfs:seeAlso pzo2101:Characteristic .


###  https://raw.githubusercontent.com/AbsVahter/trpgontologies/main/gumshoe/cthulhu_confidential/PELGOC01.ttl#DieRoll
:DieRoll rdf:type owl:Class ;
         rdfs:subClassOf :Gamerule ,
                         [ rdf:type owl:Restriction ;
                           owl:onProperty :calculations ;
                           owl:hasValue "die roll = (count of ability dices)d6"
                         ] ;
         rdfs:seeAlso pzo2101:SkillRoll .


###  https://raw.githubusercontent.com/AbsVahter/trpgontologies/main/gumshoe/cthulhu_confidential/PELGOC01.ttl#Gamerule
:Gamerule rdf:type owl:Class ;
          rdfs:label "Gamerule" ;
          rdfs:seeAlso pzo2101:Gamerule .


###  https://raw.githubusercontent.com/AbsVahter/trpgontologies/main/gumshoe/cthulhu_confidential/PELGOC01.ttl#GeneralAbility
:GeneralAbility rdf:type owl:Class ;
                rdfs:subClassOf :Characteristic ;
                rdfs:comment "When attempting actions that don’t directly gather information, and which can lead to engaging story possibilities whether you succeed or fail, use your General Abilities." ,
                             "{ability: number of dice}" ;
                rdfs:label "General ability" ;
                rdfs:seeAlso pzo2101:Skill .


###  https://raw.githubusercontent.com/AbsVahter/trpgontologies/main/gumshoe/cthulhu_confidential/PELGOC01.ttl#InterpersonalAbility
:InterpersonalAbility rdf:type owl:Class ;
                      rdfs:subClassOf :InvestigativeAbility ;
                      rdfs:label "Interpersonal ability" .


###  https://raw.githubusercontent.com/AbsVahter/trpgontologies/main/gumshoe/cthulhu_confidential/PELGOC01.ttl#InvestigativeAbility
:InvestigativeAbility rdf:type owl:Class ;
                      rdfs:subClassOf :Characteristic ;
                      rdfs:comment "Ability for gathering information" ;
                      rdfs:label "Investigative ability" .


###  https://raw.githubusercontent.com/AbsVahter/trpgontologies/main/gumshoe/cthulhu_confidential/PELGOC01.ttl#ManualAbility
:ManualAbility rdf:type owl:Class ;
               rdfs:subClassOf :GeneralAbility ;
               rdfs:comment "drawing on a combination of skill training and fine motor skills" ;
               rdfs:label "Manual ability" .


###  https://raw.githubusercontent.com/AbsVahter/trpgontologies/main/gumshoe/cthulhu_confidential/PELGOC01.ttl#MentalAbility
:MentalAbility rdf:type owl:Class ;
               rdfs:subClassOf :GeneralAbility ;
               rdfs:comment "drawing on mostly on intellectual study, perception, thought, and/or memory" ;
               rdfs:label "Mental ability" .


###  https://raw.githubusercontent.com/AbsVahter/trpgontologies/main/gumshoe/cthulhu_confidential/PELGOC01.ttl#PhysicalAbility
:PhysicalAbility rdf:type owl:Class ;
                 rdfs:subClassOf :GeneralAbility ;
                 rdfs:comment "using your gross motor skills" ;
                 rdfs:label "Physical ability" .


###  https://raw.githubusercontent.com/AbsVahter/trpgontologies/main/gumshoe/cthulhu_confidential/PELGOC01.ttl#TechnicalAbility
:TechnicalAbility rdf:type owl:Class ;
                  rdfs:subClassOf :InvestigativeAbility ;
                  rdfs:label "Technical ability" .


###  https://raw.githubusercontent.com/AbsVahter/trpgontologies/main/gumshoe/cthulhu_confidential/PELGOC01.ttl#Test
:Test rdf:type owl:Class ;
      rdfs:subClassOf :Gamerule ;
      rdfs:comment "A test determines what happens when your Investigator tries to do something that might not work." ;
      rdfs:label "Test" .


#################################################################
#    Individuals
#################################################################

###  https://raw.githubusercontent.com/AbsVahter/trpgontologies/main/gumshoe/cthulhu_confidential/PELGOC01.ttl#accounting
:accounting rdf:type owl:NamedIndividual ,
                     :AcademicAbility ;
            :application "reconstruct financial histories from old records (uncovering, say, slave-trading or smuggling)" ,
                         "reel off the latest rumors from the world of business, finance and industry" ,
                         "spot the telltale signs of embezzlement, bribes, blackmail, or dummy companies" ,
                         "tell legitimate businesses from criminal enterprises" ,
                         "track payments to their source" ;
            rdfs:comment "You understand bookkeeping and accountancy procedures; you can read and keep financial records." ;
            rdfs:label "Accounting ability" .


###  https://raw.githubusercontent.com/AbsVahter/trpgontologies/main/gumshoe/cthulhu_confidential/PELGOC01.ttl#anthropology
:anthropology rdf:type owl:NamedIndividual ,
                       :AcademicAbility ;
              :application "describe and predict the customs of a foreign group or local subculture" ,
                           "extrapolate the practices of an unknown culture from similar examples" ,
                           "identify artifacts and rituals of living cultures" ;
              rdfs:comment "You are an expert in the study of human cultures, from the Stone Age to the Jazz Age" ;
              rdfs:label "Anthropology ability" .


###  https://raw.githubusercontent.com/AbsVahter/trpgontologies/main/gumshoe/cthulhu_confidential/PELGOC01.ttl#archaeology
:archaeology rdf:type owl:NamedIndividual ,
                      :AcademicAbility ;
             :application "describe the customs of ancient or historical cultures" ,
                          "distinguish real artifacts from fakes" ,
                          "identify artifacts by culture and usage" ,
                          "navigate inside ruins and catacombs, including finding secret doors and hidden construction" ,
                          "spot well-disguised graves and underground hiding places" ,
                          "tell how long something has been buried and date its construction" ;
             rdfs:comment "You excavate and study the structures and artifacts of historical cultures and civilizations." ;
             rdfs:label "Archaeology ability" .


###  https://raw.githubusercontent.com/AbsVahter/trpgontologies/main/gumshoe/cthulhu_confidential/PELGOC01.ttl#architecture
:architecture rdf:type owl:NamedIndividual ,
                       :AcademicAbility ;
              :application "construct stable makeshift structures" ,
                           "deduce the existence of hidden rooms, priest-holes, hyper-geometric witch-garrets, and other anomalies" ,
                           "guess what lies around the corner while exploring an unknown structure" ,
                           "identify a building’s age, architectural style, original use, and history of modifications" ,
                           "identify elements vital to a building’s structural integrity" ,
                           "judge the relative strength of building materials" ,
                           "name the architectural firm responsible for any well-known building in your area, recounting any peculiarities involved in its construction" ;
              rdfs:comment "You know how buildings are designed and constructed." ;
              rdfs:label "Architecture ability" .


###  https://raw.githubusercontent.com/AbsVahter/trpgontologies/main/gumshoe/cthulhu_confidential/PELGOC01.ttl#art_history
:art_history rdf:type owl:NamedIndividual ,
                      :AcademicAbility ;
             :application "accurately estimate the price of an objet d’art" ,
                          "call to mind historical details on artists and those around them" ,
                          "distinguish real works from fakes" ,
                          "identify the age of an object by style and materials" ,
                          "list the most recent films set in a given stylistic period and comment on their relative accuracy" ,
                          "tell when something has been retouched or altered" ;
             rdfs:comment "You’re an expert on works of art (including the practical arts such as furniture and pottery) from an aesthetic and technical point of view." ;
             rdfs:label "Art history ability" .


###  https://raw.githubusercontent.com/AbsVahter/trpgontologies/main/gumshoe/cthulhu_confidential/PELGOC01.ttl#assess_honesty
:assess_honesty rdf:type owl:NamedIndividual ,
                         :InterpersonalAbility ;
                :application "tell when someone’s trying to play you for a sap" ,
                             "to cold-read a mark for fortune-telling scams, phony séances or mentalist acts, and the like" ;
                rdfs:comment "You can tell when someone’s trying to play you for a sap. Not only does your gut tell you when a witness is lying, life’s hard knocks have taught you to instinctively judge and sense motives and character." ;
                rdfs:label "Assess honesty ability" .


###  https://raw.githubusercontent.com/AbsVahter/trpgontologies/main/gumshoe/cthulhu_confidential/PELGOC01.ttl#astronomy
:astronomy rdf:type owl:NamedIndividual ,
                    :TechnicalAbility ;
           :application "decipher astrological texts" ,
                        "plot the movement of stars and planets, and know which ones are overhead at any given time" ,
                        "predict eclipses, comets, meteor showers, and other regular astronomical phenomena" ,
                        "use a telescope, including large reflectors" ;
           rdfs:comment "You study celestial objects, including the stars and planets." ;
           rdfs:label "Astronomy ability" .


###  https://raw.githubusercontent.com/AbsVahter/trpgontologies/main/gumshoe/cthulhu_confidential/PELGOC01.ttl#athletics
:athletics rdf:type owl:NamedIndividual ,
                    :PhysicalAbility ;
           :application "perform general acts of physical derring-do, from running to jumping to throwing bundles of dynamite to dodging oncoming objects" ,
                        "resist the direct harm of magic" ,
                        "resist the effects of disease, poisoning, and intoxicants" ,
                        "resist the effects of exposure, such as hypothermia, frostbite, and sunstroke" ;
           rdfs:label "Athletics ability" .


###  https://raw.githubusercontent.com/AbsVahter/trpgontologies/main/gumshoe/cthulhu_confidential/PELGOC01.ttl#athletics_challenge
:athletics_challenge rdf:type owl:NamedIndividual ,
                              :Challenge ;
                     :uses :athletics_die_roll ;
                     rdfs:label "Athletics challenge" .


###  https://raw.githubusercontent.com/AbsVahter/trpgontologies/main/gumshoe/cthulhu_confidential/PELGOC01.ttl#athletics_die_roll
:athletics_die_roll rdf:type owl:NamedIndividual ,
                             :DieRoll ;
                    :uses :athletics ;
                    rdfs:label "Athletics die roll" .


###  https://raw.githubusercontent.com/AbsVahter/trpgontologies/main/gumshoe/cthulhu_confidential/PELGOC01.ttl#bargain
:bargain rdf:type owl:NamedIndividual ,
                  :InterpersonalAbility ;
         :application "exchange cash for information" ,
                      "gauge likely prices of items, including what someone else will pay for them" ,
                      "haggle for goods and services" ,
                      "mediate hostage situations or diplomatic crises" ,
                      "swap favors or information with others" ;
         rdfs:comment "Spends allow you to gain an advantage other than information in exchange for money or other considerations." ,
                      "You are an expert in making deals with others, convincing them that the best arrangement for you is also the best for them." ;
         rdfs:label "Bargain ability" .


###  https://raw.githubusercontent.com/AbsVahter/trpgontologies/main/gumshoe/cthulhu_confidential/PELGOC01.ttl#biology
:biology rdf:type owl:NamedIndividual ,
                  :AcademicAbility ;
         :application "analyze unknown ichor, scales, or slime identify a plant from a small sample" ,
                      "identify an animal from samples of its hair, blood, bones, or other tissue" ,
                      "isolate or detect natural poisons or venoms" ,
                      "tell when an animal is behaving strangely" ,
                      "tell whether an animal or plant is natural to a given area" ;
         rdfs:comment "You study the evolution, behavior, and physical makeup of living organisms." ;
         rdfs:label "Biology ability" .


###  https://raw.githubusercontent.com/AbsVahter/trpgontologies/main/gumshoe/cthulhu_confidential/PELGOC01.ttl#bureaucracy
:bureaucracy rdf:type owl:NamedIndividual ,
                      :InterpersonalAbility ;
             :application "borrow equipment or supplies" ,
                          "convince officials to provide sensitive information" ,
                          "develop and maintain contacts within a bureaucracy with which you have regular dealings" ,
                          "find the person who really knows what’s going on" ,
                          "gain credentials on false pretenses" ,
                          "know which government officials are honest and which are corrupt" ,
                          "locate offices and files" ;
             rdfs:comment "You expertly navigate bureaucratic organization, from government offices to large private firms." ;
             rdfs:label "Bureaucracy ability" .


###  https://raw.githubusercontent.com/AbsVahter/trpgontologies/main/gumshoe/cthulhu_confidential/PELGOC01.ttl#chemistry
:chemistry rdf:type owl:NamedIndividual ,
                    :TechnicalAbility ;
           :application "analyze unknown substances, alloys, compounds, etc." ,
                        "create simple explosives, poisons, gases, and acids" ,
                        "identify drugs, pharmaceuticals, toxins, and viruses, among a wide variety of other materials" ,
                        "match samples of dirt or vegetation from a piece of evidence to a scene" ,
                        "perform ballistics and gunpowder analysis of bullets or other evidence" ,
                        "perform chemical document analysis on ink or paper" ;
           rdfs:comment "You’re trained in the analysis of chemical substances." ;
           rdfs:label "Chemistry ability" .


###  https://raw.githubusercontent.com/AbsVahter/trpgontologies/main/gumshoe/cthulhu_confidential/PELGOC01.ttl#conceal
:conceal rdf:type owl:NamedIndividual ,
                  :ManualAbility ;
         :application "altering an object’s visual signature with paint or plaster" ,
                      "building secret compartments" ,
                      "camouflage" ,
                      "holding items out on your person" ,
                      "sneaking things into drawers unobserved" ;
         rdfs:comment "You can hide things from view and conceal them from searchers" ;
         rdfs:label "Conceal ability" .


###  https://raw.githubusercontent.com/AbsVahter/trpgontologies/main/gumshoe/cthulhu_confidential/PELGOC01.ttl#conceal_challenge
:conceal_challenge rdf:type owl:NamedIndividual ,
                            :Challenge ;
                   :uses :conceal_die_roll ;
                   rdfs:label "Conceal challenge" .


###  https://raw.githubusercontent.com/AbsVahter/trpgontologies/main/gumshoe/cthulhu_confidential/PELGOC01.ttl#conceal_die_roll
:conceal_die_roll rdf:type owl:NamedIndividual ,
                           :DieRoll ;
                  :uses :conceal ;
                  rdfs:label "Conceal die roll" .


###  https://raw.githubusercontent.com/AbsVahter/trpgontologies/main/gumshoe/cthulhu_confidential/PELGOC01.ttl#cool
:cool rdf:type owl:NamedIndividual ,
               :MentalAbility ;
      :application "avoid attempting a futile grand gesture to wring real justice from a rigged system" ,
                   "avoid falling for the wrong kind of dame" ,
                   "avoid hitting the roulette wheel when you know you shouldn’t" ,
                   "avoid showing a tell that warns the killer that you know he did it" ,
                   "avoid smart-mouthing the cop who’s itching to club you" ,
                   "resist supernatural forces attempting to influence your behavior" ;
      rdfs:comment "Measures your ability to make the smart play, instead of the impulsive one, in response to emotional temptation." ;
      rdfs:label "Cool ability" .


###  https://raw.githubusercontent.com/AbsVahter/trpgontologies/main/gumshoe/cthulhu_confidential/PELGOC01.ttl#cool_challenge
:cool_challenge rdf:type owl:NamedIndividual ,
                         :Challenge ;
                :uses :cool_die_roll ;
                rdfs:label "Cool challenge" .


###  https://raw.githubusercontent.com/AbsVahter/trpgontologies/main/gumshoe/cthulhu_confidential/PELGOC01.ttl#cool_die_roll
:cool_die_roll rdf:type owl:NamedIndividual ,
                        :DieRoll ;
               :uses :cool ;
               rdfs:label "Cool die roll" .


###  https://raw.githubusercontent.com/AbsVahter/trpgontologies/main/gumshoe/cthulhu_confidential/PELGOC01.ttl#cop_talk
:cop_talk rdf:type owl:NamedIndividual ,
                   :InterpersonalAbility ;
          :application "call in favors from law enforcement contacts — often the one cop on the force who genuinely likes and trusts you" ,
                       "get excused for minor infractions" ,
                       "prompt them to spill confidential information" ,
                       "read between the lines when a cop can’t come out and tell you the whole truth" ;
          rdfs:comment "Despite the low regard in which cops hold private detectives, you know their lingo and needs well enough to extract information from them." ;
          rdfs:label "Cop talk ability" .


###  https://raw.githubusercontent.com/AbsVahter/trpgontologies/main/gumshoe/cthulhu_confidential/PELGOC01.ttl#cover_art
:cover_art rdf:type owl:NamedIndividual ,
                    bbo:Art ;
           sche:image "https://cf.geekdo-images.com/px_RKnwymHK5mlXm2HHLfQ__imagepage/img/r_KLEj1V01cBVnu7-HtcF7Laaj0=/fit-in/900x600/filters:no_upscale():strip_icc()/pic3375012.jpg" ;
           rdfs:label "Cover art" .


###  https://raw.githubusercontent.com/AbsVahter/trpgontologies/main/gumshoe/cthulhu_confidential/PELGOC01.ttl#craft
:craft rdf:type owl:NamedIndividual ,
                :TechnicalAbility ;
       :application "discover a secret drawer in a wooden desk" ,
                    "identify its famous maker, if applicable" ,
                    "in the case of gems and precious metals, tell whether the materials are genuine" ,
                    "know what kind of wood, stone, porcelain and so on an item is made of" ,
                    "say whether an item was skillfully or crudely fashioned" ,
                    "sort fakes from authentic items" ,
                    "tell roughly how old a craft object is" ;
       rdfs:comment "You can create useful physical objects, working with materials like wood, metal, precious stones, leather, and so forth. This allows you a general background knowledge in handmade items of all kinds." ;
       rdfs:label "Craft ability" .


###  https://raw.githubusercontent.com/AbsVahter/trpgontologies/main/gumshoe/cthulhu_confidential/PELGOC01.ttl#cryptography
:cryptography rdf:type owl:NamedIndividual ,
                       :AcademicAbility ;
              :application "given some time and a dictionary, you may be able to puzzle out foreign alphabets, translating languages by brute force" ,
                           "make or break codes and ciphers in any language you can read" ;
              rdfs:comment "You can make or break codes and ciphers in any language you can read." ;
              rdfs:label "Cryptography ability" .


###  https://raw.githubusercontent.com/AbsVahter/trpgontologies/main/gumshoe/cthulhu_confidential/PELGOC01.ttl#cthulhu_mythos
:cthulhu_mythos rdf:type owl:NamedIndividual ,
                         :AcademicAbility ;
                :application "distinguish a practitioner of an ordinary, ineffectual human occult tradition from a sorcerer able to call on the power of the Old Ones" ,
                             "identify inhuman creatures and their spoor" ,
                             "identify which alien god has incarnated itself inside the formless monster that is currently crushing the life out of you" ,
                             "read inscriptions of the far-distant past predict what comes next when watching cultists perform an obscene rite" ,
                             "translate pre-human tongues" ;
                rdfs:comment "You have begun to piece together the secret rules of the real world, rather than the ignorant scrim of physics and religion. You recognize the great names, and the truths they conceal." ;
                rdfs:label "Cthulhu mythos ability" .


###  https://raw.githubusercontent.com/AbsVahter/trpgontologies/main/gumshoe/cthulhu_confidential/PELGOC01.ttl#devices
:devices rdf:type owl:NamedIndividual ,
                  :ManualAbility ;
         :application "create jury-rigged devices and booby-traps from odd bits of scrap" ,
                      "determine the function of a given piece of equipment" ,
                      "evaluate the quality of workmanship used to create an item" ,
                      "know the workings of electrical devices from simple alarm systems to the most advanced radios" ,
                      "make high-quality audio recordings on records, Dictaphone cylinders, or wire" ,
                      "operate and (where relevant) drive a new type of heavy machinery, once per case" ,
                      "read Morse Code" ,
                      "tap telephone or telegraph lines" ,
                      "use a device in good repair as intended" ;
         rdfs:comment "You build, repair, and operate electrical or mechanical devices. And what you can put together, you can take apart, disabling equipment either unnoticeably or completely." ;
         rdfs:label "Devices ability" .


###  https://raw.githubusercontent.com/AbsVahter/trpgontologies/main/gumshoe/cthulhu_confidential/PELGOC01.ttl#devices_challenge
:devices_challenge rdf:type owl:NamedIndividual ,
                            :Challenge ;
                   :uses :devices_die_roll ;
                   rdfs:label "Devices challenge" .


###  https://raw.githubusercontent.com/AbsVahter/trpgontologies/main/gumshoe/cthulhu_confidential/PELGOC01.ttl#devices_die_roll
:devices_die_roll rdf:type owl:NamedIndividual ,
                           :DieRoll ;
                  :uses :devices ;
                  rdfs:label "Devices die roll" .


###  https://raw.githubusercontent.com/AbsVahter/trpgontologies/main/gumshoe/cthulhu_confidential/PELGOC01.ttl#disguise
:disguise rdf:type owl:NamedIndividual ,
                   :ManualAbility ;
          :application "blend into a crowd in the street" ,
                       "hold an entire conversation with an unwitting friend or suspect" ,
                       "impersonate someone on the phone" ,
                       "mingle at a party with those outside your social station" ;
          rdfs:comment "You can become someone else: clothes, voice, mannerisms, and posture." ;
          rdfs:label "Disguise ability" .


###  https://raw.githubusercontent.com/AbsVahter/trpgontologies/main/gumshoe/cthulhu_confidential/PELGOC01.ttl#disguise_challenge
:disguise_challenge rdf:type owl:NamedIndividual ,
                             :Challenge ;
                    :uses :disguise_die_roll ;
                    rdfs:label "Disguise challenge" .


###  https://raw.githubusercontent.com/AbsVahter/trpgontologies/main/gumshoe/cthulhu_confidential/PELGOC01.ttl#disguise_die_roll
:disguise_die_roll rdf:type owl:NamedIndividual ,
                            :DieRoll ;
                   :uses :disguise ;
                   rdfs:label "Disguise die roll" .


###  https://raw.githubusercontent.com/AbsVahter/trpgontologies/main/gumshoe/cthulhu_confidential/PELGOC01.ttl#driving
:driving rdf:type owl:NamedIndividual ,
                  :ManualAbility ;
         :application "avoid collisions, or minimize damage from collisions" ,
                      "drive another type of vehicle requiring specialized training, once per case" ,
                      "evade or conduct pursuit" ,
                      "navigate, read maps, and maintain a sense of direction" ;
         rdfs:comment "Anyone who’s been taught can drive a car down the road without this ability. You, on the other hand, are a skilled defensive driver, capable of wringing high performance from even the most recalcitrant automobile, pickup truck, or bus." ;
         rdfs:label "Driving ability" .


###  https://raw.githubusercontent.com/AbsVahter/trpgontologies/main/gumshoe/cthulhu_confidential/PELGOC01.ttl#driving_challenge
:driving_challenge rdf:type owl:NamedIndividual ,
                            :Challenge ;
                   :uses :driving_die_roll ;
                   rdfs:label "Driving challenge" .


###  https://raw.githubusercontent.com/AbsVahter/trpgontologies/main/gumshoe/cthulhu_confidential/PELGOC01.ttl#driving_die_roll
:driving_die_roll rdf:type owl:NamedIndividual ,
                           :DieRoll ;
                  :uses :driving ;
                  rdfs:label "Driving die roll" .


###  https://raw.githubusercontent.com/AbsVahter/trpgontologies/main/gumshoe/cthulhu_confidential/PELGOC01.ttl#evidence_collection
:evidence_collection rdf:type owl:NamedIndividual ,
                              :TechnicalAbility ;
                     :application "discover items others have concealed" ,
                                  "find, transfer, take, and compare fingerprints" ,
                                  "match handwriting to a known sample" ,
                                  "match typewritten materials to a given machine" ,
                                  "note relationships between objects at a crime scene, reconstructing sequences of events" ,
                                  "spot hidden objects or objects of interest (such as bullet casings under a couch, or drops of blue ooze behind a desk) at a crime scene or other investigation site" ,
                                  "store objects for forensic analysis without contaminating your samples" ;
                     rdfs:comment "You’re adept at casing an investigation site and at finding important clues." ;
                     rdfs:label "Evidence collection ability" .


###  https://raw.githubusercontent.com/AbsVahter/trpgontologies/main/gumshoe/cthulhu_confidential/PELGOC01.ttl#explosives
:explosives rdf:type owl:NamedIndividual ,
                     :ManualAbility ;
            :application "defuse bombs and traps" ,
                         "figure out the configuration of a bomb from its blast effect and shrapnel" ,
                         "for any bomb (exploded or unexploded), determine the method and materials of the bomb-maker, and deduce his sophistication, background, and skill" ,
                         "given time, blow open safes or vaults without damaging the contents" ,
                         "handle nitroglycerin or other dangerously unstable materials with relative safety" ,
                         "mix explosive compounds from common chemicals" ,
                         "safely construct and detonate explosive devices or booby-traps of your own" ;
            rdfs:comment "expert in bombs and booby-traps" ;
            rdfs:label "Explosives ability" .


###  https://raw.githubusercontent.com/AbsVahter/trpgontologies/main/gumshoe/cthulhu_confidential/PELGOC01.ttl#explosives_challenge
:explosives_challenge rdf:type owl:NamedIndividual ,
                               :Challenge ;
                      :uses :explosives_die_roll ;
                      rdfs:label "Explosives challenge" .


###  https://raw.githubusercontent.com/AbsVahter/trpgontologies/main/gumshoe/cthulhu_confidential/PELGOC01.ttl#explosives_die_roll
:explosives_die_roll rdf:type owl:NamedIndividual ,
                              :DieRoll ;
                     :uses :explosives ;
                     rdfs:label "Explosives die roll" .


###  https://raw.githubusercontent.com/AbsVahter/trpgontologies/main/gumshoe/cthulhu_confidential/PELGOC01.ttl#fighting
:fighting rdf:type owl:NamedIndividual ,
                   :PhysicalAbility ;
          :application "hand-to-hand weapons" ,
                       "scuffling" ,
                       "shooting" ;
          rdfs:comment "covers all forms of combat, from scuffling to shooting to hand-to-hand weapons" ;
          rdfs:label "Fighting ability" .


###  https://raw.githubusercontent.com/AbsVahter/trpgontologies/main/gumshoe/cthulhu_confidential/PELGOC01.ttl#fighting_challenge
:fighting_challenge rdf:type owl:NamedIndividual ,
                             :Challenge ;
                    :uses :fighting_die_roll ;
                    rdfs:label "Fighting challenge" .


###  https://raw.githubusercontent.com/AbsVahter/trpgontologies/main/gumshoe/cthulhu_confidential/PELGOC01.ttl#fighting_die_roll
:fighting_die_roll rdf:type owl:NamedIndividual ,
                            :DieRoll ;
                   :uses :fighting ;
                   rdfs:label "Fighting die roll" .


###  https://raw.githubusercontent.com/AbsVahter/trpgontologies/main/gumshoe/cthulhu_confidential/PELGOC01.ttl#filch
:filch rdf:type owl:NamedIndividual ,
                :ManualAbility ;
       :application "pick pockets" ,
                    "pilfer clues from (or plant clues at) a crime scene under the very noses of unsuspecting authorities" ,
                    "plant objects on unsuspecting subjects" ;
       rdfs:comment "Your nimble fingers allow you to unobtrusively manipulate small objects." ;
       rdfs:label "Filch ability" .


###  https://raw.githubusercontent.com/AbsVahter/trpgontologies/main/gumshoe/cthulhu_confidential/PELGOC01.ttl#filch_challenge
:filch_challenge rdf:type owl:NamedIndividual ,
                          :Challenge ;
                 :uses :filch_die_roll ;
                 rdfs:label "Filch challenge" .


###  https://raw.githubusercontent.com/AbsVahter/trpgontologies/main/gumshoe/cthulhu_confidential/PELGOC01.ttl#filch_die_roll
:filch_die_roll rdf:type owl:NamedIndividual ,
                         :DieRoll ;
                :uses :filch ;
                rdfs:label "Filch die roll" .


###  https://raw.githubusercontent.com/AbsVahter/trpgontologies/main/gumshoe/cthulhu_confidential/PELGOC01.ttl#first_aid
:first_aid rdf:type owl:NamedIndividual ,
                    :ManualAbility ;
           :application "first aid on sick or injured individuals" ;
           rdfs:comment "You can perform first aid on sick or injured individuals, including yourself." ;
           rdfs:label "First aid ability" .


###  https://raw.githubusercontent.com/AbsVahter/trpgontologies/main/gumshoe/cthulhu_confidential/PELGOC01.ttl#first_aid_challenge
:first_aid_challenge rdf:type owl:NamedIndividual ,
                              :Challenge ;
                     :uses :first_aid_die_roll ;
                     rdfs:label "First aid challenge" .


###  https://raw.githubusercontent.com/AbsVahter/trpgontologies/main/gumshoe/cthulhu_confidential/PELGOC01.ttl#first_aid_die_roll
:first_aid_die_roll rdf:type owl:NamedIndividual ,
                             :DieRoll ;
                    :uses :first_aid ;
                    rdfs:label "First aid die roll" .


###  https://raw.githubusercontent.com/AbsVahter/trpgontologies/main/gumshoe/cthulhu_confidential/PELGOC01.ttl#flattery
:flattery rdf:type owl:NamedIndividual ,
                   :InterpersonalAbility ;
          :application "date you (if applicable)" ,
                       "perform minor favors" ,
                       "regard you as trustworthy" ,
                       "reveal information" ;
          rdfs:comment "You get people to help you by complimenting or playing up to them, as subtly or blatantly as they prefer." ;
          rdfs:label "Flattery ability" .


###  https://raw.githubusercontent.com/AbsVahter/trpgontologies/main/gumshoe/cthulhu_confidential/PELGOC01.ttl#fleeing
:fleeing rdf:type owl:NamedIndividual ,
                  :PhysicalAbility ;
         :application "run away from impending danger" ;
         rdfs:comment "This ability governs how speedily you run away from impending danger." ;
         rdfs:label "Fleeing ability" .


###  https://raw.githubusercontent.com/AbsVahter/trpgontologies/main/gumshoe/cthulhu_confidential/PELGOC01.ttl#fleeing_challenge
:fleeing_challenge rdf:type owl:NamedIndividual ,
                            :Challenge ;
                   :uses :fleeing_die_roll ;
                   rdfs:label "Fleeing challenge" .


###  https://raw.githubusercontent.com/AbsVahter/trpgontologies/main/gumshoe/cthulhu_confidential/PELGOC01.ttl#fleeing_die_roll
:fleeing_die_roll rdf:type owl:NamedIndividual ,
                           :DieRoll ;
                  :uses :fleeing ;
                  rdfs:label "Fleeing die roll" .


###  https://raw.githubusercontent.com/AbsVahter/trpgontologies/main/gumshoe/cthulhu_confidential/PELGOC01.ttl#forensics
:forensics rdf:type owl:NamedIndividual ,
                    :TechnicalAbility ;
           :application "reconstruct the sequence of events leading to the victim’s death from the arrangement of wounds on the body" ,
                        "the approximate time of death" ,
                        "the contents of the victim’s last meal" ,
                        "the nature of the weapon or weapons used" ,
                        "the presence of intoxicants or other foreign substances in the bloodstream or on the skin" ;
           rdfs:comment "You study crime scenes and perform autopsies on deceased subjects to determine their cause and circumstances of death. You can use skeletal evidence to reconstruct the physical details (age, sex, medical condition, sometimes occupation) of the deceased." ;
           rdfs:label "Forensics ability" .


###  https://raw.githubusercontent.com/AbsVahter/trpgontologies/main/gumshoe/cthulhu_confidential/PELGOC01.ttl#geology
:geology rdf:type owl:NamedIndividual ,
                  :AcademicAbility ;
         :application "analyze soil samples, crystals, minerals, and so forth" ,
                      "anticipate vulcanism, seismic events, avalanches, and other earth phenomena" ,
                      "date and identify fossils" ,
                      "determine the age of a rock stratum" ,
                      "evaluate soil for agriculture or industry" ,
                      "identify promising sites for oil or water wells, mines, etc." ;
         rdfs:comment "You are expert on rocks, soils, minerals, and the primordial history of the Earth." ;
         rdfs:label "Geology ability" .


###  https://raw.githubusercontent.com/AbsVahter/trpgontologies/main/gumshoe/cthulhu_confidential/PELGOC01.ttl#history
:history rdf:type owl:NamedIndividual ,
                  :AcademicAbility ;
         :application "(if based in L.A.) name Hollywood productions set in a particular historical period, supplemented with a list of their ludicrous inaccuracies" ,
                      "determine the age of a document" ,
                      "identify ancient languages and scripts (assuming they’re of human origin)" ,
                      "identify the period of an article of dress or costume" ,
                      "perform textual analysis on a manuscript or book to date it or identify the author" ,
                      "recall important or relevant events in a given country, city, or region" ,
                      "recognize obscure historical allusions" ,
                      "tell where and when an object made during historical times was fashioned" ;
         rdfs:comment "A broad study of recorded human history, with an emphasis on political, military, economic, and technological developments." ;
         rdfs:label "History ability" .


###  https://raw.githubusercontent.com/AbsVahter/trpgontologies/main/gumshoe/cthulhu_confidential/PELGOC01.ttl#hypnosis
:hypnosis rdf:type owl:NamedIndividual ,
                   :MentalAbility ;
          :application "recover lost memories" ,
                       "remove destructive compulsions" ,
                       "suppress unwanted memories" ;
          rdfs:comment "You can hypnotize a willing subject, recovering lost memories, suppressing unwanted ones, or removing destructive compulsions." ;
          rdfs:label "Hypnosis ability" .


###  https://raw.githubusercontent.com/AbsVahter/trpgontologies/main/gumshoe/cthulhu_confidential/PELGOC01.ttl#hypnosis_challenge
:hypnosis_challenge rdf:type owl:NamedIndividual ,
                             :Challenge ;
                    :uses :hypnosis_die_roll ;
                    rdfs:label "Hypnosis challenge" .


###  https://raw.githubusercontent.com/AbsVahter/trpgontologies/main/gumshoe/cthulhu_confidential/PELGOC01.ttl#hypnosis_die_roll
:hypnosis_die_roll rdf:type owl:NamedIndividual ,
                            :DieRoll ;
                   :uses :hypnosis ;
                   rdfs:label "Hypnosis die roll" .


###  https://raw.githubusercontent.com/AbsVahter/trpgontologies/main/gumshoe/cthulhu_confidential/PELGOC01.ttl#inspiration
:inspiration rdf:type owl:NamedIndividual ,
                      :InterpersonalAbility ;
             :application "call to belief in a secular ideology, whether it be democracy, Marxism, or pacifism" ,
                          "call to desire for justice" ,
                          "call to love of friends, family, or community" ,
                          "call to pride in personal achievement" ,
                          "call to religious beliefs" ,
                          "call to sense of fairness" ;
             rdfs:comment "You can convince reluctant witnesses to supply information by appealing to their better selves. After a few moments of interaction, you intuitively sense the positive values they hold dearest, then invoke them in a brief but stirring speech." ;
             rdfs:label "Inspiration ability" .


###  https://raw.githubusercontent.com/AbsVahter/trpgontologies/main/gumshoe/cthulhu_confidential/PELGOC01.ttl#intimidation
:intimidation rdf:type owl:NamedIndividual ,
                       :InterpersonalAbility ;
              :application "extract promises of future cooperation, secured by the threat of your later retaliation" ,
                           "gain information" ,
                           "inspire the subject to leave the area" ,
                           "quell a subject’s desire to attempt violence against you or others" ;
              rdfs:comment "You get what you want from people by scaring them — physically, or with vividly detailed threats." ;
              rdfs:label "Intimidation ability" .


###  https://raw.githubusercontent.com/AbsVahter/trpgontologies/main/gumshoe/cthulhu_confidential/PELGOC01.ttl#languages
:languages rdf:type owl:NamedIndividual ,
                    :AcademicAbility ;
           :application "extract information from documents written in languages other than English" ;
           rdfs:comment "Allows you to extract information from documents written in languages other than English. You may not be able to elegantly translate or win points for accuracy among true academics, but you find the clue you need." ;
           rdfs:label "Languages ability" .


###  https://raw.githubusercontent.com/AbsVahter/trpgontologies/main/gumshoe/cthulhu_confidential/PELGOC01.ttl#law
:law rdf:type owl:NamedIndividual ,
              :AcademicAbility ;
     :application "assess the legal risks attendant on any course of action" ,
                  "call on legal colleagues or contacts for favors and advice" ,
                  "convincingly dispute the legality of actions undertaken by police and prosecutors" ,
                  "understand lawyerly jargon" ;
     rdfs:comment "You are familiar with the criminal and civil laws that pertain in your noir city, as well as on the state and federal levels. You can bluff your way through dealings with foreign legal systems." ;
     rdfs:label "Law ability" .


###  https://raw.githubusercontent.com/AbsVahter/trpgontologies/main/gumshoe/cthulhu_confidential/PELGOC01.ttl#locksmith
:locksmith rdf:type owl:NamedIndividual ,
                    :TechnicalAbility ;
           :application "disarm alarms" ,
                        "find convenient windows to jimmy or coal-cellar doors to force" ,
                        "open doors and locks" ;
           rdfs:comment "You can open doors and locks, and disarm alarms, without benefit of a key. Or maybe you have some universal passkeys with you." ;
           rdfs:label "Locksmith ability" .


###  https://raw.githubusercontent.com/AbsVahter/trpgontologies/main/gumshoe/cthulhu_confidential/PELGOC01.ttl#magic
:magic rdf:type owl:NamedIndividual ,
                :MentalAbility ;
       :application "harm opponent with magic" ,
                    "subject opponent to mental influence with magic" ;
       rdfs:comment "learn and practice efficacious magic" ;
       rdfs:label "Magic ability" .


###  https://raw.githubusercontent.com/AbsVahter/trpgontologies/main/gumshoe/cthulhu_confidential/PELGOC01.ttl#magic_challenge
:magic_challenge rdf:type owl:NamedIndividual ,
                          :Challenge ;
                 :uses :magic_die_roll ;
                 rdfs:label "Magic challenge" .


###  https://raw.githubusercontent.com/AbsVahter/trpgontologies/main/gumshoe/cthulhu_confidential/PELGOC01.ttl#magic_die_roll
:magic_die_roll rdf:type owl:NamedIndividual ,
                         :DieRoll ;
                :uses :magic ;
                rdfs:label "Magic die roll" .


###  https://raw.githubusercontent.com/AbsVahter/trpgontologies/main/gumshoe/cthulhu_confidential/PELGOC01.ttl#medicine
:medicine rdf:type owl:NamedIndividual ,
                   :AcademicAbility ;
          :application "deliver a baby" ,
                       "detect when a person is suffering from a physically debilitating condition such as drug addiction, pregnancy, or malnutrition" ,
                       "diagnose diseases, poisonings, and other ailments" ,
                       "establish a person’s general level of health" ,
                       "identify medical abnormalities" ,
                       "identify the extent and cause of an unconscious person’s trauma" ,
                       "prescribe remedies for a treatable condition" ,
                       "understand medical jargon" ;
          rdfs:comment "You can diagnose human disease, injuries, poisonings, and physical frailties, and may be broadly acquainted with veterinary medicine as well. If past medical training makes sense as part of your backstory, you may still hold a medical license." ;
          rdfs:label "Medicine ability" .


###  https://raw.githubusercontent.com/AbsVahter/trpgontologies/main/gumshoe/cthulhu_confidential/PELGOC01.ttl#occult
:occult rdf:type owl:NamedIndividual ,
                 :AcademicAbility ;
        :application "fake a fortune-telling session, séance, or other occult activity" ,
                     "guess the intended effect of a ritual from its physical traces identify occult activities as the work of informed practitioners or dilettante thrill-seekers" ,
                     "identify occult paraphernalia, grimoires, symbols, and codes" ,
                     "identify the cultural traditions informing a ritual by examining its physical remnants" ,
                     "read and cast a horoscope" ,
                     "supply historical facts and anecdotes concerning various occult traditions, demons, and legends" ;
        rdfs:comment "You’re an expert in the historical study of magic, superstition, and sorcery from the Stone Age to the present" ;
        rdfs:label "Occult ability" .


###  https://raw.githubusercontent.com/AbsVahter/trpgontologies/main/gumshoe/cthulhu_confidential/PELGOC01.ttl#oral_history
:oral_history rdf:type owl:NamedIndividual ,
                       :InterpersonalAbility ;
              :application "do research in illiterate or semi-literate societies, and in rural or small-town communities in general" ,
                           "take shorthand notes or making recordings without spooking your sources" ;
              rdfs:comment "You can find sources willing to talk, win their confidence, and gather (usually lengthy) oral testimony about historical events, local traditions, folklore, family legend, or gossip." ;
              rdfs:label "Oral history ability" .


###  https://raw.githubusercontent.com/AbsVahter/trpgontologies/main/gumshoe/cthulhu_confidential/PELGOC01.ttl#outdoorsman
:outdoorsman rdf:type owl:NamedIndividual ,
                      :TechnicalAbility ;
             :application "find edible plants, hunt, and fish" ,
                          "hunt with dogs, including tracking with bloodhounds, assuming you have friendly dogs available" ,
                          "make fire and survive outdoors at night or in bad weather" ,
                          "navigate overland, albeit more easily with a compass and a map" ,
                          "tell when an animal is behaving strangely" ,
                          "tell whether an animal or plant is natural to a given area" ,
                          "track people, animals, or vehicles across grass or through forests" ;
             rdfs:comment "Long hours of camping and exploration in the wild have made it as comfortable to you as life in the concrete jungle." ;
             rdfs:label "Outdoorsman ability" .


###  https://raw.githubusercontent.com/AbsVahter/trpgontologies/main/gumshoe/cthulhu_confidential/PELGOC01.ttl#pharmacy
:pharmacy rdf:type owl:NamedIndividual ,
                   :TechnicalAbility ;
          :application "identify drugs and potions, and recognize their side-effects and contraindications" ,
                       "identify poisons and determine antidotes" ,
                       "secure or manufacture morphine, cocaine, and other controlled substances" ;
          rdfs:comment "You are able to identify and compound drugs and medicines." ;
          rdfs:label "Pharmacy ability" .


###  https://raw.githubusercontent.com/AbsVahter/trpgontologies/main/gumshoe/cthulhu_confidential/PELGOC01.ttl#photography
:photography rdf:type owl:NamedIndividual ,
                      :TechnicalAbility ;
             :application "(Los Angeles) look at a movie or professionally taken still photo and identify the studio employee who lensed it" ,
                          "(Los Angeles) put cinematographers at ease by talking shop with them about the latest equipment" ,
                          "develop film or plates and enhance hidden details" ,
                          "realistically retouch and manipulate photographic images" ,
                          "spot manual retouching or camera trickery in a photographic image or negative" ,
                          "take trick photographs using double exposures and other methods" ,
                          "take useful visual records of crime scenes or expeditions" ,
                          "use filters and lights to capture images only visible in infrared or ultraviolet" ;
             rdfs:comment "You’re proficient in the use of cameras, including still and motion-picture photography." ;
             rdfs:label "Photography ability" .


###  https://raw.githubusercontent.com/AbsVahter/trpgontologies/main/gumshoe/cthulhu_confidential/PELGOC01.ttl#physics
:physics rdf:type owl:NamedIndividual ,
                  :AcademicAbility ;
         :application "(perhaps) understand advanced or alien technologies" ,
                      "design or refit experimental machinery to test, detect, or manipulate physical forces and energies" ,
                      "obtain and operate expensive or obscure pieces of laboratory equipment such as Crookes tubes, Geiger counters, or magnetometers" ,
                      "understand and apply advanced mathematics, including non-Euclidean geometries" ;
         rdfs:comment "You study the fundamental forces of the universe: pressure, electromagnetism, motion, gravity, optics, and radioactivity." ;
         rdfs:label "Physics ability" .


###  https://raw.githubusercontent.com/AbsVahter/trpgontologies/main/gumshoe/cthulhu_confidential/PELGOC01.ttl#preparedness
:preparedness rdf:type owl:NamedIndividual ,
                       :ManualAbility ;
              :application "prepare tools for investigation" ;
              rdfs:comment "You expertly anticipate the needs of any investigation by packing a kit efficiently arranged with necessary gear." ;
              rdfs:label "Preparedness ability" .


###  https://raw.githubusercontent.com/AbsVahter/trpgontologies/main/gumshoe/cthulhu_confidential/PELGOC01.ttl#preparedness_challenge
:preparedness_challenge rdf:type owl:NamedIndividual ,
                                 :Challenge ;
                        :uses :preparedness_die_roll ;
                        rdfs:label "Preparedness challenge" .


###  https://raw.githubusercontent.com/AbsVahter/trpgontologies/main/gumshoe/cthulhu_confidential/PELGOC01.ttl#preparedness_die_roll
:preparedness_die_roll rdf:type owl:NamedIndividual ,
                                :DieRoll ;
                       :uses :preparedness ;
                       rdfs:label "Preparedness die roll" .


###  https://raw.githubusercontent.com/AbsVahter/trpgontologies/main/gumshoe/cthulhu_confidential/PELGOC01.ttl#psychoanalysis
:psychoanalysis rdf:type owl:NamedIndividual ,
                         :MentalAbility ;
                :application "provide comfort, perspective, and solace to the mentally troubled" ;
                rdfs:comment "You can provide comfort, perspective, and solace to the mentally troubled." ;
                rdfs:label "Psychoanalysis ability" .


###  https://raw.githubusercontent.com/AbsVahter/trpgontologies/main/gumshoe/cthulhu_confidential/PELGOC01.ttl#psychoanalysis_challenge
:psychoanalysis_challenge rdf:type owl:NamedIndividual ,
                                   :Challenge ;
                          :uses :psychoanalysis_die_roll ;
                          rdfs:label "Psychoanalysis challenge" .


###  https://raw.githubusercontent.com/AbsVahter/trpgontologies/main/gumshoe/cthulhu_confidential/PELGOC01.ttl#psychoanalysis_die_roll
:psychoanalysis_die_roll rdf:type owl:NamedIndividual ,
                                  :DieRoll ;
                         :uses :psychoanalysis ;
                         rdfs:label "Psychoanalysis die roll" .


###  https://raw.githubusercontent.com/AbsVahter/trpgontologies/main/gumshoe/cthulhu_confidential/PELGOC01.ttl#psychology
:psychology rdf:type owl:NamedIndividual ,
                     :InterpersonalAbility ;
            :application "distinguish an individual whose violence is deemed acceptable by his home culture from one who consciously defies cultural norms" ,
                         "distinguish subjects who can be successfully rehabilitated from the incorrigibly violent or deviant" ,
                         "predict their upcoming actions based on their past behavior" ,
                         "tell whether a known individual’s criminal behavior is in response to deep psychological impulses, or is driven primarily by greed" ;
            rdfs:comment "Your familiarity with the latest in the burgeoning field of human psychology grants you insight into the criminal mind. Based solely on their known modus operandi, you can make accurate guesses as to the upbringing and pathology of unidentified criminals." ;
            rdfs:label "Psychology ability" .


###  https://raw.githubusercontent.com/AbsVahter/trpgontologies/main/gumshoe/cthulhu_confidential/PELGOC01.ttl#reassurance
:reassurance rdf:type owl:NamedIndividual ,
                      :InterpersonalAbility ;
             :application "allay fear or panic in others" ,
                          "elicit information and minor favors" ,
                          "follows through on promises" ,
                          "gain trust" ,
                          "instill a sense of calm during a crisis" ,
                          "present yourself as someone who successfully" ;
             rdfs:comment "You can get people to do what you want by putting them at ease. This may involve fast talk, genuine sympathy, a rational accounting of risks, or just a calming presence." ;
             rdfs:label "Reassurance ability" .


###  https://raw.githubusercontent.com/AbsVahter/trpgontologies/main/gumshoe/cthulhu_confidential/PELGOC01.ttl#research
:research rdf:type owl:NamedIndividual ,
                   :AcademicAbility ;
          :application "determine patterns: who wrote about what and to whom, what kinds of books an eccentric collector values, what might be missing from the official files, which records seem doctored and by whom, and so forth" ,
                       "ferret out information from collections of data" ;
          rdfs:comment "You can ferret out information from collections of books, records, files, archives, newspaper morgues, or big piles of unsorted telegrams and correspondence." ;
          rdfs:label "Research ability" .


###  https://raw.githubusercontent.com/AbsVahter/trpgontologies/main/gumshoe/cthulhu_confidential/PELGOC01.ttl#sense_trouble
:sense_trouble rdf:type owl:NamedIndividual ,
                        :MentalAbility ;
               :application "have a bad feeling about that eerily hunchbacked priest at the seemingly deserted cathedral" ,
                            "hear the splash of a Deep One dropping into the sewer behind you" ,
                            "notice that those two palookas in the dark corner of the bar have been intently watching you all night long" ,
                            "realize that anyone up in that lighthouse will have seen you coming a mile away" ,
                            "see a flittering shape cross the moon" ;
               rdfs:comment "This ability allows you to perceive (either with sight or other senses) potential hazards to yourself or others." ;
               rdfs:label "Sense trouble ability" .


###  https://raw.githubusercontent.com/AbsVahter/trpgontologies/main/gumshoe/cthulhu_confidential/PELGOC01.ttl#sense_trouble_challenge
:sense_trouble_challenge rdf:type owl:NamedIndividual ,
                                  :Challenge ;
                         :uses :sense_trouble_die_roll ;
                         rdfs:label "Sense trouble challenge" .


###  https://raw.githubusercontent.com/AbsVahter/trpgontologies/main/gumshoe/cthulhu_confidential/PELGOC01.ttl#sense_trouble_die_roll
:sense_trouble_die_roll rdf:type owl:NamedIndividual ,
                                 :DieRoll ;
                        :uses :sense_trouble ;
                        rdfs:label "Sense trouble die roll" .


###  https://raw.githubusercontent.com/AbsVahter/trpgontologies/main/gumshoe/cthulhu_confidential/PELGOC01.ttl#shadowing
:shadowing rdf:type owl:NamedIndividual ,
                    :PhysicalAbility ;
           :application "anticipate blind spots in your coverage and plan for them, or use them to lose your own shadowers" ,
                        "find undetectable vantage points" ,
                        "hide in plain sight" ,
                        "use binoculars or telescopes to keep watch on a target from a distance" ;
           rdfs:comment "You follow suspects without revealing your presence." ;
           rdfs:label "Shadowing ability" .


###  https://raw.githubusercontent.com/AbsVahter/trpgontologies/main/gumshoe/cthulhu_confidential/PELGOC01.ttl#shadowing_challenge
:shadowing_challenge rdf:type owl:NamedIndividual ,
                              :Challenge ;
                     :uses :shadowing_die_roll ;
                     rdfs:label "Shadowing challenge" .


###  https://raw.githubusercontent.com/AbsVahter/trpgontologies/main/gumshoe/cthulhu_confidential/PELGOC01.ttl#shadowing_die_roll
:shadowing_die_roll rdf:type owl:NamedIndividual ,
                             :DieRoll ;
                    :uses :shadowing ;
                    rdfs:label "Shadowing die roll" .


###  https://raw.githubusercontent.com/AbsVahter/trpgontologies/main/gumshoe/cthulhu_confidential/PELGOC01.ttl#stability
:stability rdf:type owl:NamedIndividual ,
                    :MentalAbility ;
           :application "appear calm to others, even when terrified inside" ,
                        "avoid or suppress physical symptoms of terror and disgust, from nausea to adrenaline rush" ,
                        "file a weird sight deep in your memory, keeping your mind intact by refusing to entertain its true significance" ,
                        "move toward danger a self-protective person would avoid" ;
           rdfs:comment "Remain in control of your thoughts and actions when confronted with frightening or traumatic sights, sounds, or other sensory input." ;
           rdfs:label "Stability ability" .


###  https://raw.githubusercontent.com/AbsVahter/trpgontologies/main/gumshoe/cthulhu_confidential/PELGOC01.ttl#stability_challenge
:stability_challenge rdf:type owl:NamedIndividual ,
                              :Challenge ;
                     :uses :stability_die_roll ;
                     rdfs:label "Stchallenge challenge" .


###  https://raw.githubusercontent.com/AbsVahter/trpgontologies/main/gumshoe/cthulhu_confidential/PELGOC01.ttl#stability_die_roll
:stability_die_roll rdf:type owl:NamedIndividual ,
                             :DieRoll ;
                    :uses :stability ;
                    rdfs:label "Stdie roll die roll" .


###  https://raw.githubusercontent.com/AbsVahter/trpgontologies/main/gumshoe/cthulhu_confidential/PELGOC01.ttl#stealth
:stealth rdf:type owl:NamedIndividual ,
                  :PhysicalAbility ;
         :application "evade visual security, whether guards (usual) or cameras (unusual)" ,
                      "hide in shadows or cover" ,
                      "listen at doors or windows without being overheard yourself" ,
                      "move silently" ;
         rdfs:comment "You’re good at moving (and standing still) without being noticed." ;
         rdfs:label "Stealth ability" .


###  https://raw.githubusercontent.com/AbsVahter/trpgontologies/main/gumshoe/cthulhu_confidential/PELGOC01.ttl#stealth_challenge
:stealth_challenge rdf:type owl:NamedIndividual ,
                            :Challenge ;
                   :uses :stealth_die_roll ;
                   rdfs:label "Stealth challenge" .


###  https://raw.githubusercontent.com/AbsVahter/trpgontologies/main/gumshoe/cthulhu_confidential/PELGOC01.ttl#stealth_die_roll
:stealth_die_roll rdf:type owl:NamedIndividual ,
                           :DieRoll ;
                  :uses :stealth ;
                  rdfs:label "Stealth die roll" .


###  https://raw.githubusercontent.com/AbsVahter/trpgontologies/main/gumshoe/cthulhu_confidential/PELGOC01.ttl#streetwise
:streetwise rdf:type owl:NamedIndividual ,
                     :InterpersonalAbility ;
            :application "gather underworld rumors" ,
                         "identify unsafe locations and dangerous people" ,
                         "identify your city’s gangland players and understand their power relationships, even if these have recently changed" ,
                         "make and utilize criminal contacts — fences, black marketeers, drug dealers, gun runners, and so forth" ,
                         "successfully price illegal goods such as drugs, stolen items, or weapons" ,
                         "use criminal etiquette to avoid fights and conflicts" ;
            rdfs:comment "You know how to behave among crooks, gangsters, dopers, hookers, grifters, and other habitués of the criminal underworld." ;
            rdfs:label "Streetwise ability" .


###  https://raw.githubusercontent.com/AbsVahter/trpgontologies/main/gumshoe/cthulhu_confidential/PELGOC01.ttl#theology
:theology rdf:type owl:NamedIndividual ,
                   :AcademicAbility ;
          :application "fake (or in some traditions, officiate at) a religious ceremony" ,
                       "identify whether a given religious practice or ritual is orthodox or heretical" ,
                       "know the prominent faiths and religious figures of your noir city — for example, the many wild new cults of the L.A. basin" ,
                       "quote relevant passages from the major scriptures" ,
                       "recognize the names and attributes of various saints, gods, and other figures of religious worship and veneration" ,
                       "supply information about religious practices and beliefs" ;
          rdfs:comment "You study human religions in their various forms, both ancient and modern." ;
          rdfs:label "Theology ability" .


###  Generated by the OWL API (version 4.5.25.2023-02-15T19:15:49Z) https://github.com/owlcs/owlapi
