@prefix : <https://raw.githubusercontent.com/AbsVahter/ontoTRPG/main/crown_and_skull/crown_and_skull.ttl#> .
@prefix gen: <https://raw.githubusercontent.com/AbsVahter/ontoTRPG/main/ontoGeneral.ttl#> .
@prefix owl: <http://www.w3.org/2002/07/owl#> .
@prefix rdf: <http://www.w3.org/1999/02/22-rdf-syntax-ns#> .
@prefix xml: <http://www.w3.org/XML/1998/namespace> .
@prefix xsd: <http://www.w3.org/2001/XMLSchema#> .
@prefix rdfs: <http://www.w3.org/2000/01/rdf-schema#> .
@base <https://raw.githubusercontent.com/AbsVahter/ontoTRPG/main/crown_and_skull/crown_and_skull.ttl#> .

<https://raw.githubusercontent.com/AbsVahter/ontoTRPG/main/crown_and_skull/crown_and_skull.ttl#> rdf:type owl:Ontology ;
                                                                                                  owl:imports gen: .

#################################################################
#    Annotation properties
#################################################################

###  https://raw.githubusercontent.com/AbsVahter/ontoTRPG/main/ontoGeneral.ttl#Location
gen:Location rdf:type owl:AnnotationProperty .


###  https://raw.githubusercontent.com/AbsVahter/ontoTRPG/main/ontoGeneral.ttl#after
gen:after rdf:type owl:AnnotationProperty .


###  https://raw.githubusercontent.com/AbsVahter/ontoTRPG/main/ontoGeneral.ttl#basedOn
gen:basedOn rdf:type owl:AnnotationProperty .


###  https://raw.githubusercontent.com/AbsVahter/ontoTRPG/main/ontoGeneral.ttl#blocked
gen:blocked rdf:type owl:AnnotationProperty .


###  https://raw.githubusercontent.com/AbsVahter/ontoTRPG/main/ontoGeneral.ttl#checkFailure
gen:checkFailure rdf:type owl:AnnotationProperty .


###  https://raw.githubusercontent.com/AbsVahter/ontoTRPG/main/ontoGeneral.ttl#checkSuccess
gen:checkSuccess rdf:type owl:AnnotationProperty .


###  https://raw.githubusercontent.com/AbsVahter/ontoTRPG/main/ontoGeneral.ttl#checkThreshold
gen:checkThreshold rdf:type owl:AnnotationProperty .


###  https://raw.githubusercontent.com/AbsVahter/ontoTRPG/main/ontoGeneral.ttl#damage
gen:damage rdf:type owl:AnnotationProperty .


###  https://raw.githubusercontent.com/AbsVahter/ontoTRPG/main/ontoGeneral.ttl#defense
gen:defense rdf:type owl:AnnotationProperty .


###  https://raw.githubusercontent.com/AbsVahter/ontoTRPG/main/ontoGeneral.ttl#duration
gen:duration rdf:type owl:AnnotationProperty .


###  https://raw.githubusercontent.com/AbsVahter/ontoTRPG/main/ontoGeneral.ttl#effectOption
gen:effectOption rdf:type owl:AnnotationProperty .


###  https://raw.githubusercontent.com/AbsVahter/ontoTRPG/main/ontoGeneral.ttl#included
gen:included rdf:type owl:AnnotationProperty .


###  https://raw.githubusercontent.com/AbsVahter/ontoTRPG/main/ontoGeneral.ttl#input
gen:input rdf:type owl:AnnotationProperty .


###  https://raw.githubusercontent.com/AbsVahter/ontoTRPG/main/ontoGeneral.ttl#inputOption
gen:inputOption rdf:type owl:AnnotationProperty .


###  https://raw.githubusercontent.com/AbsVahter/ontoTRPG/main/ontoGeneral.ttl#modified
gen:modified rdf:type owl:AnnotationProperty .


###  https://raw.githubusercontent.com/AbsVahter/ontoTRPG/main/ontoGeneral.ttl#motive
gen:motive rdf:type owl:AnnotationProperty .


###  https://raw.githubusercontent.com/AbsVahter/ontoTRPG/main/ontoGeneral.ttl#resource
gen:resource rdf:type owl:AnnotationProperty .


###  https://raw.githubusercontent.com/AbsVahter/ontoTRPG/main/ontoGeneral.ttl#set
gen:set rdf:type owl:AnnotationProperty .


###  https://raw.githubusercontent.com/AbsVahter/ontoTRPG/main/ontoGeneral.ttl#setCurrent
gen:setCurrent rdf:type owl:AnnotationProperty .


###  https://raw.githubusercontent.com/AbsVahter/ontoTRPG/main/ontoGeneral.ttl#target
gen:target rdf:type owl:AnnotationProperty .


###  https://raw.githubusercontent.com/AbsVahter/ontoTRPG/main/ontoGeneral.ttl#valueNumeric
gen:valueNumeric rdf:type owl:AnnotationProperty .


###  https://raw.githubusercontent.com/AbsVahter/ontoTRPG/main/ontoGeneral.ttl#valueObject
gen:valueObject rdf:type owl:AnnotationProperty .


###  https://raw.githubusercontent.com/AbsVahter/ontoTRPG/main/ontoGeneral.ttl#gen:setAdditive
gen:gen:setAdditive rdf:type owl:AnnotationProperty .


#################################################################
#    Data properties
#################################################################

###  https://raw.githubusercontent.com/AbsVahter/ontoTRPG/main/crown_and_skull/crown_and_skull.ttl#tier
:tier rdf:type owl:DatatypeProperty ;
      rdfs:domain :MagicAdvancement ;
      rdfs:range xsd:integer .


#################################################################
#    Classes
#################################################################

###  https://raw.githubusercontent.com/AbsVahter/ontoTRPG/main/crown_and_skull/crown_and_skull.ttl#Ability
:Ability rdf:type owl:Class ;
         rdfs:subClassOf :RequiredDetails .


###  https://raw.githubusercontent.com/AbsVahter/ontoTRPG/main/crown_and_skull/crown_and_skull.ttl#Attrition
:Attrition rdf:type owl:Class ;
           rdfs:subClassOf gen:Act ,
                           [ rdf:type owl:Restriction ;
                             owl:onProperty gen:effect ;
                             owl:hasValue :set_status_close_to_death
                           ] .


###  https://raw.githubusercontent.com/AbsVahter/ontoTRPG/main/crown_and_skull/crown_and_skull.ttl#Companion
:Companion rdf:type owl:Class ;
           rdfs:subClassOf gen:Creature .


###  https://raw.githubusercontent.com/AbsVahter/ontoTRPG/main/crown_and_skull/crown_and_skull.ttl#CoreAbility
:CoreAbility rdf:type owl:Class ;
             rdfs:subClassOf :Ability .


###  https://raw.githubusercontent.com/AbsVahter/ontoTRPG/main/crown_and_skull/crown_and_skull.ttl#Effect
:Effect rdf:type owl:Class ;
        rdfs:subClassOf gen:Act ;
        rdfs:label "Effect"@en .


###  https://raw.githubusercontent.com/AbsVahter/ontoTRPG/main/crown_and_skull/crown_and_skull.ttl#EffectCompanion
:EffectCompanion rdf:type owl:Class ;
                 rdfs:subClassOf :Effect .


###  https://raw.githubusercontent.com/AbsVahter/ontoTRPG/main/crown_and_skull/crown_and_skull.ttl#EffectItem
:EffectItem rdf:type owl:Class ;
            rdfs:subClassOf :Effect .


###  https://raw.githubusercontent.com/AbsVahter/ontoTRPG/main/crown_and_skull/crown_and_skull.ttl#EffectSpell
:EffectSpell rdf:type owl:Class ;
             rdfs:subClassOf :Effect .


###  https://raw.githubusercontent.com/AbsVahter/ontoTRPG/main/crown_and_skull/crown_and_skull.ttl#Flaw
:Flaw rdf:type owl:Class ;
      rdfs:label "Flaw"@en .


###  https://raw.githubusercontent.com/AbsVahter/ontoTRPG/main/crown_and_skull/crown_and_skull.ttl#FlawBasic
:FlawBasic rdf:type owl:Class ;
           rdfs:subClassOf :Flaw .


###  https://raw.githubusercontent.com/AbsVahter/ontoTRPG/main/crown_and_skull/crown_and_skull.ttl#FlawCrownAndSkull
:FlawCrownAndSkull rdf:type owl:Class ;
                   rdfs:subClassOf :Flaw ;
                   rdfs:label "Flaw after crown and skull choice"@en .


###  https://raw.githubusercontent.com/AbsVahter/ontoTRPG/main/crown_and_skull/crown_and_skull.ttl#Item
:Item rdf:type owl:Class ;
      rdfs:subClassOf :RequiredDetails .


###  https://raw.githubusercontent.com/AbsVahter/ontoTRPG/main/crown_and_skull/crown_and_skull.ttl#ItemArmor
:ItemArmor rdf:type owl:Class ;
           rdfs:subClassOf :Item .


###  https://raw.githubusercontent.com/AbsVahter/ontoTRPG/main/crown_and_skull/crown_and_skull.ttl#ItemBasic
:ItemBasic rdf:type owl:Class ;
           rdfs:subClassOf :Item .


###  https://raw.githubusercontent.com/AbsVahter/ontoTRPG/main/crown_and_skull/crown_and_skull.ttl#ItemCrown
:ItemCrown rdf:type owl:Class ;
           rdfs:subClassOf :Item .


###  https://raw.githubusercontent.com/AbsVahter/ontoTRPG/main/crown_and_skull/crown_and_skull.ttl#ItemLarge
:ItemLarge rdf:type owl:Class ;
           rdfs:subClassOf :Item ;
           rdfs:label "Large item"@en .


###  https://raw.githubusercontent.com/AbsVahter/ontoTRPG/main/crown_and_skull/crown_and_skull.ttl#ItemSkull
:ItemSkull rdf:type owl:Class ;
           rdfs:subClassOf :Item .


###  https://raw.githubusercontent.com/AbsVahter/ontoTRPG/main/crown_and_skull/crown_and_skull.ttl#ItemWeapon
:ItemWeapon rdf:type owl:Class ;
            rdfs:subClassOf :Item .


###  https://raw.githubusercontent.com/AbsVahter/ontoTRPG/main/crown_and_skull/crown_and_skull.ttl#Limitation
:Limitation rdf:type owl:Class ;
            rdfs:subClassOf gen:Act ;
            rdfs:label "Limitation"@en .


###  https://raw.githubusercontent.com/AbsVahter/ontoTRPG/main/crown_and_skull/crown_and_skull.ttl#LimitationCompanion
:LimitationCompanion rdf:type owl:Class ;
                     rdfs:subClassOf :Limitation .


###  https://raw.githubusercontent.com/AbsVahter/ontoTRPG/main/crown_and_skull/crown_and_skull.ttl#LimitationItem
:LimitationItem rdf:type owl:Class ;
                rdfs:subClassOf :Limitation .


###  https://raw.githubusercontent.com/AbsVahter/ontoTRPG/main/crown_and_skull/crown_and_skull.ttl#LimitationSpell
:LimitationSpell rdf:type owl:Class ;
                 rdfs:subClassOf :Limitation .


###  https://raw.githubusercontent.com/AbsVahter/ontoTRPG/main/crown_and_skull/crown_and_skull.ttl#Lineage
:Lineage rdf:type owl:Class .


###  https://raw.githubusercontent.com/AbsVahter/ontoTRPG/main/crown_and_skull/crown_and_skull.ttl#MagicAdvancement
:MagicAdvancement rdf:type owl:Class ;
                  rdfs:subClassOf :Ability .


###  https://raw.githubusercontent.com/AbsVahter/ontoTRPG/main/crown_and_skull/crown_and_skull.ttl#MagicAdvancementAncientOne
:MagicAdvancementAncientOne rdf:type owl:Class ;
                            rdfs:subClassOf :MagicAdvancement ,
                                            [ rdf:type owl:Restriction ;
                                              owl:onProperty gen:prerequisite ;
                                              owl:hasValue :wizard_ancient_one
                                            ] ;
                            rdfs:label "Ancient One magic advancement"@en .


###  https://raw.githubusercontent.com/AbsVahter/ontoTRPG/main/crown_and_skull/crown_and_skull.ttl#MagicAdvancementAncientOneTier1
:MagicAdvancementAncientOneTier1 rdf:type owl:Class ;
                                 rdfs:subClassOf :MagicAdvancementAncientOne ,
                                                 [ rdf:type owl:Restriction ;
                                                   owl:onProperty :tier ;
                                                   owl:hasValue 1
                                                 ] ,
                                                 [ rdf:type owl:Restriction ;
                                                   owl:onProperty gen:cost ;
                                                   owl:hasValue "3 hero points"
                                                 ] ;
                                 rdfs:label "Ancient One magic advancement: tier 1"@en .


###  https://raw.githubusercontent.com/AbsVahter/ontoTRPG/main/crown_and_skull/crown_and_skull.ttl#MagicAdvancementAncientOneTier2
:MagicAdvancementAncientOneTier2 rdf:type owl:Class ;
                                 rdfs:subClassOf :MagicAdvancementAncientOne ,
                                                 [ rdf:type owl:Restriction ;
                                                   owl:onProperty :tier ;
                                                   owl:hasValue 2
                                                 ] ,
                                                 [ rdf:type owl:Restriction ;
                                                   owl:onProperty gen:cost ;
                                                   owl:hasValue "6 hero points"
                                                 ] ;
                                 rdfs:label "Ancient One magic advancement: tier 2"@en .


###  https://raw.githubusercontent.com/AbsVahter/ontoTRPG/main/crown_and_skull/crown_and_skull.ttl#MagicAdvancementAncientOneTier3
:MagicAdvancementAncientOneTier3 rdf:type owl:Class ;
                                 rdfs:subClassOf :MagicAdvancementAncientOne ,
                                                 [ rdf:type owl:Restriction ;
                                                   owl:onProperty :tier ;
                                                   owl:hasValue 3
                                                 ] ,
                                                 [ rdf:type owl:Restriction ;
                                                   owl:onProperty gen:cost ;
                                                   owl:hasValue "12 hero points"
                                                 ] ;
                                 rdfs:label "Ancient One magic advancement: tier 3"@en .


###  https://raw.githubusercontent.com/AbsVahter/ontoTRPG/main/crown_and_skull/crown_and_skull.ttl#MagicAdvancementAncientOneTier4
:MagicAdvancementAncientOneTier4 rdf:type owl:Class ;
                                 rdfs:subClassOf :MagicAdvancementAncientOne ,
                                                 [ rdf:type owl:Restriction ;
                                                   owl:onProperty :tier ;
                                                   owl:hasValue 4
                                                 ] ,
                                                 [ rdf:type owl:Restriction ;
                                                   owl:onProperty gen:cost ;
                                                   owl:hasValue "15 hero points"
                                                 ] ;
                                 rdfs:label "Ancient One magic advancement: tier 4"@en .


###  https://raw.githubusercontent.com/AbsVahter/ontoTRPG/main/crown_and_skull/crown_and_skull.ttl#MagicAdvancementDemonologist
:MagicAdvancementDemonologist rdf:type owl:Class ;
                              rdfs:subClassOf :MagicAdvancement ,
                                              [ rdf:type owl:Restriction ;
                                                owl:onProperty gen:prerequisite ;
                                                owl:hasValue :wizard_demonologist
                                              ] ;
                              rdfs:label "Demonologist magic advancement"@en .


###  https://raw.githubusercontent.com/AbsVahter/ontoTRPG/main/crown_and_skull/crown_and_skull.ttl#MagicAdvancementDemonologistTier1
:MagicAdvancementDemonologistTier1 rdf:type owl:Class ;
                                   rdfs:subClassOf :MagicAdvancementDemonologist ,
                                                   [ rdf:type owl:Restriction ;
                                                     owl:onProperty :tier ;
                                                     owl:hasValue 1
                                                   ] ,
                                                   [ rdf:type owl:Restriction ;
                                                     owl:onProperty gen:cost ;
                                                     owl:hasValue "3 hero points"
                                                   ] ;
                                   rdfs:label "Demonologist magic advancement: tier 1"@en .


###  https://raw.githubusercontent.com/AbsVahter/ontoTRPG/main/crown_and_skull/crown_and_skull.ttl#MagicAdvancementDemonologistTier2
:MagicAdvancementDemonologistTier2 rdf:type owl:Class ;
                                   rdfs:subClassOf :MagicAdvancementDemonologist ,
                                                   [ rdf:type owl:Restriction ;
                                                     owl:onProperty :tier ;
                                                     owl:hasValue 2
                                                   ] ,
                                                   [ rdf:type owl:Restriction ;
                                                     owl:onProperty gen:cost ;
                                                     owl:hasValue "6 hero points"
                                                   ] ;
                                   rdfs:label "Demonologist magic advancement: tier 2"@en .


###  https://raw.githubusercontent.com/AbsVahter/ontoTRPG/main/crown_and_skull/crown_and_skull.ttl#MagicAdvancementDemonologistTier3
:MagicAdvancementDemonologistTier3 rdf:type owl:Class ;
                                   rdfs:subClassOf :MagicAdvancementDemonologist ,
                                                   [ rdf:type owl:Restriction ;
                                                     owl:onProperty :tier ;
                                                     owl:hasValue 3
                                                   ] ,
                                                   [ rdf:type owl:Restriction ;
                                                     owl:onProperty gen:cost ;
                                                     owl:hasValue "12 hero points"
                                                   ] ;
                                   rdfs:label "Demonologist magic advancement: tier 3"@en .


###  https://raw.githubusercontent.com/AbsVahter/ontoTRPG/main/crown_and_skull/crown_and_skull.ttl#MagicAdvancementDemonologistTier4
:MagicAdvancementDemonologistTier4 rdf:type owl:Class ;
                                   rdfs:subClassOf :MagicAdvancementDemonologist ,
                                                   [ rdf:type owl:Restriction ;
                                                     owl:onProperty :tier ;
                                                     owl:hasValue 4
                                                   ] ,
                                                   [ rdf:type owl:Restriction ;
                                                     owl:onProperty gen:cost ;
                                                     owl:hasValue "15 hero points"
                                                   ] ;
                                   rdfs:label "Demonologist magic advancement: tier 4"@en .


###  https://raw.githubusercontent.com/AbsVahter/ontoTRPG/main/crown_and_skull/crown_and_skull.ttl#MagicAdvancementHolySymbol
:MagicAdvancementHolySymbol rdf:type owl:Class ;
                            rdfs:subClassOf :MagicAdvancement .


###  https://raw.githubusercontent.com/AbsVahter/ontoTRPG/main/crown_and_skull/crown_and_skull.ttl#MagicAdvancementStarfallen
:MagicAdvancementStarfallen rdf:type owl:Class ;
                            rdfs:subClassOf :MagicAdvancement ,
                                            [ rdf:type owl:Restriction ;
                                              owl:onProperty gen:prerequisite ;
                                              owl:hasValue :wizard_starfallen
                                            ] ;
                            rdfs:label "Starfallen magic advancement"@en .


###  https://raw.githubusercontent.com/AbsVahter/ontoTRPG/main/crown_and_skull/crown_and_skull.ttl#MagicAdvancementStarfallenTier1
:MagicAdvancementStarfallenTier1 rdf:type owl:Class ;
                                 rdfs:subClassOf :MagicAdvancementStarfallen ,
                                                 [ rdf:type owl:Restriction ;
                                                   owl:onProperty :tier ;
                                                   owl:hasValue 1
                                                 ] ,
                                                 [ rdf:type owl:Restriction ;
                                                   owl:onProperty gen:cost ;
                                                   owl:hasValue "3 hero points"
                                                 ] ;
                                 rdfs:label "Starfallen magic advancement: tier 1"@en .


###  https://raw.githubusercontent.com/AbsVahter/ontoTRPG/main/crown_and_skull/crown_and_skull.ttl#MagicAdvancementStarfallenTier2
:MagicAdvancementStarfallenTier2 rdf:type owl:Class ;
                                 rdfs:subClassOf :MagicAdvancementStarfallen ,
                                                 [ rdf:type owl:Restriction ;
                                                   owl:onProperty :tier ;
                                                   owl:hasValue 2
                                                 ] ,
                                                 [ rdf:type owl:Restriction ;
                                                   owl:onProperty gen:cost ;
                                                   owl:hasValue "6 hero points"
                                                 ] ;
                                 rdfs:label "Starfallen magic advancement: tier 2"@en .


###  https://raw.githubusercontent.com/AbsVahter/ontoTRPG/main/crown_and_skull/crown_and_skull.ttl#MagicAdvancementStarfallenTier3
:MagicAdvancementStarfallenTier3 rdf:type owl:Class ;
                                 rdfs:subClassOf :MagicAdvancementStarfallen ,
                                                 [ rdf:type owl:Restriction ;
                                                   owl:onProperty :tier ;
                                                   owl:hasValue 3
                                                 ] ,
                                                 [ rdf:type owl:Restriction ;
                                                   owl:onProperty gen:cost ;
                                                   owl:hasValue "12 hero points"
                                                 ] ;
                                 rdfs:label "Starfallen magic advancement: tier 3"@en .


###  https://raw.githubusercontent.com/AbsVahter/ontoTRPG/main/crown_and_skull/crown_and_skull.ttl#MagicAdvancementStarfallenTier4
:MagicAdvancementStarfallenTier4 rdf:type owl:Class ;
                                 rdfs:subClassOf :MagicAdvancementStarfallen ,
                                                 [ rdf:type owl:Restriction ;
                                                   owl:onProperty :tier ;
                                                   owl:hasValue 4
                                                 ] ,
                                                 [ rdf:type owl:Restriction ;
                                                   owl:onProperty gen:cost ;
                                                   owl:hasValue "15 hero points"
                                                 ] ;
                                 rdfs:label "Starfallen magic advancement: tier 4"@en .


###  https://raw.githubusercontent.com/AbsVahter/ontoTRPG/main/crown_and_skull/crown_and_skull.ttl#RequiredDetails
:RequiredDetails rdf:type owl:Class ;
                 rdfs:label "Required details"@en .


###  https://raw.githubusercontent.com/AbsVahter/ontoTRPG/main/crown_and_skull/crown_and_skull.ttl#SetAdditiveEquipment
:SetAdditiveEquipment rdf:type owl:Class ;
                      owl:equivalentClass [ rdf:type owl:Restriction ;
                                            owl:onProperty gen:setAdditive ;
                                            owl:hasValue :equipment
                                          ] ;
                      rdfs:subClassOf gen:Act ,
                                      [ rdf:type owl:Restriction ;
                                        owl:onProperty gen:prerequisiteDescription ;
                                        owl:hasValue "final number of equipment <= 10"
                                      ] .


###  https://raw.githubusercontent.com/AbsVahter/ontoTRPG/main/crown_and_skull/crown_and_skull.ttl#SetAdditiveSkill
:SetAdditiveSkill rdf:type owl:Class ;
                  owl:equivalentClass [ rdf:type owl:Restriction ;
                                        owl:onProperty gen:setAdditive ;
                                        owl:hasValue :skills
                                      ] ;
                  rdfs:subClassOf gen:Act ,
                                  [ rdf:type owl:Restriction ;
                                    owl:onProperty gen:prerequisiteDescription ;
                                    owl:hasValue "(final number of skills <= 10) and (final skill level >= 3) and (final skill level <= 18)"
                                  ] .


###  https://raw.githubusercontent.com/AbsVahter/ontoTRPG/main/crown_and_skull/crown_and_skull.ttl#Skill
:Skill rdf:type owl:Class ;
       rdfs:subClassOf :RequiredDetails ,
                       gen:ParameterPC .


###  https://raw.githubusercontent.com/AbsVahter/ontoTRPG/main/crown_and_skull/crown_and_skull.ttl#SkillAntimagic
:SkillAntimagic rdf:type owl:Class ;
                rdfs:subClassOf :Skill .


###  https://raw.githubusercontent.com/AbsVahter/ontoTRPG/main/crown_and_skull/crown_and_skull.ttl#SkillBasic
:SkillBasic rdf:type owl:Class ;
            rdfs:subClassOf :Skill .


###  https://raw.githubusercontent.com/AbsVahter/ontoTRPG/main/crown_and_skull/crown_and_skull.ttl#SkillCompanion
:SkillCompanion rdf:type owl:Class ;
                rdfs:subClassOf :Skill .


###  https://raw.githubusercontent.com/AbsVahter/ontoTRPG/main/crown_and_skull/crown_and_skull.ttl#SkillCrown
:SkillCrown rdf:type owl:Class ;
            rdfs:subClassOf :Skill .


###  https://raw.githubusercontent.com/AbsVahter/ontoTRPG/main/crown_and_skull/crown_and_skull.ttl#SkillSkull
:SkillSkull rdf:type owl:Class ;
            rdfs:subClassOf :Skill .


###  https://raw.githubusercontent.com/AbsVahter/ontoTRPG/main/crown_and_skull/crown_and_skull.ttl#Spell
:Spell rdf:type owl:Class .


###  https://raw.githubusercontent.com/AbsVahter/ontoTRPG/main/crown_and_skull/crown_and_skull.ttl#SpellConsequenceInfernal
:SpellConsequenceInfernal rdf:type owl:Class ;
                          rdfs:subClassOf gen:Act .


###  https://raw.githubusercontent.com/AbsVahter/ontoTRPG/main/crown_and_skull/crown_and_skull.ttl#SpellConsequenceUnstable
:SpellConsequenceUnstable rdf:type owl:Class ;
                          rdfs:subClassOf gen:Act .


###  https://raw.githubusercontent.com/AbsVahter/ontoTRPG/main/crown_and_skull/crown_and_skull.ttl#Wizard
:Wizard rdf:type owl:Class .


###  https://raw.githubusercontent.com/AbsVahter/ontoTRPG/main/ontoGeneral.ttl#Check
gen:Check rdfs:subClassOf [ rdf:type owl:Restriction ;
                            owl:onProperty gen:Actor ;
                            owl:hasValue gen:player
                          ] ,
                          [ rdf:type owl:Restriction ;
                            owl:onProperty gen:valueFormula ;
                            owl:hasValue """
{
    d20 = 1: critical success ;
    d20 <= threshold: success ;
    d20 > threshold: failure ;
    d20 = 20: critical failure ;
}
"""
                          ] .


###  https://raw.githubusercontent.com/AbsVahter/ontoTRPG/main/ontoGeneral.ttl#Community
gen:Community rdfs:subClassOf :RequiredDetails .


###  https://raw.githubusercontent.com/AbsVahter/ontoTRPG/main/ontoGeneral.ttl#Creature
gen:Creature rdfs:subClassOf :RequiredDetails .


###  https://raw.githubusercontent.com/AbsVahter/ontoTRPG/main/ontoGeneral.ttl#TemplatePC
gen:TemplatePC rdf:type owl:Class ;
               rdfs:subClassOf :RequiredDetails ,
                               gen:Creature .


#################################################################
#    Individuals
#################################################################

###  https://raw.githubusercontent.com/AbsVahter/ontoTRPG/main/crown_and_skull/crown_and_skull.ttl#Ability
:Ability rdf:type owl:NamedIndividual .


###  https://raw.githubusercontent.com/AbsVahter/ontoTRPG/main/crown_and_skull/crown_and_skull.ttl#Attrition
:Attrition rdf:type owl:NamedIndividual .


###  https://raw.githubusercontent.com/AbsVahter/ontoTRPG/main/crown_and_skull/crown_and_skull.ttl#Companion
:Companion rdf:type owl:NamedIndividual .


###  https://raw.githubusercontent.com/AbsVahter/ontoTRPG/main/crown_and_skull/crown_and_skull.ttl#CoreAbility
:CoreAbility rdf:type owl:NamedIndividual .


###  https://raw.githubusercontent.com/AbsVahter/ontoTRPG/main/crown_and_skull/crown_and_skull.ttl#EffectCompanion
:EffectCompanion rdf:type owl:NamedIndividual .


###  https://raw.githubusercontent.com/AbsVahter/ontoTRPG/main/crown_and_skull/crown_and_skull.ttl#EffectItem
:EffectItem rdf:type owl:NamedIndividual .


###  https://raw.githubusercontent.com/AbsVahter/ontoTRPG/main/crown_and_skull/crown_and_skull.ttl#EffectSpell
:EffectSpell rdf:type owl:NamedIndividual .


###  https://raw.githubusercontent.com/AbsVahter/ontoTRPG/main/crown_and_skull/crown_and_skull.ttl#FlawBasic
:FlawBasic rdf:type owl:NamedIndividual .


###  https://raw.githubusercontent.com/AbsVahter/ontoTRPG/main/crown_and_skull/crown_and_skull.ttl#Item
:Item rdf:type owl:NamedIndividual .


###  https://raw.githubusercontent.com/AbsVahter/ontoTRPG/main/crown_and_skull/crown_and_skull.ttl#ItemArmor
:ItemArmor rdf:type owl:NamedIndividual .


###  https://raw.githubusercontent.com/AbsVahter/ontoTRPG/main/crown_and_skull/crown_and_skull.ttl#ItemBasic
:ItemBasic rdf:type owl:NamedIndividual .


###  https://raw.githubusercontent.com/AbsVahter/ontoTRPG/main/crown_and_skull/crown_and_skull.ttl#ItemCrown
:ItemCrown rdf:type owl:NamedIndividual .


###  https://raw.githubusercontent.com/AbsVahter/ontoTRPG/main/crown_and_skull/crown_and_skull.ttl#ItemSkull
:ItemSkull rdf:type owl:NamedIndividual .


###  https://raw.githubusercontent.com/AbsVahter/ontoTRPG/main/crown_and_skull/crown_and_skull.ttl#ItemWeapon
:ItemWeapon rdf:type owl:NamedIndividual .


###  https://raw.githubusercontent.com/AbsVahter/ontoTRPG/main/crown_and_skull/crown_and_skull.ttl#LimitationCompanion
:LimitationCompanion rdf:type owl:NamedIndividual .


###  https://raw.githubusercontent.com/AbsVahter/ontoTRPG/main/crown_and_skull/crown_and_skull.ttl#LimitationItem
:LimitationItem rdf:type owl:NamedIndividual .


###  https://raw.githubusercontent.com/AbsVahter/ontoTRPG/main/crown_and_skull/crown_and_skull.ttl#LimitationSpell
:LimitationSpell rdf:type owl:NamedIndividual .


###  https://raw.githubusercontent.com/AbsVahter/ontoTRPG/main/crown_and_skull/crown_and_skull.ttl#Lineage
:Lineage rdf:type owl:NamedIndividual .


###  https://raw.githubusercontent.com/AbsVahter/ontoTRPG/main/crown_and_skull/crown_and_skull.ttl#MagicAdvancement
:MagicAdvancement rdf:type owl:NamedIndividual .


###  https://raw.githubusercontent.com/AbsVahter/ontoTRPG/main/crown_and_skull/crown_and_skull.ttl#MagicAdvancementHolySymbol
:MagicAdvancementHolySymbol rdf:type owl:NamedIndividual .


###  https://raw.githubusercontent.com/AbsVahter/ontoTRPG/main/crown_and_skull/crown_and_skull.ttl#SetAdditiveEquipment
:SetAdditiveEquipment rdf:type owl:NamedIndividual .


###  https://raw.githubusercontent.com/AbsVahter/ontoTRPG/main/crown_and_skull/crown_and_skull.ttl#SetAdditiveSkill
:SetAdditiveSkill rdf:type owl:NamedIndividual .


###  https://raw.githubusercontent.com/AbsVahter/ontoTRPG/main/crown_and_skull/crown_and_skull.ttl#Skill
:Skill rdf:type owl:NamedIndividual .


###  https://raw.githubusercontent.com/AbsVahter/ontoTRPG/main/crown_and_skull/crown_and_skull.ttl#SkillAntimagic
:SkillAntimagic rdf:type owl:NamedIndividual .


###  https://raw.githubusercontent.com/AbsVahter/ontoTRPG/main/crown_and_skull/crown_and_skull.ttl#SkillBasic
:SkillBasic rdf:type owl:NamedIndividual .


###  https://raw.githubusercontent.com/AbsVahter/ontoTRPG/main/crown_and_skull/crown_and_skull.ttl#SkillCompanion
:SkillCompanion rdf:type owl:NamedIndividual .


###  https://raw.githubusercontent.com/AbsVahter/ontoTRPG/main/crown_and_skull/crown_and_skull.ttl#SkillCrown
:SkillCrown rdf:type owl:NamedIndividual .


###  https://raw.githubusercontent.com/AbsVahter/ontoTRPG/main/crown_and_skull/crown_and_skull.ttl#SkillSkull
:SkillSkull rdf:type owl:NamedIndividual .


###  https://raw.githubusercontent.com/AbsVahter/ontoTRPG/main/crown_and_skull/crown_and_skull.ttl#Spell
:Spell rdf:type owl:NamedIndividual .


###  https://raw.githubusercontent.com/AbsVahter/ontoTRPG/main/crown_and_skull/crown_and_skull.ttl#SpellConsequenceInfernal
:SpellConsequenceInfernal rdf:type owl:NamedIndividual .


###  https://raw.githubusercontent.com/AbsVahter/ontoTRPG/main/crown_and_skull/crown_and_skull.ttl#SpellConsequenceUnstable
:SpellConsequenceUnstable rdf:type owl:NamedIndividual .


###  https://raw.githubusercontent.com/AbsVahter/ontoTRPG/main/crown_and_skull/crown_and_skull.ttl#Wizard
:Wizard rdf:type owl:NamedIndividual .


###  https://raw.githubusercontent.com/AbsVahter/ontoTRPG/main/crown_and_skull/crown_and_skull.ttl#alderman_wallaby
:alderman_wallaby rdf:type owl:NamedIndividual ,
                           gen:Creature ;
                  rdfs:comment "He is a proudfoot scholar, almost two centuries old, and a lover of festivals. He relies on good counsel from many townsfolk. Local envoys and lords are widely known to adore the old fellow, coming from far and wide to offer gifts on his birthday."@en ;
                  rdfs:label "Alderman Wallabytarnwhatwallaby"@en .


###  https://raw.githubusercontent.com/AbsVahter/ontoTRPG/main/crown_and_skull/crown_and_skull.ttl#attack_of_enemy
:attack_of_enemy rdf:type owl:NamedIndividual ;
                 rdfs:label "Attack of enemy"@en ;
                 gen:Actor gen:master ;
                 gen:effect :check_defense ;
                 gen:prerequisiteDescription "enemy creature" ;
                 gen:set :defense_penalty ;
                 gen:target "PC" ;
                 gen:valueObject :stat_atk .


###  https://raw.githubusercontent.com/AbsVahter/ontoTRPG/main/crown_and_skull/crown_and_skull.ttl#attrition_basic
:attrition_basic rdf:type owl:NamedIndividual ,
                          :Attrition ;
                 rdfs:comment "cross off any 1 equipment or skill"@en ;
                 rdfs:label "Basic attrition"@en ;
                 gen:modified :equipment ,
                              :skills ;
                 gen:valueFormula "(1 equipment non-crossed -> crossed) or (1 skill non-crossed -> crossed)" .


###  https://raw.githubusercontent.com/AbsVahter/ontoTRPG/main/crown_and_skull/crown_and_skull.ttl#attrition_brutal
:attrition_brutal rdf:type owl:NamedIndividual ,
                           :Attrition ;
                  rdfs:comment "cross off random 1d6 equipment and skill"@en ;
                  rdfs:label "Brutal attrition"@en ;
                  gen:effect :set_status_stun_by_brutal_attrition ;
                  gen:modified :equipment ,
                               :skills ;
                  gen:valueFormula "random 1d6 equipment and skill non-crossed -> crossed" .


###  https://raw.githubusercontent.com/AbsVahter/ontoTRPG/main/crown_and_skull/crown_and_skull.ttl#attrition_destroy
:attrition_destroy rdf:type owl:NamedIndividual ,
                            :Attrition ;
                   rdfs:comment "destroy 1 random equipment and cross off 1 random skill"@en ;
                   rdfs:label "Destroy attrition"@en ;
                   gen:modified :skills ;
                   gen:setAdditive :equipment ;
                   gen:valueFormula "(equipment -= 1 random item) and (1 random skill non-crossed -> crossed)" .


###  https://raw.githubusercontent.com/AbsVahter/ontoTRPG/main/crown_and_skull/crown_and_skull.ttl#attrition_equipment
:attrition_equipment rdf:type owl:NamedIndividual ,
                              :Attrition ;
                     rdfs:comment "cross off random 1 equipment"@en ;
                     rdfs:label "Equipment attrition"@en ;
                     gen:modified :equipment ;
                     gen:valueFormula "1 random equipment non-crossed -> crossed" .


###  https://raw.githubusercontent.com/AbsVahter/ontoTRPG/main/crown_and_skull/crown_and_skull.ttl#attrition_flesh
:attrition_flesh rdf:type owl:NamedIndividual ,
                          :Attrition ;
                 rdfs:comment "cross off random 1 skill" ;
                 rdfs:label "Flesh attrition"@en ;
                 gen:modified :skills ;
                 gen:valueFormula "1 random skill non-crossed -> crossed" .


###  https://raw.githubusercontent.com/AbsVahter/ontoTRPG/main/crown_and_skull/crown_and_skull.ttl#bee_spoke
:bee_spoke rdf:type owl:NamedIndividual ;
           rdfs:comment "The oldest tavern in town was recently damaged by a collapse and fire during an orc incursion. Its owner, Bespo Kerat, was killed in the blaze. Now his daughter Revelle has disappeared. The calamity of the Bee Spoke has rallied folk to fight back against the orcs, no matter what the cost. So, reconstruction has begun."@en ;
           rdfs:label "The Bee Spoke"@en .


###  https://raw.githubusercontent.com/AbsVahter/ontoTRPG/main/crown_and_skull/crown_and_skull.ttl#block_status_bleed
:block_status_bleed rdf:type owl:NamedIndividual ;
                    rdfs:label "Block bleed"@en ;
                    gen:blocked :status_bleed .


###  https://raw.githubusercontent.com/AbsVahter/ontoTRPG/main/crown_and_skull/crown_and_skull.ttl#block_status_immobilized_by_magic
:block_status_immobilized_by_magic rdf:type owl:NamedIndividual ;
                                   rdfs:label "Escape from immobilized condition by magic"@en ;
                                   gen:blocked :status_immobilized_by_magic .


###  https://raw.githubusercontent.com/AbsVahter/ontoTRPG/main/crown_and_skull/crown_and_skull.ttl#block_status_immobilized_by_material_forces
:block_status_immobilized_by_material_forces rdf:type owl:NamedIndividual ;
                                             rdfs:label "Escape from immobilized condition by material forces"@en ;
                                             gen:blocked :status_immobilized_by_material_forces .


###  https://raw.githubusercontent.com/AbsVahter/ontoTRPG/main/crown_and_skull/crown_and_skull.ttl#block_status_stun
:block_status_stun rdf:type owl:NamedIndividual ;
                   rdfs:label "Block stun"@en ;
                   gen:blocked :status_stun .


###  https://raw.githubusercontent.com/AbsVahter/ontoTRPG/main/crown_and_skull/crown_and_skull.ttl#bloodwing
:bloodwing rdf:type owl:NamedIndividual ,
                    gen:Creature ;
           rdfs:comment "Bloodwing was a colossal green dragon, driven mad by a slime-entity called The Corruption."@en ;
           rdfs:label "Bloodwing"@en .


###  https://raw.githubusercontent.com/AbsVahter/ontoTRPG/main/crown_and_skull/crown_and_skull.ttl#bloodwing_war
:bloodwing_war rdf:type owl:NamedIndividual ,
                        gen:Event ;
               rdfs:comment "Some 30 years before present day, The Bloodwing War ravaged the realm. The once-unifi ed lands no longer have a king, borders have decayed, wilds are more dangerous than ever. An age of order and ideas has come to an end. With no unifying rule, The North Holds struggle to fi nd new purpose and new direction. An era of adventure."@en ;
               rdfs:label "The Bloodwing War"@en ;
               gen:Actor :bloodwing ;
               gen:Location :north_holds ;
               gen:motive gen:madness .


###  https://raw.githubusercontent.com/AbsVahter/ontoTRPG/main/crown_and_skull/crown_and_skull.ttl#character_creation
:character_creation rdf:type owl:NamedIndividual ;
                    rdfs:label "Character creation"@en ;
                    gen:Actor gen:player ;
                    gen:after :set_hometown ;
                    gen:inputOption :character_creation_custom ,
                                    :character_creation_discovery ,
                                    :character_creation_templates_and_prompts ;
                    gen:set gen:pc .


###  https://raw.githubusercontent.com/AbsVahter/ontoTRPG/main/crown_and_skull/crown_and_skull.ttl#character_creation_companion
:character_creation_companion rdf:type owl:NamedIndividual ;
                              rdfs:label "Custom character creation: acquire and customize a companion"@en ;
                              gen:after :character_creation_spell ;
                              gen:cost "companion cost" ;
                              gen:input :companion_custom ;
                              gen:resource :hero_points ;
                              gen:set :companions .


###  https://raw.githubusercontent.com/AbsVahter/ontoTRPG/main/crown_and_skull/crown_and_skull.ttl#character_creation_core_ability
:character_creation_core_ability rdf:type owl:NamedIndividual ;
                                 rdfs:label "Custom character creation: core ability"@en ;
                                 gen:after :character_creation_flaws ;
                                 gen:cost "15" ;
                                 gen:inputOption :CoreAbility ;
                                 gen:prerequisiteDescription "number of core abilities < 2" ;
                                 gen:resource :hero_points ;
                                 gen:set :core_ability .


###  https://raw.githubusercontent.com/AbsVahter/ontoTRPG/main/crown_and_skull/crown_and_skull.ttl#character_creation_custom
:character_creation_custom rdf:type owl:NamedIndividual ;
                           rdfs:label "Custom character creation"@en ;
                           gen:Actor gen:player ;
                           gen:included :character_creation_custom_hero_points_distribution ,
                                        :character_creation_lineage ;
                           gen:set gen:pc .


###  https://raw.githubusercontent.com/AbsVahter/ontoTRPG/main/crown_and_skull/crown_and_skull.ttl#character_creation_custom_hero_points_distribution
:character_creation_custom_hero_points_distribution rdf:type owl:NamedIndividual ;
                                                    rdfs:label "Custom character creation by distribution of hero points"@en ;
                                                    gen:included :character_creation_companion ,
                                                                 :character_creation_core_ability ,
                                                                 :character_creation_equipment ,
                                                                 :character_creation_flaws ,
                                                                 :character_creation_skill ,
                                                                 :character_creation_spell ,
                                                                 :character_creation_starting_points .


###  https://raw.githubusercontent.com/AbsVahter/ontoTRPG/main/crown_and_skull/crown_and_skull.ttl#character_creation_discovery
:character_creation_discovery rdf:type owl:NamedIndividual ;
                              rdfs:label "Character creation by discovery"@en ;
                              gen:Actor gen:party ;
                              gen:included :character_creation_discovery_finding_gear ,
                                           :character_creation_discovery_finding_memories ,
                                           :character_creation_discovery_finding_past ,
                                           :character_creation_discovery_one_little_memory ,
                                           :character_creation_discovery_opener ,
                                           :character_creation_discovery_origin_revealed ,
                                           :character_creation_discovery_remember_name ;
                              gen:set gen:pc .


###  https://raw.githubusercontent.com/AbsVahter/ontoTRPG/main/crown_and_skull/crown_and_skull.ttl#character_creation_discovery_finding_gear
:character_creation_discovery_finding_gear rdf:type owl:NamedIndividual ;
                                           rdfs:label "Character creation by discovery: finding gear"@en ;
                                           gen:after :character_creation_discovery_remember_name ;
                                           gen:prerequisiteDescription "in session 1" ;
                                           gen:setAdditive :equipment ;
                                           gen:valueFormula "1-3 useful items per PC" .


###  https://raw.githubusercontent.com/AbsVahter/ontoTRPG/main/crown_and_skull/crown_and_skull.ttl#character_creation_discovery_finding_memories
:character_creation_discovery_finding_memories rdf:type owl:NamedIndividual ;
                                               rdfs:comment "This could be an increase to a skill, a new skill, a piece of character background, or even a flaw."@en ;
                                               rdfs:label "Character creation by discovery: finding memories"@en ;
                                               gen:after :character_creation_discovery_remember_name ;
                                               gen:prerequisiteDescription "in session 1" ;
                                               gen:valueFormula "3-5 memories per PC" .


###  https://raw.githubusercontent.com/AbsVahter/ontoTRPG/main/crown_and_skull/crown_and_skull.ttl#character_creation_discovery_finding_past
:character_creation_discovery_finding_past rdf:type owl:NamedIndividual ;
                                           rdfs:comment "All PC are encouraged to seek their history."@en ;
                                           rdfs:label "Character creation by discovery: finding your past"@en ;
                                           gen:after :character_creation_discovery_finding_gear ,
                                                     :character_creation_discovery_finding_memories .


###  https://raw.githubusercontent.com/AbsVahter/ontoTRPG/main/crown_and_skull/crown_and_skull.ttl#character_creation_discovery_one_little_memory
:character_creation_discovery_one_little_memory rdf:type owl:NamedIndividual ;
                                                rdfs:comment "As heroes seek to escape or get moving, a fleeting shadow, reflection, or strange feeling triggers one small memory for each character."@en ;
                                                rdfs:label "Character creation by discovery: one little memory"@en ;
                                                gen:after :character_creation_discovery_opener ;
                                                gen:inputOption :SkillBasic ;
                                                gen:valueNumeric 6 ;
                                                gen:gen:setAdditive :skills .


###  https://raw.githubusercontent.com/AbsVahter/ontoTRPG/main/crown_and_skull/crown_and_skull.ttl#character_creation_discovery_opener
:character_creation_discovery_opener rdf:type owl:NamedIndividual ;
                                     rdfs:label "Character creation by discovery: the opener"@en ;
                                     gen:Actor gen:party ;
                                     gen:set gen:pc ;
                                     gen:valueFormula "(hero points = 0) and location and condition and time pressure" .


###  https://raw.githubusercontent.com/AbsVahter/ontoTRPG/main/crown_and_skull/crown_and_skull.ttl#character_creation_discovery_origin_revealed
:character_creation_discovery_origin_revealed rdf:type owl:NamedIndividual ;
                                              rdfs:comment "Memory of how you got into all this"@en ;
                                              rdfs:label "Character creation by discovery: origin revealed"@en ;
                                              gen:after :character_creation_discovery_finding_past ;
                                              gen:included :character_creation_discovery_origin_revealed_core_ability ,
                                                           :character_creation_discovery_origin_revealed_equipment ,
                                                           :character_creation_discovery_origin_revealed_skills ;
                                              gen:prerequisiteDescription "a character reaches a moment of truly epic success, poignant role play, or powerful luck" .


###  https://raw.githubusercontent.com/AbsVahter/ontoTRPG/main/crown_and_skull/crown_and_skull.ttl#character_creation_discovery_origin_revealed_core_ability
:character_creation_discovery_origin_revealed_core_ability rdf:type owl:NamedIndividual ;
                                                           rdfs:label "Character creation by discovery: origin revealed with gaining core ability"@en ;
                                                           gen:set :core_ability .


###  https://raw.githubusercontent.com/AbsVahter/ontoTRPG/main/crown_and_skull/crown_and_skull.ttl#character_creation_discovery_origin_revealed_equipment
:character_creation_discovery_origin_revealed_equipment rdf:type owl:NamedIndividual ;
                                                        rdfs:label "Character creation by discovery: origin revealed with gaining equipment"@en ;
                                                        gen:setAdditive :equipment ;
                                                        gen:valueFormula "10 points" .


###  https://raw.githubusercontent.com/AbsVahter/ontoTRPG/main/crown_and_skull/crown_and_skull.ttl#character_creation_discovery_origin_revealed_skills
:character_creation_discovery_origin_revealed_skills rdf:type owl:NamedIndividual ;
                                                     rdfs:label "Character creation by discovery: origin revealed with gaining skills"@en ;
                                                     gen:setAdditive :skills ;
                                                     gen:valueFormula "2 skills with 9 level" .


###  https://raw.githubusercontent.com/AbsVahter/ontoTRPG/main/crown_and_skull/crown_and_skull.ttl#character_creation_discovery_remember_name
:character_creation_discovery_remember_name rdf:type owl:NamedIndividual ;
                                            rdfs:label "Character creation by discovery: I remember my name"@en ;
                                            gen:after :character_creation_discovery_one_little_memory .


###  https://raw.githubusercontent.com/AbsVahter/ontoTRPG/main/crown_and_skull/crown_and_skull.ttl#character_creation_equipment
:character_creation_equipment rdf:type owl:NamedIndividual ;
                              rdfs:label "Custom character creation: buy and customize equipment"@en ;
                              gen:after :character_creation_skill ;
                              gen:cost "cost of item" ;
                              gen:input :item_custom ;
                              gen:resource :hero_points ;
                              gen:setAdditive :equipment .


###  https://raw.githubusercontent.com/AbsVahter/ontoTRPG/main/crown_and_skull/crown_and_skull.ttl#character_creation_flaws
:character_creation_flaws rdf:type owl:NamedIndividual ;
                          rdfs:comment "What is a weakness or stress point for character? Flaws imply history and drive believable role play."@en ;
                          rdfs:label "Custom character creation: flaws"@en ;
                          gen:after :character_creation_starting_points ;
                          gen:included :character_creation_flaws_additional_points ,
                                       :character_creation_flaws_selection .


###  https://raw.githubusercontent.com/AbsVahter/ontoTRPG/main/crown_and_skull/crown_and_skull.ttl#character_creation_flaws_additional_points
:character_creation_flaws_additional_points rdf:type owl:NamedIndividual ;
                                            rdfs:label "Custom character creation: additional points per flaw"@en ;
                                            gen:after :character_creation_flaws_selection ;
                                            gen:setAdditive :hero_points ;
                                            gen:valueFormula "5 * (number of flaws)" .


###  https://raw.githubusercontent.com/AbsVahter/ontoTRPG/main/crown_and_skull/crown_and_skull.ttl#character_creation_flaws_selection
:character_creation_flaws_selection rdf:type owl:NamedIndividual ;
                                    rdfs:comment "Take a maximum 2 flaws at creation. Flaws are entirely optional!"@en ;
                                    rdfs:label "Custom character creation: choose flaws"@en ;
                                    gen:inputOption :FlawBasic ;
                                    gen:prerequisiteDescription "number of selected flaws <= 2" ;
                                    gen:set :flaws .


###  https://raw.githubusercontent.com/AbsVahter/ontoTRPG/main/crown_and_skull/crown_and_skull.ttl#character_creation_lineage
:character_creation_lineage rdf:type owl:NamedIndividual ;
                            rdfs:label "Custom character creation: choose lineage"@en ;
                            gen:inputOption :Lineage ;
                            gen:set :lineage .


###  https://raw.githubusercontent.com/AbsVahter/ontoTRPG/main/crown_and_skull/crown_and_skull.ttl#character_creation_prompt
:character_creation_prompt rdf:type owl:NamedIndividual ;
                           rdfs:label "Character creation: select prompt"@en ;
                           gen:after :character_creation_template ;
                           gen:modified gen:pc ;
                           gen:valueFormula "prompt" .


###  https://raw.githubusercontent.com/AbsVahter/ontoTRPG/main/crown_and_skull/crown_and_skull.ttl#character_creation_skill
:character_creation_skill rdf:type owl:NamedIndividual ;
                          rdfs:label "Custom character creation: choose skills"@en ;
                          gen:after :character_creation_core_ability ;
                          gen:cost "1 point per 1 skill level" ;
                          gen:inputOption :SkillBasic ;
                          gen:resource :hero_points ;
                          gen:setAdditive :skills .


###  https://raw.githubusercontent.com/AbsVahter/ontoTRPG/main/crown_and_skull/crown_and_skull.ttl#character_creation_spell
:character_creation_spell rdf:type owl:NamedIndividual ;
                          rdfs:label "Custom character creation: buy and customise spells"@en ;
                          gen:after :character_creation_equipment ;
                          gen:cost "spell cost" ;
                          gen:input :spell_custom ;
                          gen:resource :hero_points ;
                          gen:set :spells .


###  https://raw.githubusercontent.com/AbsVahter/ontoTRPG/main/crown_and_skull/crown_and_skull.ttl#character_creation_starting_points
:character_creation_starting_points rdf:type owl:NamedIndividual ;
                                    rdfs:label "Custom character creation: starting points"@en ;
                                    gen:set :hero_points ;
                                    gen:valueNumeric 50 .


###  https://raw.githubusercontent.com/AbsVahter/ontoTRPG/main/crown_and_skull/crown_and_skull.ttl#character_creation_template
:character_creation_template rdf:type owl:NamedIndividual ;
                             rdfs:label "Character creation: select template"@en ;
                             gen:set gen:pc ;
                             gen:valueObject gen:TemplatePC .


###  https://raw.githubusercontent.com/AbsVahter/ontoTRPG/main/crown_and_skull/crown_and_skull.ttl#character_creation_templates_and_prompts
:character_creation_templates_and_prompts rdf:type owl:NamedIndividual ;
                                          rdfs:label "Character creation by templates and prompts"@en ;
                                          gen:Actor gen:player ;
                                          gen:included :character_creation_prompt ,
                                                       :character_creation_template ;
                                          gen:set gen:pc .


###  https://raw.githubusercontent.com/AbsVahter/ontoTRPG/main/crown_and_skull/crown_and_skull.ttl#check_defense
:check_defense rdf:type owl:NamedIndividual ,
                        gen:Check ;
               rdfs:label "Called-for defense roll"@en ;
               gen:checkFailure :Attrition ;
               gen:checkThreshold :threshold_defense .


###  https://raw.githubusercontent.com/AbsVahter/ontoTRPG/main/crown_and_skull/crown_and_skull.ttl#check_flat
:check_flat rdf:type owl:NamedIndividual ,
                     gen:Check ;
            rdfs:label "Flat roll"@en ;
            gen:checkThreshold :threshold_flat .


###  https://raw.githubusercontent.com/AbsVahter/ontoTRPG/main/crown_and_skull/crown_and_skull.ttl#check_skill
:check_skill rdf:type owl:NamedIndividual ,
                      gen:Check ;
             rdfs:label "Skill check"@en ;
             gen:checkFailure :check_skill_faith_failure ;
             gen:checkSuccess :check_skill_faith_success ;
             gen:checkThreshold :threshold_skill .


###  https://raw.githubusercontent.com/AbsVahter/ontoTRPG/main/crown_and_skull/crown_and_skull.ttl#check_skill_armorer
:check_skill_armorer rdf:type owl:NamedIndividual ,
                              gen:Check ;
                     rdfs:label "Armor repair check"@en ;
                     gen:basedOn :check_skill ;
                     gen:checkFailure :repair_failed ;
                     gen:checkSuccess :repair ;
                     gen:input :skill_armorer ;
                     gen:prerequisite :ItemArmor ;
                     gen:target "ally in touch distance" .


###  https://raw.githubusercontent.com/AbsVahter/ontoTRPG/main/crown_and_skull/crown_and_skull.ttl#check_skill_brawling_grapple
:check_skill_brawling_grapple rdf:type owl:NamedIndividual ,
                                       gen:Check ;
                              rdfs:label "Grapple check"@en ;
                              gen:basedOn :check_skill ;
                              gen:checkSuccess :set_status_grappled ;
                              gen:input :skill_brawling .


###  https://raw.githubusercontent.com/AbsVahter/ontoTRPG/main/crown_and_skull/crown_and_skull.ttl#check_skill_brawling_stun
:check_skill_brawling_stun rdf:type owl:NamedIndividual ,
                                    gen:Check ;
                           rdfs:label "Grapple check"@en ;
                           gen:basedOn :check_skill ;
                           gen:checkSuccess :set_status_stun_brawling ;
                           gen:input :skill_brawling .


###  https://raw.githubusercontent.com/AbsVahter/ontoTRPG/main/crown_and_skull/crown_and_skull.ttl#check_skill_breakfall
:check_skill_breakfall rdf:type owl:NamedIndividual ,
                                gen:Check ;
                       rdfs:label "Breakfall skill check"@en ;
                       gen:basedOn :check_skill ;
                       gen:checkSuccess :halving_fall_damage ;
                       gen:input :skill_breakfall .


###  https://raw.githubusercontent.com/AbsVahter/ontoTRPG/main/crown_and_skull/crown_and_skull.ttl#check_skill_faith_failure
:check_skill_faith_failure rdf:type owl:NamedIndividual ;
                           rdfs:label "Failed faith skill roll"@en ;
                           gen:prerequisite :skill_faith ;
                           gen:setCurrent :skill_faith ;
                           gen:valueFormula "temporal faith = current faith" .


###  https://raw.githubusercontent.com/AbsVahter/ontoTRPG/main/crown_and_skull/crown_and_skull.ttl#check_skill_faith_success
:check_skill_faith_success rdf:type owl:NamedIndividual ;
                           rdfs:label "Success faith skill roll"@en ;
                           gen:prerequisite :skill_faith ;
                           gen:prerequisiteDescription "temporal faith skill < 14" ;
                           gen:setCurrent :skill_faith ;
                           gen:valueFormula "temporal faith += 1" .


###  https://raw.githubusercontent.com/AbsVahter/ontoTRPG/main/crown_and_skull/crown_and_skull.ttl#check_skill_magic_vs_immobilized
:check_skill_magic_vs_immobilized rdf:type owl:NamedIndividual ,
                                           gen:Check ;
                                  rdfs:label "Magic check against immobilized status"@en ;
                                  gen:basedOn :check_skill ;
                                  gen:checkSuccess :block_status_immobilized_by_magic ;
                                  gen:input :skill_magic .


###  https://raw.githubusercontent.com/AbsVahter/ontoTRPG/main/crown_and_skull/crown_and_skull.ttl#check_skill_medical
:check_skill_medical rdf:type owl:NamedIndividual ,
                              gen:Check ;
                     rdfs:label "Medical skill check"@en ;
                     gen:basedOn :check_skill ;
                     gen:checkFailure :first_aid_failed ;
                     gen:checkSuccess :first_aid ;
                     gen:input :skill_medical .


###  https://raw.githubusercontent.com/AbsVahter/ontoTRPG/main/crown_and_skull/crown_and_skull.ttl#check_skill_muscle_vs_immobilized
:check_skill_muscle_vs_immobilized rdf:type owl:NamedIndividual ,
                                            gen:Check ;
                                   rdfs:label "Muscle check against immobilized status"@en ;
                                   gen:basedOn :check_skill ;
                                   gen:checkSuccess :block_status_immobilized_by_material_forces ;
                                   gen:input :skill_muscle .


###  https://raw.githubusercontent.com/AbsVahter/ontoTRPG/main/crown_and_skull/crown_and_skull.ttl#check_skill_repair
:check_skill_repair rdf:type owl:NamedIndividual ,
                             gen:Check ;
                    rdfs:label "Weapon and item repair check"@en ;
                    gen:basedOn :check_skill ;
                    gen:checkFailure :repair_failed ;
                    gen:checkSuccess :repair ;
                    gen:input :skill_repair ;
                    gen:prerequisite :ItemBasic ,
                                     :ItemWeapon ;
                    gen:target "ally in touch distance" .


###  https://raw.githubusercontent.com/AbsVahter/ontoTRPG/main/crown_and_skull/crown_and_skull.ttl#check_skill_resist_vs_horror
:check_skill_resist_vs_horror rdf:type owl:NamedIndividual ,
                                       gen:Check ;
                              rdfs:label "Resist horror"@en ;
                              gen:basedOn :check_skill ;
                              gen:checkFailure :set_status_afraid ;
                              gen:input :skill_resist ;
                              gen:prerequisiteDescription "extreme horror" .


###  https://raw.githubusercontent.com/AbsVahter/ontoTRPG/main/crown_and_skull/crown_and_skull.ttl#check_skill_resist_vs_stun
:check_skill_resist_vs_stun rdf:type owl:NamedIndividual ,
                                     gen:Check ;
                            rdfs:label "Resist stun"@en ;
                            gen:basedOn :check_skill ;
                            gen:checkSuccess :block_status_stun ;
                            gen:input :skill_resist .


###  https://raw.githubusercontent.com/AbsVahter/ontoTRPG/main/crown_and_skull/crown_and_skull.ttl#check_spell_infernal
:check_spell_infernal rdf:type owl:NamedIndividual ,
                               gen:Check ;
                      rdfs:label "Infernal magic check"@en ;
                      gen:basedOn :check_skill ;
                      gen:checkFailure :SpellConsequenceInfernal ;
                      gen:checkSuccess :set_spell ;
                      gen:input :skill_magic ;
                      gen:prerequisite :limitation_spell_infernal .


###  https://raw.githubusercontent.com/AbsVahter/ontoTRPG/main/crown_and_skull/crown_and_skull.ttl#check_spell_unstable
:check_spell_unstable rdf:type owl:NamedIndividual ,
                               gen:Check ;
                      rdfs:label "Unstable magic check"@en ;
                      gen:basedOn :check_skill ;
                      gen:checkFailure :SpellConsequenceUnstable ;
                      gen:checkSuccess :set_spell ;
                      gen:input :skill_magic ;
                      gen:prerequisite :limitation_spell_unstable .


###  https://raw.githubusercontent.com/AbsVahter/ontoTRPG/main/crown_and_skull/crown_and_skull.ttl#companion_custom
:companion_custom rdf:type owl:NamedIndividual ,
                           :Companion ;
                  rdfs:label "Custom companion"@en .


###  https://raw.githubusercontent.com/AbsVahter/ontoTRPG/main/crown_and_skull/crown_and_skull.ttl#companions
:companions rdf:type owl:NamedIndividual ,
                     gen:ParameterPC ;
            rdfs:comment "A companion action counts as action of PC."@en ,
                         "format = [list of companions]"@en ;
            rdfs:label "Companion"@en .


###  https://raw.githubusercontent.com/AbsVahter/ontoTRPG/main/crown_and_skull/crown_and_skull.ttl#contacting_arcanum
:contacting_arcanum rdf:type owl:NamedIndividual ;
                    rdfs:comment "A bargain as described here is made between the wizard seeking power and the semi-sentient demigod of magic energy called The Arcanum."@en ;
                    rdfs:label "Contacting the Arcanum"@en ;
                    gen:effectOption :path_of_magic_wizard_during_action ,
                                     :path_of_magic_wizard_overspend .


###  https://raw.githubusercontent.com/AbsVahter/ontoTRPG/main/crown_and_skull/crown_and_skull.ttl#core_ability
:core_ability rdf:type owl:NamedIndividual ,
                       gen:ParameterPC ;
              rdfs:comment "This is one of the most useful mechanical aspects of character."@en ;
              rdfs:label "Core ability"@en .


###  https://raw.githubusercontent.com/AbsVahter/ontoTRPG/main/crown_and_skull/crown_and_skull.ttl#core_ability_battlemaster
:core_ability_battlemaster rdf:type owl:NamedIndividual ,
                                    :CoreAbility ;
                           rdfs:comment "You have been trained as a soldier who knows how to hit hard. When you roll maximum damage, roll again. There is no limit to the number of times the dice can ‘explode.’"@en ;
                           rdfs:label "Battlemaster"@en ;
                           gen:modified :damage_roll ;
                           gen:prerequisite :equipment ;
                           gen:valueFormula "when you roll maximum value, roll again" ;
                           gen:valueObject gen:valueFormula .


###  https://raw.githubusercontent.com/AbsVahter/ontoTRPG/main/crown_and_skull/crown_and_skull.ttl#core_ability_brutal_fighter
:core_ability_brutal_fighter rdf:type owl:NamedIndividual ,
                                      :CoreAbility ;
                             rdfs:comment "You are fast, efficient, and adept at taking on multiple opponents in close quarters. All of your melee attacks may hit 2 foes with a single damage roll."@en ;
                             rdfs:label "Brutal Fighter"@en ;
                             gen:modified :set_damage ;
                             gen:prerequisite :equipment ;
                             gen:valueFormula "target: enemy -> 2 enemy" ;
                             gen:valueObject gen:target .


###  https://raw.githubusercontent.com/AbsVahter/ontoTRPG/main/crown_and_skull/crown_and_skull.ttl#core_ability_druid
:core_ability_druid rdf:type owl:NamedIndividual ,
                             :CoreAbility ;
                    rdfs:comment "Master of wilderness. Gain the Tracking and Hunting skills for free, each at 9. When outdoors, gain +3 on all skills."@en ;
                    rdfs:label "Druid"@en ;
                    gen:included :core_ability_druid_set_skills ,
                                 :core_ability_druid_skill_bonus .


###  https://raw.githubusercontent.com/AbsVahter/ontoTRPG/main/crown_and_skull/crown_and_skull.ttl#core_ability_druid_set_skills
:core_ability_druid_set_skills rdf:type owl:NamedIndividual ;
                               rdfs:comment "Gain the Tracking and Hunting skills for free, each at 9."@en ;
                               rdfs:label "Druid: gain the Tracking and Hunting skills for free"@en ;
                               gen:setAdditive :skills ;
                               gen:valueNumeric 9 ;
                               gen:valueObject :skill_hunting ,
                                               :skill_tracking .


###  https://raw.githubusercontent.com/AbsVahter/ontoTRPG/main/crown_and_skull/crown_and_skull.ttl#core_ability_druid_skill_bonus
:core_ability_druid_skill_bonus rdf:type owl:NamedIndividual ;
                                rdfs:comment "When outdoors, gain +3 on all skills."@en ;
                                rdfs:label "Druid: gain skill bonus at outdoors"@en ;
                                gen:modified :check_skill ;
                                gen:prerequisiteDescription "outdoors" ;
                                gen:valueNumeric 3 .


###  https://raw.githubusercontent.com/AbsVahter/ontoTRPG/main/crown_and_skull/crown_and_skull.ttl#core_ability_empath
:core_ability_empath rdf:type owl:NamedIndividual ,
                              :CoreAbility ;
                     rdfs:comment "You have masterful intuition. Gain the Investigation, Streetwise, and Oratory skills at a value of 7 for free."@en ;
                     rdfs:label "Empath"@en ;
                     gen:setAdditive :skills ;
                     gen:valueNumeric 7 ;
                     gen:valueObject :skill_investigate ,
                                     :skill_oratory ,
                                     :skill_streetwise .


###  https://raw.githubusercontent.com/AbsVahter/ontoTRPG/main/crown_and_skull/crown_and_skull.ttl#core_ability_go_unnoticed
:core_ability_go_unnoticed rdf:type owl:NamedIndividual ,
                                    :CoreAbility ;
                           rdfs:comment "You blend into shadows with ease. When enemies are attacking you and your allies, they will target you last."@en ;
                           rdfs:label "Go Unnoticed"@en ;
                           gen:modified :attack_of_enemy .


###  https://raw.githubusercontent.com/AbsVahter/ontoTRPG/main/crown_and_skull/crown_and_skull.ttl#core_ability_mountaineer
:core_ability_mountaineer rdf:type owl:NamedIndividual ,
                                   :CoreAbility ;
                          rdfs:comment "A master of finding ways through rock and cavern. Gain the Climber and Breakfall skills at 10. In mountains or underground, you also have a Scout skill of 15."@en ;
                          rdfs:label "Mountaineer"@en ;
                          gen:included :core_ability_mountaineer_climber_and_breakfall ,
                                       :core_ability_mountaineer_scout .


###  https://raw.githubusercontent.com/AbsVahter/ontoTRPG/main/crown_and_skull/crown_and_skull.ttl#core_ability_mountaineer_climber_and_breakfall
:core_ability_mountaineer_climber_and_breakfall rdf:type owl:NamedIndividual ;
                                                rdfs:comment "Gain the Climber and Breakfall skills at 10"@en ;
                                                rdfs:label "Mountaineer: gain the Climber and Breakfall skills"@en ;
                                                gen:setAdditive :skills ;
                                                gen:valueNumeric 10 ;
                                                gen:valueObject :skill_breakfall ,
                                                                :skill_climber .


###  https://raw.githubusercontent.com/AbsVahter/ontoTRPG/main/crown_and_skull/crown_and_skull.ttl#core_ability_mountaineer_scout
:core_ability_mountaineer_scout rdf:type owl:NamedIndividual ;
                                rdfs:comment "Gain the Scout skills at 15 in mountains or underground"@en ;
                                rdfs:label "Mountaineer: gain the Scout skill"@en ;
                                gen:prerequisiteDescription "in mountains or underground" ;
                                gen:setAdditive :skills ;
                                gen:valueNumeric 15 ;
                                gen:valueObject :skill_scout .


###  https://raw.githubusercontent.com/AbsVahter/ontoTRPG/main/crown_and_skull/crown_and_skull.ttl#core_ability_paragon_of_faith
:core_ability_paragon_of_faith rdf:type owl:NamedIndividual ,
                                        :CoreAbility ;
                               rdfs:comment "Your Faith skill grows by 2 with a successful cast, and maxes at 16. Additionally, destroy 1D6 weak undead (such as zombies, shamblers, or skeletons) as an Exhausting spell."@en ;
                               rdfs:label "Paragon of Faith"@en ;
                               gen:included :core_ability_paragon_of_faith_bonus_to_faith_grow ,
                                            :core_ability_paragon_of_faith_destroy_undead .


###  https://raw.githubusercontent.com/AbsVahter/ontoTRPG/main/crown_and_skull/crown_and_skull.ttl#core_ability_paragon_of_faith_bonus_to_faith_grow
:core_ability_paragon_of_faith_bonus_to_faith_grow rdf:type owl:NamedIndividual ;
                                                   rdfs:comment "Your Faith skill grows by 2 with a successful cast, and maxes at 16."@en ;
                                                   rdfs:label "Paragon of Faith: Faith skill grows by 2 with a successful cast"@en ;
                                                   gen:modified :check_skill_faith_success ;
                                                   gen:valueFormula "{formula: temporal faith += 2; prerequisite: temporal faith skill <= 16}" ;
                                                   gen:valueObject gen:prerequisiteDescription ,
                                                                   gen:valueFormula .


###  https://raw.githubusercontent.com/AbsVahter/ontoTRPG/main/crown_and_skull/crown_and_skull.ttl#core_ability_paragon_of_faith_destroy_undead
:core_ability_paragon_of_faith_destroy_undead rdf:type owl:NamedIndividual ;
                                              rdfs:comment "Destroy 1D6 weak undead (such as zombies, shamblers, or skeletons) as an Exhausting spell."@en ;
                                              rdfs:label "Paragon of Faith: destroy undead"@en ;
                                              gen:modified :perform_action ;
                                              gen:set :status_exhausting .


###  https://raw.githubusercontent.com/AbsVahter/ontoTRPG/main/crown_and_skull/crown_and_skull.ttl#core_ability_protector
:core_ability_protector rdf:type owl:NamedIndividual ,
                                 :CoreAbility ;
                        rdfs:comment "When using a shield, change a failed Defense roll by an ally into a success once per round, if they are nearby."@en ;
                        rdfs:label "Protector"@en ;
                        gen:input :equipment ;
                        gen:modified :check_defense ;
                        gen:prerequisiteDescription "(worn shield) and (once per round)" ;
                        gen:target "nearby ally" ;
                        gen:valueFormula "fail -> success" ;
                        gen:valueObject gen:effect .


###  https://raw.githubusercontent.com/AbsVahter/ontoTRPG/main/crown_and_skull/crown_and_skull.ttl#core_ability_spellsinger
:core_ability_spellsinger rdf:type owl:NamedIndividual ,
                                   :CoreAbility ;
                          rdfs:comment "You cast spells with flair and oratory. You can never use ‘silent’ or ‘still’ spells. As a default, though, your spells work on a target that can HEAR you cast. Upgrade from there as normal."@en ;
                          rdfs:label "Spellsinger"@en ;
                          gen:modified :creation_custom_spell .


###  https://raw.githubusercontent.com/AbsVahter/ontoTRPG/main/crown_and_skull/crown_and_skull.ttl#core_ability_uncanny_shot
:core_ability_uncanny_shot rdf:type owl:NamedIndividual ,
                                    :CoreAbility ;
                           rdfs:comment "Roll an extra damage die with all ranged weapons, and ignore 1 DEF on all targets when using ranged weapons."@en ;
                           rdfs:label "Uncanny Shot"@en ;
                           gen:input :equipment ;
                           gen:modified :set_damage ;
                           gen:prerequisiteDescription "worn ranged weapon" ;
                           gen:valueFormula "formula: (defense of enemy - 1) + (damage penalty) - 2 * (damage roll)" ;
                           gen:valueObject gen:valueFormula .


###  https://raw.githubusercontent.com/AbsVahter/ontoTRPG/main/crown_and_skull/crown_and_skull.ttl#core_ability_veteran_commander
:core_ability_veteran_commander rdf:type owl:NamedIndividual ,
                                         :CoreAbility ;
                                rdfs:comment "When a combat encounter starts, choose 1 ally. Inspire them with a command to fight! Their first attack does maximum damage, and they cannot be harmed for the remainder of that round."@en ;
                                rdfs:label "Veteran Commander"@en ;
                                gen:modified :attack_of_enemy ,
                                             :damage_roll ;
                                gen:prerequisiteDescription "first attack" ;
                                gen:target "ally" .


###  https://raw.githubusercontent.com/AbsVahter/ontoTRPG/main/crown_and_skull/crown_and_skull.ttl#core_ability_wizard_savant
:core_ability_wizard_savant rdf:type owl:NamedIndividual ,
                                     :CoreAbility ;
                            rdfs:comment "You don’t just cast spells; you are a conduit of incredible power. When casting, effects and outputs of all magic you cast are maximized on a Magic skill roll of 6 or less on a D20."@en ;
                            rdfs:label "Wizard Savant"@en .


###  https://raw.githubusercontent.com/AbsVahter/ontoTRPG/main/crown_and_skull/crown_and_skull.ttl#creation_custom_companion
:creation_custom_companion rdf:type owl:NamedIndividual ;
                           rdfs:label "Custom companion creation"@en ;
                           gen:Actor gen:player ;
                           gen:included :creation_custom_companion_base ,
                                        :creation_custom_companion_skills ,
                                        :creation_custom_companion_upgrade ;
                           gen:set :companion_custom .


###  https://raw.githubusercontent.com/AbsVahter/ontoTRPG/main/crown_and_skull/crown_and_skull.ttl#creation_custom_companion_base
:creation_custom_companion_base rdf:type owl:NamedIndividual ;
                                rdfs:label "Custom companion: base"@en ;
                                gen:inputOption :Companion ;
                                gen:set :companion_custom ;
                                gen:valueFormula """
cost = (base companion cost) or
{
    small animal (d4 attacks, 1 skill value 9, 6 defense): 3 points ;
    medium sized beasts or simple devices (d6 attacks, 2 skills value 9, 9 defense): 5 points ;
    large animals or retainers (d8 attacks, 3 skills value 9, 9 defense): 12 points ;
}
""" .


###  https://raw.githubusercontent.com/AbsVahter/ontoTRPG/main/crown_and_skull/crown_and_skull.ttl#creation_custom_companion_skills
:creation_custom_companion_skills rdf:type owl:NamedIndividual ;
                                  rdfs:label "Custom companion: skills"@en ;
                                  gen:after :creation_custom_companion_base ;
                                  gen:prerequisiteDescription "number of skills <= maximum of skills of base" ;
                                  gen:setAdditive :companion_custom ;
                                  gen:valueObject :SkillCompanion .


###  https://raw.githubusercontent.com/AbsVahter/ontoTRPG/main/crown_and_skull/crown_and_skull.ttl#creation_custom_companion_upgrade
:creation_custom_companion_upgrade rdf:type owl:NamedIndividual ;
                                   rdfs:label "Custom companion: upgrade"@en ;
                                   gen:after :creation_custom_companion_skills ;
                                   gen:prerequisiteDescription "final cost > 0" ;
                                   gen:resource :hero_points ;
                                   gen:setAdditive :companion_custom ;
                                   gen:valueFormula """
cost += {
    effect: 3 points ;
    limitation: -3 points ;
}
""" ;
                                   gen:valueObject :EffectCompanion ,
                                                   :LimitationCompanion .


###  https://raw.githubusercontent.com/AbsVahter/ontoTRPG/main/crown_and_skull/crown_and_skull.ttl#creation_custom_item
:creation_custom_item rdf:type owl:NamedIndividual ;
                      rdfs:label "Custom item creation"@en ;
                      gen:Actor gen:player ;
                      gen:included :creation_custom_item_base ,
                                   :creation_custom_item_upgrade ;
                      gen:set :item_custom .


###  https://raw.githubusercontent.com/AbsVahter/ontoTRPG/main/crown_and_skull/crown_and_skull.ttl#creation_custom_item_base
:creation_custom_item_base rdf:type owl:NamedIndividual ;
                           rdfs:label "Custom item: base"@en ;
                           gen:inputOption :Item ;
                           gen:set :item_custom ;
                           gen:valueFormula """
cost = (base item cost) or
{
    d6 weapon, +1 armor (small weapons, pouches, rope, lantern, torch, climbing kit, travel rations, staff, ring or jewelry item, cloak, boots): 1 point ;
    d8 weapon, +2 armor (medium-sized weapons, light armor, flares, bear traps & snares, thieves’ tools, common supplies): 2 points ;
    d10 weapon, +3 armor (heavy and exotic weapons, mechanized weapons and tools, gear for horses, complex or heavy armor): 3 points ;
    d12 weapon, +4 armor (firearms, siege weapons, war-ready equipment and armor): 5 points ;
}
""" .


###  https://raw.githubusercontent.com/AbsVahter/ontoTRPG/main/crown_and_skull/crown_and_skull.ttl#creation_custom_item_upgrade
:creation_custom_item_upgrade rdf:type owl:NamedIndividual ;
                              rdfs:label "Custom item: upgrade"@en ;
                              gen:after :creation_custom_item_base ;
                              gen:prerequisiteDescription "(limitations cannot be added as part of an upgrade while rest) and (no stacking) and (final cost > 0)" ;
                              gen:resource :hero_points ;
                              gen:setAdditive :item_custom ;
                              gen:valueFormula """
cost += {
    effect: 3 points ;
    limitation: -3 points ;
}
""" ;
                              gen:valueObject :EffectItem ,
                                              :LimitationItem .


###  https://raw.githubusercontent.com/AbsVahter/ontoTRPG/main/crown_and_skull/crown_and_skull.ttl#creation_custom_spell
:creation_custom_spell rdf:type owl:NamedIndividual ;
                       rdfs:label "Custom spell creation"@en ;
                       gen:Actor gen:player ;
                       gen:included :creation_custom_spell_base ,
                                    :creation_custom_spell_upgrade ;
                       gen:set :spell_custom .


###  https://raw.githubusercontent.com/AbsVahter/ontoTRPG/main/crown_and_skull/crown_and_skull.ttl#creation_custom_spell_base
:creation_custom_spell_base rdf:type owl:NamedIndividual ;
                            rdfs:label "Custom spell: base"@en ;
                            gen:inputOption :Spell ;
                            gen:set :spell_custom ;
                            gen:valueFormula """
cost = (base spell cost) or
{
    normal spell: 3 points ;
    heavy spell: 5 points ;
}
""" .


###  https://raw.githubusercontent.com/AbsVahter/ontoTRPG/main/crown_and_skull/crown_and_skull.ttl#creation_custom_spell_upgrade
:creation_custom_spell_upgrade rdf:type owl:NamedIndividual ;
                               rdfs:label "Custom spell: upgrade"@en ;
                               gen:after :creation_custom_spell_base ;
                               gen:prerequisiteDescription "(no stacking limitations) and (effect's stack < 4) and (final cost > 0)" ;
                               gen:resource :hero_points ;
                               gen:setAdditive :spell_custom ;
                               gen:valueFormula """
cost += {
    effect: 3 points ;
    limitation: -3 points ;
}
""" ;
                               gen:valueObject :EffectSpell ,
                                               :LimitationSpell .


###  https://raw.githubusercontent.com/AbsVahter/ontoTRPG/main/crown_and_skull/crown_and_skull.ttl#crown
:crown rdf:type owl:NamedIndividual ;
       rdfs:comment "Those who choose the CROWN will join an order of protectors, knights, and heralds sworn to the well-being of the realm, the sanctity of all life, and the upholding of ancient codes. They swear to honor the decrees of kings and queens, to serve as a beacon of truth and loyalty." ;
       rdfs:label "Crown"@en ;
       gen:included :crown_gain_ring ,
                    :crown_gaining_hero_points ,
                    :crown_select_equipment ,
                    :crown_select_skill ,
                    :crown_set_flaw .


###  https://raw.githubusercontent.com/AbsVahter/ontoTRPG/main/crown_and_skull/crown_and_skull.ttl#crown_gain_ring
:crown_gain_ring rdf:type owl:NamedIndividual ;
                 rdfs:label "Crown: gaining Ring of the Anvil's Light"@en ;
                 gen:Actor gen:player ;
                 gen:setAdditive :equipment ;
                 gen:valueObject :ring_anvil_light .


###  https://raw.githubusercontent.com/AbsVahter/ontoTRPG/main/crown_and_skull/crown_and_skull.ttl#crown_gaining_hero_points
:crown_gaining_hero_points rdf:type owl:NamedIndividual ;
                           rdfs:label "Crown: gaining hero points"@en ;
                           gen:Actor gen:master ;
                           gen:setAdditive :hero_points ;
                           gen:valueNumeric 6 .


###  https://raw.githubusercontent.com/AbsVahter/ontoTRPG/main/crown_and_skull/crown_and_skull.ttl#crown_or_skull
:crown_or_skull rdf:type owl:NamedIndividual ;
                rdfs:comment """
Since the fall of the world’s unity three decades ago, many heroes have faced this choice. It has become tradition... a sacrament to lend order to a chaotic world.
If a hero refuses to choose, they will be scorned widely, possibly deemed an enemy to all.
"""@en ;
                rdfs:label "Crown or Skull?"@en ;
                gen:Actor gen:party ;
                gen:effectOption :crown ,
                                 :skull ;
                gen:input :hero_points ;
                gen:prerequisiteDescription "(earned hero points >= 25) and (only chance)" ;
                gen:valueFormula "crown xor skull xor nothing" .


###  https://raw.githubusercontent.com/AbsVahter/ontoTRPG/main/crown_and_skull/crown_and_skull.ttl#crown_select_equipment
:crown_select_equipment rdf:type owl:NamedIndividual ;
                        rdfs:label "Crown: choosing equipment"@en ;
                        gen:Actor gen:player ;
                        gen:inputOption :ItemCrown ;
                        gen:setAdditive :equipment ;
                        gen:valueFormula "1 item" .


###  https://raw.githubusercontent.com/AbsVahter/ontoTRPG/main/crown_and_skull/crown_and_skull.ttl#crown_select_skill
:crown_select_skill rdf:type owl:NamedIndividual ;
                    rdfs:label "Crown: choosing skill"@en ;
                    gen:Actor gen:player ;
                    gen:inputOption :SkillCrown ;
                    gen:setAdditive :skills ;
                    gen:valueFormula "1 crown skill with level 9" ;
                    gen:valueNumeric 9 .


###  https://raw.githubusercontent.com/AbsVahter/ontoTRPG/main/crown_and_skull/crown_and_skull.ttl#crown_set_flaw
:crown_set_flaw rdf:type owl:NamedIndividual ;
                rdfs:label "Crown: set Crown-Sworn flaw"@en ;
                gen:Actor gen:player ;
                gen:setAdditive :flaws ;
                gen:valueObject :flaw_crown_sworn .


###  https://raw.githubusercontent.com/AbsVahter/ontoTRPG/main/crown_and_skull/crown_and_skull.ttl#damage_penalty
:damage_penalty rdf:type owl:NamedIndividual ;
                rdfs:label "Penalty to damage roll"@en ;
                gen:valueFormula "zero by default" .


###  https://raw.githubusercontent.com/AbsVahter/ontoTRPG/main/crown_and_skull/crown_and_skull.ttl#damage_roll
:damage_roll rdf:type owl:NamedIndividual ;
             rdfs:label "Damage roll"@en ;
             gen:inputOption :companions ,
                             :equipment ,
                             :skill_brawling ,
                             :spells ;
             gen:valueFormula "roll of (worn weapon or spell or companion or (d6 if brawling > 0)) damage stat" .


###  https://raw.githubusercontent.com/AbsVahter/ontoTRPG/main/crown_and_skull/crown_and_skull.ttl#death_of_pc
:death_of_pc rdf:type owl:NamedIndividual ;
             rdfs:label "Death of PC at encounter"@en ;
             gen:after :phase_action ;
             gen:prerequisite :status_close_to_death ;
             gen:prerequisiteDescription "(close to death) and (after phase 5)" ;
             gen:set gen:death .


###  https://raw.githubusercontent.com/AbsVahter/ontoTRPG/main/crown_and_skull/crown_and_skull.ttl#deeds
:deeds rdf:type owl:NamedIndividual ,
                gen:ParameterPC ;
       rdfs:comment """
{
    3 deeds: after a few exploits, a hero or group receives a title derived from a famous doing ;
    5 deeds: after so many doings, our heroes acquire actual titles either individually or as group ;
    10 deeds: here the greatest heroes fi nd their place in history ;
}"""@en ;
       rdfs:label "Deeds"@en .


###  https://raw.githubusercontent.com/AbsVahter/ontoTRPG/main/crown_and_skull/crown_and_skull.ttl#defense_penalty
:defense_penalty rdf:type owl:NamedIndividual ;
                 rdfs:label "Penalty to defense"@en .


###  https://raw.githubusercontent.com/AbsVahter/ontoTRPG/main/crown_and_skull/crown_and_skull.ttl#dunsel_and_kid
:dunsel_and_kid rdf:type owl:NamedIndividual ;
                rdfs:comment "Operating from a blacksmith-and-mercantile in town called ‘Haldur’s Goods,’ Dunsel is a stout folk merchant, beer expert, and journeyman smith. His ever-present sidekick is a fearless boy known simply as The Kid. These two have their ear to most of the goings-on in town, and the growing military challenges at hand."@en ;
                rdfs:label "Dunsel & the Kid"@en .


###  https://raw.githubusercontent.com/AbsVahter/ontoTRPG/main/crown_and_skull/crown_and_skull.ttl#effect_companion_cunning
:effect_companion_cunning rdf:type owl:NamedIndividual ,
                                   :EffectCompanion ;
                          rdfs:comment "Upgrade the skill value used by +1."@en ;
                          rdfs:label "Cunning"@en .


###  https://raw.githubusercontent.com/AbsVahter/ontoTRPG/main/crown_and_skull/crown_and_skull.ttl#effect_companion_deadly
:effect_companion_deadly rdf:type owl:NamedIndividual ,
                                  :EffectCompanion ;
                         rdfs:comment "Upgrade the companion’s damage with an additional die."@en ;
                         rdfs:label "Deadly"@en .


###  https://raw.githubusercontent.com/AbsVahter/ontoTRPG/main/crown_and_skull/crown_and_skull.ttl#effect_companion_evasive
:effect_companion_evasive rdf:type owl:NamedIndividual ,
                                   :EffectCompanion ;
                          rdfs:comment "This creature gains +3 Defense."@en ;
                          rdfs:label "Evasive"@en .


###  https://raw.githubusercontent.com/AbsVahter/ontoTRPG/main/crown_and_skull/crown_and_skull.ttl#effect_companion_precise
:effect_companion_precise rdf:type owl:NamedIndividual ,
                                   :EffectCompanion ;
                          rdfs:comment "Your companion ignores most penalties in combat."@en ;
                          rdfs:label "Precise"@en .


###  https://raw.githubusercontent.com/AbsVahter/ontoTRPG/main/crown_and_skull/crown_and_skull.ttl#effect_item_balanced_weapon
:effect_item_balanced_weapon rdf:type owl:NamedIndividual ,
                                      :EffectItem ;
                             rdfs:comment "Ignore 1 target DEF to attack with this weapon."@en ;
                             rdfs:label "Balanced weapon"@en .


###  https://raw.githubusercontent.com/AbsVahter/ontoTRPG/main/crown_and_skull/crown_and_skull.ttl#effect_item_bleed
:effect_item_bleed rdf:type owl:NamedIndividual ,
                            :EffectItem ;
                   rdfs:comment "After inflicting damage, target bleeds same damage D4 rounds."@en ;
                   rdfs:label "Bleed"@en .


###  https://raw.githubusercontent.com/AbsVahter/ontoTRPG/main/crown_and_skull/crown_and_skull.ttl#effect_item_chained_weapon
:effect_item_chained_weapon rdf:type owl:NamedIndividual ,
                                     :EffectItem ;
                            rdfs:comment "You cannot lose or be robbed of this weapon."@en ;
                            rdfs:label "Chained weapon"@en .


###  https://raw.githubusercontent.com/AbsVahter/ontoTRPG/main/crown_and_skull/crown_and_skull.ttl#effect_item_cold_forged
:effect_item_cold_forged rdf:type owl:NamedIndividual ,
                                  :EffectItem ;
                         rdfs:comment "This metal equipment is immune to corrosion of all kinds."@en ;
                         rdfs:label "Cold Forged"@en .


###  https://raw.githubusercontent.com/AbsVahter/ontoTRPG/main/crown_and_skull/crown_and_skull.ttl#effect_item_compact
:effect_item_compact rdf:type owl:NamedIndividual ,
                              :EffectItem ;
                     rdfs:comment "This gear incurs no unwanted attention or clumsiness."@en ;
                     rdfs:label "Compact"@en .


###  https://raw.githubusercontent.com/AbsVahter/ontoTRPG/main/crown_and_skull/crown_and_skull.ttl#effect_item_deadly_weapon
:effect_item_deadly_weapon rdf:type owl:NamedIndividual ,
                                    :EffectItem ;
                           rdfs:comment "Add an additional damage die of the weapon’s type."@en ;
                           rdfs:label "Deadly weapon"@en .


###  https://raw.githubusercontent.com/AbsVahter/ontoTRPG/main/crown_and_skull/crown_and_skull.ttl#effect_item_die_upgrade
:effect_item_die_upgrade rdf:type owl:NamedIndividual ,
                                  :EffectItem ;
                         rdfs:comment "Upgrade the damage die of a weapon by 1 grade."@en ;
                         rdfs:label "Die Upgrade"@en .


###  https://raw.githubusercontent.com/AbsVahter/ontoTRPG/main/crown_and_skull/crown_and_skull.ttl#effect_item_lightweight
:effect_item_lightweight rdf:type owl:NamedIndividual ,
                                  :EffectItem ;
                         rdfs:comment "Finely made equipment doesn’t inhibit stealth or swimming."@en ;
                         rdfs:label "Lightweight"@en .


###  https://raw.githubusercontent.com/AbsVahter/ontoTRPG/main/crown_and_skull/crown_and_skull.ttl#effect_item_lucky_weapon
:effect_item_lucky_weapon rdf:type owl:NamedIndividual ,
                                   :EffectItem ;
                          rdfs:comment "Critical fails with this weapon incur no penalties."@en ;
                          rdfs:label "Lucky weapon"@en .


###  https://raw.githubusercontent.com/AbsVahter/ontoTRPG/main/crown_and_skull/crown_and_skull.ttl#effect_item_reinforced
:effect_item_reinforced rdf:type owl:NamedIndividual ,
                                 :EffectItem ;
                        rdfs:comment "This gear is resilient to damage (2 hits to cross off)."@en ;
                        rdfs:label "Reinforced"@en .


###  https://raw.githubusercontent.com/AbsVahter/ontoTRPG/main/crown_and_skull/crown_and_skull.ttl#effect_item_reinforced_armor
:effect_item_reinforced_armor rdf:type owl:NamedIndividual ,
                                       :EffectItem ;
                              rdfs:comment "Add an additional +1 Defense."@en ;
                              rdfs:label "Reinforced armor"@en .


###  https://raw.githubusercontent.com/AbsVahter/ontoTRPG/main/crown_and_skull/crown_and_skull.ttl#effect_spell_accuracy
:effect_spell_accuracy rdf:type owl:NamedIndividual ,
                                :EffectSpell ;
                       rdfs:comment "Boost an upcoming damage roll."@en ;
                       rdfs:label "Accuracy"@en .


###  https://raw.githubusercontent.com/AbsVahter/ontoTRPG/main/crown_and_skull/crown_and_skull.ttl#effect_spell_adapt
:effect_spell_adapt rdf:type owl:NamedIndividual ,
                             :EffectSpell ;
                    rdfs:comment "Select a specific substance you can now breathe easily."@en ;
                    rdfs:label "Adapt"@en .


###  https://raw.githubusercontent.com/AbsVahter/ontoTRPG/main/crown_and_skull/crown_and_skull.ttl#effect_spell_additional_cast
:effect_spell_additional_cast rdf:type owl:NamedIndividual ,
                                       :EffectSpell ;
                              rdfs:comment "Add a cast to this spell."@en ;
                              rdfs:label "Additional Cast"@en .


###  https://raw.githubusercontent.com/AbsVahter/ontoTRPG/main/crown_and_skull/crown_and_skull.ttl#effect_spell_analyze
:effect_spell_analyze rdf:type owl:NamedIndividual ,
                               :EffectSpell ;
                      rdfs:comment "Cast and roll effect. If this effect is greater than the approximate point value of the target spell or item, gain all information about it."@en ;
                      rdfs:label "Analyze"@en .


###  https://raw.githubusercontent.com/AbsVahter/ontoTRPG/main/crown_and_skull/crown_and_skull.ttl#effect_spell_animate
:effect_spell_animate rdf:type owl:NamedIndividual ,
                               :EffectSpell ;
                      rdfs:comment "Use objects as puppets, D6 of them per cast."@en ;
                      rdfs:label "Animate"@en .


###  https://raw.githubusercontent.com/AbsVahter/ontoTRPG/main/crown_and_skull/crown_and_skull.ttl#effect_spell_arcane_armor
:effect_spell_arcane_armor rdf:type owl:NamedIndividual ,
                                    :EffectSpell ;
                           rdfs:comment "Roll the output effect and add it to target Defense."@en ;
                           rdfs:label "Arcane Armor"@en .


###  https://raw.githubusercontent.com/AbsVahter/ontoTRPG/main/crown_and_skull/crown_and_skull.ttl#effect_spell_area
:effect_spell_area rdf:type owl:NamedIndividual ,
                            :EffectSpell ;
                   rdfs:comment "Modify a single-target spell to affect an arm’s-width radius."@en ;
                   rdfs:label "Area"@en .


###  https://raw.githubusercontent.com/AbsVahter/ontoTRPG/main/crown_and_skull/crown_and_skull.ttl#effect_spell_banish
:effect_spell_banish rdf:type owl:NamedIndividual ,
                              :EffectSpell ;
                     rdfs:comment "Cast out a summoned creature or construct."@en ;
                     rdfs:label "Banish"@en .


###  https://raw.githubusercontent.com/AbsVahter/ontoTRPG/main/crown_and_skull/crown_and_skull.ttl#effect_spell_blast
:effect_spell_blast rdf:type owl:NamedIndividual ,
                             :EffectSpell ;
                    rdfs:comment "Inflict magic damage of specified theme, element, or style."@en ;
                    rdfs:label "Blast"@en .


###  https://raw.githubusercontent.com/AbsVahter/ontoTRPG/main/crown_and_skull/crown_and_skull.ttl#effect_spell_clairvoyance
:effect_spell_clairvoyance rdf:type owl:NamedIndividual ,
                                    :EffectSpell ;
                           rdfs:comment "Affect unseen target(s) with rolled effect x 10’ distance."@en ;
                           rdfs:label "Clairvoyance"@en .


###  https://raw.githubusercontent.com/AbsVahter/ontoTRPG/main/crown_and_skull/crown_and_skull.ttl#effect_spell_cloak
:effect_spell_cloak rdf:type owl:NamedIndividual ,
                             :EffectSpell ;
                    rdfs:comment "Reduce the chance of being spotted by others. This effect can have many variations including camouflage, stillness, deception."@en ;
                    rdfs:label "Cloak"@en .


###  https://raw.githubusercontent.com/AbsVahter/ontoTRPG/main/crown_and_skull/crown_and_skull.ttl#effect_spell_clone
:effect_spell_clone rdf:type owl:NamedIndividual ,
                             :EffectSpell ;
                    rdfs:comment "Duplicate an object or person into a semi-real copy."@en ;
                    rdfs:label "Clone"@en .


###  https://raw.githubusercontent.com/AbsVahter/ontoTRPG/main/crown_and_skull/crown_and_skull.ttl#effect_spell_create
:effect_spell_create rdf:type owl:NamedIndividual ,
                              :EffectSpell ;
                     rdfs:comment "Create an object imbued with a spell you know. At its base level, this spell creates an object with 1 use of the selected spell."@en ;
                     rdfs:label "Create"@en .


###  https://raw.githubusercontent.com/AbsVahter/ontoTRPG/main/crown_and_skull/crown_and_skull.ttl#effect_spell_detect_object
:effect_spell_detect_object rdf:type owl:NamedIndividual ,
                                     :EffectSpell ;
                            rdfs:comment "Detect a specific object."@en ;
                            rdfs:label "Detect Object"@en .


###  https://raw.githubusercontent.com/AbsVahter/ontoTRPG/main/crown_and_skull/crown_and_skull.ttl#effect_spell_dice_upgrade
:effect_spell_dice_upgrade rdf:type owl:NamedIndividual ,
                                    :EffectSpell ;
                           rdfs:comment "Increase the dice used by this spell by one grade."@en ;
                           rdfs:label "Dice Upgrade"@en .


###  https://raw.githubusercontent.com/AbsVahter/ontoTRPG/main/crown_and_skull/crown_and_skull.ttl#effect_spell_dispel
:effect_spell_dispel rdf:type owl:NamedIndividual ,
                              :EffectSpell ;
                     rdfs:comment "To cancel a spell, roll this output. Surpass the point value of the target spell to cancel it. Sacrifice your next phase to dispel immediately."@en ;
                     rdfs:label "Dispel"@en .


###  https://raw.githubusercontent.com/AbsVahter/ontoTRPG/main/crown_and_skull/crown_and_skull.ttl#effect_spell_dominate
:effect_spell_dominate rdf:type owl:NamedIndividual ,
                                :EffectSpell ;
                       rdfs:comment "Target rolls a D20. Surpass that roll with effect to dominate."@en ;
                       rdfs:label "Dominate"@en .


###  https://raw.githubusercontent.com/AbsVahter/ontoTRPG/main/crown_and_skull/crown_and_skull.ttl#effect_spell_drain
:effect_spell_drain rdf:type owl:NamedIndividual ,
                             :EffectSpell ;
                    rdfs:comment "Reduce a target’s DEF or ATK for 1 round."@en ;
                    rdfs:label "Drain"@en .


###  https://raw.githubusercontent.com/AbsVahter/ontoTRPG/main/crown_and_skull/crown_and_skull.ttl#effect_spell_duration
:effect_spell_duration rdf:type owl:NamedIndividual ,
                                :EffectSpell ;
                       rdfs:comment "Upgrade from 1D6 phases default to 1 full round duration."@en ;
                       rdfs:label "Duration"@en .


###  https://raw.githubusercontent.com/AbsVahter/ontoTRPG/main/crown_and_skull/crown_and_skull.ttl#effect_spell_enchant
:effect_spell_enchant rdf:type owl:NamedIndividual ,
                               :EffectSpell ;
                      rdfs:comment "Imbue a weapon or object with a single gear effect."@en ;
                      rdfs:label "Enchant"@en .


###  https://raw.githubusercontent.com/AbsVahter/ontoTRPG/main/crown_and_skull/crown_and_skull.ttl#effect_spell_evade
:effect_spell_evade rdf:type owl:NamedIndividual ,
                             :EffectSpell ;
                    rdfs:comment "Boost the Evade skill of a target."@en ;
                    rdfs:label "Evade"@en .


###  https://raw.githubusercontent.com/AbsVahter/ontoTRPG/main/crown_and_skull/crown_and_skull.ttl#effect_spell_haste
:effect_spell_haste rdf:type owl:NamedIndividual ,
                             :EffectSpell ;
                    rdfs:comment "Run or swim (choose on purchase) twice as fast as others."@en ;
                    rdfs:label "Haste"@en .


###  https://raw.githubusercontent.com/AbsVahter/ontoTRPG/main/crown_and_skull/crown_and_skull.ttl#effect_spell_held_spell
:effect_spell_held_spell rdf:type owl:NamedIndividual ,
                                  :EffectSpell ;
                         rdfs:comment "Use a turn to ‘pre-cast’ spell, triggering it any time after."@en ;
                         rdfs:label "Held Spell"@en .


###  https://raw.githubusercontent.com/AbsVahter/ontoTRPG/main/crown_and_skull/crown_and_skull.ttl#effect_spell_illusions
:effect_spell_illusions rdf:type owl:NamedIndividual ,
                                 :EffectSpell ;
                        rdfs:comment "Place illusions into a mind directly, or fabricate them for all."@en ;
                        rdfs:label "Illusions"@en .


###  https://raw.githubusercontent.com/AbsVahter/ontoTRPG/main/crown_and_skull/crown_and_skull.ttl#effect_spell_language
:effect_spell_language rdf:type owl:NamedIndividual ,
                                :EffectSpell ;
                       rdfs:comment "Listen, speak, or translate any language or cypher."@en ;
                       rdfs:label "Language"@en .


###  https://raw.githubusercontent.com/AbsVahter/ontoTRPG/main/crown_and_skull/crown_and_skull.ttl#effect_spell_lasting
:effect_spell_lasting rdf:type owl:NamedIndividual ,
                               :EffectSpell ;
                      rdfs:comment "Make a spell’s output permanent, with GM approval, for a cost of 15 points."@en ;
                      rdfs:label "Lasting"@en .


###  https://raw.githubusercontent.com/AbsVahter/ontoTRPG/main/crown_and_skull/crown_and_skull.ttl#effect_spell_levitate
:effect_spell_levitate rdf:type owl:NamedIndividual ,
                                :EffectSpell ;
                       rdfs:comment "Hover or move a few feet above the ground."@en ;
                       rdfs:label "Levitate"@en .


###  https://raw.githubusercontent.com/AbsVahter/ontoTRPG/main/crown_and_skull/crown_and_skull.ttl#effect_spell_locate
:effect_spell_locate rdf:type owl:NamedIndividual ,
                              :EffectSpell ;
                     rdfs:comment "Locate a person without seeing them. If being located by an enemy, roll your Magic skill to evade detection."@en ;
                     rdfs:label "Locate"@en .


###  https://raw.githubusercontent.com/AbsVahter/ontoTRPG/main/crown_and_skull/crown_and_skull.ttl#effect_spell_mend
:effect_spell_mend rdf:type owl:NamedIndividual ,
                            :EffectSpell ;
                   rdfs:comment "Repair 1 weapon, item, or piece of armor."@en ;
                   rdfs:label "Mend"@en .


###  https://raw.githubusercontent.com/AbsVahter/ontoTRPG/main/crown_and_skull/crown_and_skull.ttl#effect_spell_metal
:effect_spell_metal rdf:type owl:NamedIndividual ,
                             :EffectSpell ;
                    rdfs:comment "Manipulate metal in numerous ways."@en ;
                    rdfs:label "Metal"@en .


###  https://raw.githubusercontent.com/AbsVahter/ontoTRPG/main/crown_and_skull/crown_and_skull.ttl#effect_spell_mind_defense
:effect_spell_mind_defense rdf:type owl:NamedIndividual ,
                                    :EffectSpell ;
                           rdfs:comment "Ignore Dominate, Illusions, Obscure, or Telepathy being cast upon you."@en ;
                           rdfs:label "Mind Defense"@en .


###  https://raw.githubusercontent.com/AbsVahter/ontoTRPG/main/crown_and_skull/crown_and_skull.ttl#effect_spell_obscure
:effect_spell_obscure rdf:type owl:NamedIndividual ,
                               :EffectSpell ;
                      rdfs:comment "Hide objects. Use effect as penalty to detection rolls."@en ;
                      rdfs:label "Obscure"@en .


###  https://raw.githubusercontent.com/AbsVahter/ontoTRPG/main/crown_and_skull/crown_and_skull.ttl#effect_spell_perception
:effect_spell_perception rdf:type owl:NamedIndividual ,
                                  :EffectSpell ;
                         rdfs:comment "Add effect to a Scout or Investigate roll."@en ;
                         rdfs:label "Perception"@en .


###  https://raw.githubusercontent.com/AbsVahter/ontoTRPG/main/crown_and_skull/crown_and_skull.ttl#effect_spell_poison
:effect_spell_poison rdf:type owl:NamedIndividual ,
                              :EffectSpell ;
                     rdfs:comment "Conjure arcane goo or oil that inflicts poison on living things."@en ;
                     rdfs:label "Poison"@en .


###  https://raw.githubusercontent.com/AbsVahter/ontoTRPG/main/crown_and_skull/crown_and_skull.ttl#effect_spell_powerful
:effect_spell_powerful rdf:type owl:NamedIndividual ,
                                :EffectSpell ;
                       rdfs:comment "Boost a spell with a die upgrade, additional die, or similar."@en ;
                       rdfs:label "Powerful"@en .


###  https://raw.githubusercontent.com/AbsVahter/ontoTRPG/main/crown_and_skull/crown_and_skull.ttl#effect_spell_psychokinesis
:effect_spell_psychokinesis rdf:type owl:NamedIndividual ,
                                     :EffectSpell ;
                            rdfs:comment "Use the Muscle skill at distance of effect x 10 feet."@en ;
                            rdfs:label "Psychokinesis"@en .


###  https://raw.githubusercontent.com/AbsVahter/ontoTRPG/main/crown_and_skull/crown_and_skull.ttl#effect_spell_ranged
:effect_spell_ranged rdf:type owl:NamedIndividual ,
                              :EffectSpell ;
                     rdfs:comment "Cast up to long range and visible targets (most of a scene)."@en ;
                     rdfs:label "Ranged"@en .


###  https://raw.githubusercontent.com/AbsVahter/ontoTRPG/main/crown_and_skull/crown_and_skull.ttl#effect_spell_restore
:effect_spell_restore rdf:type owl:NamedIndividual ,
                               :EffectSpell ;
                      rdfs:comment "Heal 1 skill attrition."@en ;
                      rdfs:label "Restore"@en .


###  https://raw.githubusercontent.com/AbsVahter/ontoTRPG/main/crown_and_skull/crown_and_skull.ttl#effect_spell_shapechange
:effect_spell_shapechange rdf:type owl:NamedIndividual ,
                                   :EffectSpell ;
                          rdfs:comment "Change into a specified animal form."@en ;
                          rdfs:label "Shapechange"@en .


###  https://raw.githubusercontent.com/AbsVahter/ontoTRPG/main/crown_and_skull/crown_and_skull.ttl#effect_spell_shield
:effect_spell_shield rdf:type owl:NamedIndividual ,
                              :EffectSpell ;
                     rdfs:comment "Create a damage-absorbent magical barrier the size of a shield. It is impervious for 1 round and cannot be moved."@en ;
                     rdfs:label "Shield"@en .


###  https://raw.githubusercontent.com/AbsVahter/ontoTRPG/main/crown_and_skull/crown_and_skull.ttl#effect_spell_silent_spell
:effect_spell_silent_spell rdf:type owl:NamedIndividual ,
                                    :EffectSpell ;
                           rdfs:comment "Cast this spell with no magical words spoken."@en ;
                           rdfs:label "Silent Spell"@en .


###  https://raw.githubusercontent.com/AbsVahter/ontoTRPG/main/crown_and_skull/crown_and_skull.ttl#effect_spell_still
:effect_spell_still rdf:type owl:NamedIndividual ,
                             :EffectSpell ;
                    rdfs:comment "Cast this spell with no gestures."@en ;
                    rdfs:label "Still"@en .


###  https://raw.githubusercontent.com/AbsVahter/ontoTRPG/main/crown_and_skull/crown_and_skull.ttl#effect_spell_summon
:effect_spell_summon rdf:type owl:NamedIndividual ,
                              :EffectSpell ;
                     rdfs:comment "Conjure 1D6 1 attrition ‘minion’ creatures or constructs."@en ;
                     rdfs:label "Summon"@en .


###  https://raw.githubusercontent.com/AbsVahter/ontoTRPG/main/crown_and_skull/crown_and_skull.ttl#effect_spell_telepathy
:effect_spell_telepathy rdf:type owl:NamedIndividual ,
                                 :EffectSpell ;
                        rdfs:comment "Read minds by overcoming foe’s D20 roll with effect."@en ;
                        rdfs:label "Telepathy"@en .


###  https://raw.githubusercontent.com/AbsVahter/ontoTRPG/main/crown_and_skull/crown_and_skull.ttl#effect_spell_transmute
:effect_spell_transmute rdf:type owl:NamedIndividual ,
                                 :EffectSpell ;
                        rdfs:comment "Change a mass into a different material of equal or lesser value. Change effect x 10 pounds of mass."@en ;
                        rdfs:label "Transmute"@en .


###  https://raw.githubusercontent.com/AbsVahter/ontoTRPG/main/crown_and_skull/crown_and_skull.ttl#effect_spell_transport
:effect_spell_transport rdf:type owl:NamedIndividual ,
                                 :EffectSpell ;
                        rdfs:comment "Move a person from here to there instantly. Distance equal to effect x 10 feet."@en ;
                        rdfs:label "Transport"@en .


###  https://raw.githubusercontent.com/AbsVahter/ontoTRPG/main/crown_and_skull/crown_and_skull.ttl#effect_spell_vapor
:effect_spell_vapor rdf:type owl:NamedIndividual ,
                             :EffectSpell ;
                    rdfs:comment "Contain a spell’s effect in a lingering vapor cloud. The cloud is subject to air movement as a conventional gas."@en ;
                    rdfs:label "Vapor"@en .


###  https://raw.githubusercontent.com/AbsVahter/ontoTRPG/main/crown_and_skull/crown_and_skull.ttl#effect_spell_ward
:effect_spell_ward rdf:type owl:NamedIndividual ,
                            :EffectSpell ;
                   rdfs:comment "Prevent passage of a specified creature or person through a portal or passage."@en ;
                   rdfs:label "Ward"@en .


###  https://raw.githubusercontent.com/AbsVahter/ontoTRPG/main/crown_and_skull/crown_and_skull.ttl#encounter
:encounter rdf:type owl:NamedIndividual ;
           rdfs:label "Encounter"@en ;
           gen:included :phases_and_rounds ,
                        :recovery ,
                        :setting_scene ,
                        :transitions_and_table_talk .


###  https://raw.githubusercontent.com/AbsVahter/ontoTRPG/main/crown_and_skull/crown_and_skull.ttl#equipment
:equipment rdf:type owl:NamedIndividual ,
                    gen:ParameterPC ;
           rdfs:comment "format = {item: status (carried, worn, crossed) }"@en ;
           rdfs:label "Equipment"@en .


###  https://raw.githubusercontent.com/AbsVahter/ontoTRPG/main/crown_and_skull/crown_and_skull.ttl#eye_in_well
:eye_in_well rdf:type owl:NamedIndividual ;
             rdfs:comment "As Slimshire faces the challenges of a full-fledged city, darkness has entered the dreams of its people. The dream is always the same: descending into a pit of wet stone, beyond the lightless water, deeper, darker, until a single yellowish eye opens in the murk. The dread of this dream-intrusion is slowly growing in Slimshire, but its nature, origin, and solution are completely unknown. Some doomsayers claim the goblinorc alliance and the eye are somehow connected..."@en ;
             rdfs:label "The Eye in the Well"@en ;
             gen:Location :slimshire .


###  https://raw.githubusercontent.com/AbsVahter/ontoTRPG/main/crown_and_skull/crown_and_skull.ttl#first_aid
:first_aid rdf:type owl:NamedIndividual ;
           rdfs:comment "restore 1 crossed-off skill" ;
           rdfs:label "First-aid"@en ;
           gen:modified :skills ;
           gen:target "ally in touch distance" ;
           gen:valueFormula "1 skill crossed -> non-crossed" .


###  https://raw.githubusercontent.com/AbsVahter/ontoTRPG/main/crown_and_skull/crown_and_skull.ttl#first_aid_failed
:first_aid_failed rdf:type owl:NamedIndividual ;
                  rdfs:comment "skill recoverable only by rest" ;
                  rdfs:label "Failed first-aid"@en ;
                  gen:modified :skills ;
                  gen:target "ally in touch distance" ;
                  gen:valueFormula "1 skill crossed -> recoverable only by rest" .


###  https://raw.githubusercontent.com/AbsVahter/ontoTRPG/main/crown_and_skull/crown_and_skull.ttl#flaw_addict
:flaw_addict rdf:type owl:NamedIndividual ,
                      :FlawBasic ;
             rdfs:comment "You have a specific vice you cannot deny. If you can’t get your fix, the GM will ask for a roll vs. attrition in some form."@en ;
             rdfs:label "Addict flaw"@en .


###  https://raw.githubusercontent.com/AbsVahter/ontoTRPG/main/crown_and_skull/crown_and_skull.ttl#flaw_aescetic
:flaw_aescetic rdf:type owl:NamedIndividual ,
                        :FlawBasic ;
               rdfs:comment "You frown on possessions. Never exceed 5 equipment."@en ;
               rdfs:label "Aescetic flaw"@en ;
               gen:modified :SetAdditiveEquipment ;
               gen:valueFormula "prerequisite -> (final number of equipment <= 5)" ;
               gen:valueObject gen:prerequisiteDescription .


###  https://raw.githubusercontent.com/AbsVahter/ontoTRPG/main/crown_and_skull/crown_and_skull.ttl#flaw_ancient
:flaw_ancient rdf:type owl:NamedIndividual ,
                       :FlawBasic ;
              rdfs:comment "You are old! Muscle, Jump, Climber, Breakfall, and Stealth skills may not exceed 9, but you earn respect for your advanced age."@en ;
              rdfs:label "Ancient flaw"@en ;
              gen:modified :SetAdditiveSkill ;
              gen:valueFormula "prerequisite -> ((final number of skills <= 10) and (final skill level >= 3) and (final skill level <= 9))" ;
              gen:valueObject :skill_breakfall ,
                              :skill_climber ,
                              :skill_jump ,
                              :skill_muscle ,
                              :skill_stealth ,
                              gen:prerequisiteDescription .


###  https://raw.githubusercontent.com/AbsVahter/ontoTRPG/main/crown_and_skull/crown_and_skull.ttl#flaw_bad_reputation
:flaw_bad_reputation rdf:type owl:NamedIndividual ,
                              :FlawBasic ;
                     rdfs:comment "You’ve done things... terrible things, and people know about it. You’ve done harm, broken oaths, or let someone down."@en ;
                     rdfs:label "Bad reputation flaw"@en .


###  https://raw.githubusercontent.com/AbsVahter/ontoTRPG/main/crown_and_skull/crown_and_skull.ttl#flaw_crazy
:flaw_crazy rdf:type owl:NamedIndividual ,
                     :FlawBasic ;
            rdfs:comment "When faced with a diffi cult choice, choose randomly."@en ;
            rdfs:label "Crazy flaw"@en .


###  https://raw.githubusercontent.com/AbsVahter/ontoTRPG/main/crown_and_skull/crown_and_skull.ttl#flaw_crown_sworn
:flaw_crown_sworn rdf:type owl:NamedIndividual ,
                           :FlawCrownAndSkull ;
                  rdfs:comment "If you disobey a royal summons, edict or order and are caught doing so, the penalty is death."@en ;
                  rdfs:label "Crown-Sworn flaw"@en .


###  https://raw.githubusercontent.com/AbsVahter/ontoTRPG/main/crown_and_skull/crown_and_skull.ttl#flaw_disorganized
:flaw_disorganized rdf:type owl:NamedIndividual ,
                            :FlawBasic ;
                   rdfs:comment "Where’d you put that? When seeking anything but your most-used items and armor, roll 9 or less on a D20 to find it."@en ;
                   rdfs:label "Disorganized flaw"@en .


###  https://raw.githubusercontent.com/AbsVahter/ontoTRPG/main/crown_and_skull/crown_and_skull.ttl#flaw_drunkard
:flaw_drunkard rdf:type owl:NamedIndividual ,
                        :FlawBasic ;
               rdfs:comment "Your drinking wavers between revelry and tomfoolery. Beer and wine drain your pockets and frustrate your friends."@en ;
               rdfs:label "Drunkard flaw"@en .


###  https://raw.githubusercontent.com/AbsVahter/ontoTRPG/main/crown_and_skull/crown_and_skull.ttl#flaw_employed
:flaw_employed rdf:type owl:NamedIndividual ,
                        :FlawBasic ;
               rdfs:comment "You are paid or oathsworn to a lord or employer. Disobey at your own peril!"@en ;
               rdfs:label "Employed flaw"@en .


###  https://raw.githubusercontent.com/AbsVahter/ontoTRPG/main/crown_and_skull/crown_and_skull.ttl#flaw_greedy
:flaw_greedy rdf:type owl:NamedIndividual ,
                      :FlawBasic ;
             rdfs:comment "Tempted by treasure, roll 6 or less on a D20 to resist the urge."@en ;
             rdfs:label "Greedy flaw"@en .


###  https://raw.githubusercontent.com/AbsVahter/ontoTRPG/main/crown_and_skull/crown_and_skull.ttl#flaw_grudge
:flaw_grudge rdf:type owl:NamedIndividual ,
                      :FlawBasic ;
             rdfs:comment "You have been wronged, and hold it against an individual or group, unjustly. When you encounter them, you behave terribly."@en ;
             rdfs:label "Grudge flaw"@en .


###  https://raw.githubusercontent.com/AbsVahter/ontoTRPG/main/crown_and_skull/crown_and_skull.ttl#flaw_impetuous
:flaw_impetuous rdf:type owl:NamedIndividual ,
                         :FlawBasic ;
                rdfs:comment "You are impatient, leaping into situations without planning or reservation. Only take action in phase 1 or 2."@en ;
                rdfs:label "Impetuous flaw"@en ;
                gen:modified :phase_choose ;
                gen:valueFormula "1..5 -> 1..2" ;
                gen:valueObject gen:valueFormula .


###  https://raw.githubusercontent.com/AbsVahter/ontoTRPG/main/crown_and_skull/crown_and_skull.ttl#flaw_injured
:flaw_injured rdf:type owl:NamedIndividual ,
                       :FlawBasic ;
              rdfs:comment "This common flaw should be taken a few times in a character’s lifetime. An Injury brings a -1 maximum skill inventory."@en ;
              rdfs:label "Injured flaw"@en ;
              gen:modified :SetAdditiveSkill ;
              gen:valueFormula "prerequisite += (final number of skills - 1)" ;
              gen:valueObject gen:prerequisiteDescription .


###  https://raw.githubusercontent.com/AbsVahter/ontoTRPG/main/crown_and_skull/crown_and_skull.ttl#flaw_just_a_kid
:flaw_just_a_kid rdf:type owl:NamedIndividual ,
                          :FlawBasic ;
                 rdfs:comment "Hey, I’m just a kid! Never exceed 6 skills."@en ;
                 rdfs:label "Just a kid flaw"@en ;
                 gen:modified :SetAdditiveSkill ;
                 gen:valueFormula "prerequisite -> ((final number of skills <= 6) and (final skill level >= 3) and (final skill level <= 9))" ;
                 gen:valueObject gen:prerequisiteDescription .


###  https://raw.githubusercontent.com/AbsVahter/ontoTRPG/main/crown_and_skull/crown_and_skull.ttl#flaw_paranoid
:flaw_paranoid rdf:type owl:NamedIndividual ,
                        :FlawBasic ;
               rdfs:comment "What’s that? You hear that? You invent your own boogie men, and sew doubt among others. NPCs will be hesitant to trust you."@en ;
               rdfs:label "Paranoid flaw"@en .


###  https://raw.githubusercontent.com/AbsVahter/ontoTRPG/main/crown_and_skull/crown_and_skull.ttl#flaw_phobia
:flaw_phobia rdf:type owl:NamedIndividual ,
                      :FlawBasic ;
             rdfs:comment "Fear of a common thing. In its presence, no roll can succeed."@en ;
             rdfs:label "Phobia flaw"@en ;
             gen:modified :check_skill_resist_vs_horror ;
             gen:valueFormula "success -> fail" ;
             gen:valueObject gen:effect .


###  https://raw.githubusercontent.com/AbsVahter/ontoTRPG/main/crown_and_skull/crown_and_skull.ttl#flaw_pursued
:flaw_pursued rdf:type owl:NamedIndividual ,
                       :FlawBasic ;
              rdfs:comment "You have a nemesis out there... somewhere... hunting you."@en ;
              rdfs:label "Pursued flaw"@en .


###  https://raw.githubusercontent.com/AbsVahter/ontoTRPG/main/crown_and_skull/crown_and_skull.ttl#flaw_ronin
:flaw_ronin rdf:type owl:NamedIndividual ,
                     :FlawCrownAndSkull ;
            rdfs:comment "Unless in disguise, you will be identifi ed and unwelcome in any high hall, throne room, council chamber, or royal household. Even in taverns and markets you will be seen as suspicious."@en ;
            rdfs:label "Ronin flaw"@en .


###  https://raw.githubusercontent.com/AbsVahter/ontoTRPG/main/crown_and_skull/crown_and_skull.ttl#flaw_sickly
:flaw_sickly rdf:type owl:NamedIndividual ,
                      :FlawBasic ;
             rdfs:comment "You were born frail. Survival and Resist skills cannot exceed 9."@en ;
             rdfs:label "Sickly flaw"@en ;
             gen:modified :SetAdditiveSkill ;
             gen:valueFormula "prerequisite -> ((final number of skills <= 10) and (final skill level >= 3) and (final skill level <= 9))" ;
             gen:valueObject :skill_resist ,
                             :skill_survival ,
                             gen:prerequisiteDescription .


###  https://raw.githubusercontent.com/AbsVahter/ontoTRPG/main/crown_and_skull/crown_and_skull.ttl#flaw_stubborn
:flaw_stubborn rdf:type owl:NamedIndividual ,
                        :FlawBasic ;
               rdfs:comment "If you make up your mind, only a D20 contest with another player or NPC will sway you."@en ;
               rdfs:label "Stubborn flaw"@en .


###  https://raw.githubusercontent.com/AbsVahter/ontoTRPG/main/crown_and_skull/crown_and_skull.ttl#flaw_timid
:flaw_timid rdf:type owl:NamedIndividual ,
                     :FlawBasic ;
            rdfs:comment "You’d rather let others lead. Only take action in phase 4 or 5."@en ;
            rdfs:label "Timid flaw"@en ;
            gen:modified :phase_choose ;
            gen:valueFormula "1..5 -> 4..5" ;
            gen:valueObject gen:valueFormula .


###  https://raw.githubusercontent.com/AbsVahter/ontoTRPG/main/crown_and_skull/crown_and_skull.ttl#flaw_unlucky
:flaw_unlucky rdf:type owl:NamedIndividual ,
                       :FlawBasic ;
              rdfs:comment "No matter how many rabbit’s feet you carry, you have a penchant for comical mishaps and crit fail on a 16+."@en ;
              rdfs:label "Unlucky flaw"@en .


###  https://raw.githubusercontent.com/AbsVahter/ontoTRPG/main/crown_and_skull/crown_and_skull.ttl#flaws
:flaws rdf:type owl:NamedIndividual ,
                gen:ParameterPC ;
       rdfs:comment "format = list"@en ;
       rdfs:label "Flaws"@en .


###  https://raw.githubusercontent.com/AbsVahter/ontoTRPG/main/crown_and_skull/crown_and_skull.ttl#formless_evil
:formless_evil rdf:type owl:NamedIndividual ,
                        gen:Event ;
               rdfs:comment "It is not fully understood, but the dreams of mortal folk are darkening. Rumor holds that the lord of Blood Manor is somehow behind this growing shadow."@en ;
               rdfs:label "A formless evil"@en ;
               gen:Actor :lord_loyce ;
               gen:Location :north_holds ;
               gen:after :bloodwing_war .


###  https://raw.githubusercontent.com/AbsVahter/ontoTRPG/main/crown_and_skull/crown_and_skull.ttl#freezing_entire_day
:freezing_entire_day rdf:type owl:NamedIndividual ;
                     rdfs:comment "your blood will go to ice, killing you slowly"@en ;
                     rdfs:label "Freezing entire day"@en ;
                     gen:prerequisite :status_freezing ;
                     gen:prerequisiteDescription "duration of freezing = entire day" ;
                     gen:set gen:death .


###  https://raw.githubusercontent.com/AbsVahter/ontoTRPG/main/crown_and_skull/crown_and_skull.ttl#frothy_mare
:frothy_mare rdf:type owl:NamedIndividual ,
                      gen:Location ;
             rdfs:comment "One of the most famous (or infamous) taverns in the realm calls Rivergate home: The Frothy Mare. This chaotic, multi-level inn, eatery and house of revelry serves as a meeting point for all kinds of river folk, known for its cheese-sausages and dwarven ale by the gallon. The lead barkeep is a red-mustached stout fellow called Barmm."@en ;
             rdfs:label "The Frothy Mare"@en .


###  https://raw.githubusercontent.com/AbsVahter/ontoTRPG/main/crown_and_skull/crown_and_skull.ttl#gardenburrow
:gardenburrow rdf:type owl:NamedIndividual ,
                       gen:Location ;
              rdfs:comment "In the far west, the elven forest town of Gardenburrow serves as a waypost for the borders of Thryn. The town itself is on a small rise, with wooden fortifi cations, and a great central oak tree that serves as the town square."@en ;
              rdfs:label "Gardenburrow, Forest Refuge"@en ;
              gen:included :suede_and_saddle .


###  https://raw.githubusercontent.com/AbsVahter/ontoTRPG/main/crown_and_skull/crown_and_skull.ttl#gardenburrow_residents
:gardenburrow_residents rdf:type owl:NamedIndividual ;
                        rdfs:label "Residents of Gardenburrow"@en ;
                        gen:Actor :alderman_wallaby ,
                                  :selene ;
                        gen:Location :gardenburrow .


###  https://raw.githubusercontent.com/AbsVahter/ontoTRPG/main/crown_and_skull/crown_and_skull.ttl#gardenburrow_threat
:gardenburrow_threat rdf:type owl:NamedIndividual ;
                     rdfs:comment "In recent years, a shadow has been spreading through the Oakenwood. Crops are failing, elder trees are withering away. Frogman defectors, venturing here from the marshes, believe the problem demands a new alliance. Can the heroes make friends of the cruel frog-kin and heal the forest? A council is called in the town longhouse. Something must be done."@en ;
                     rdfs:label "Threat at Gardenburrow"@en ;
                     gen:Location :gardenburrow .


###  https://raw.githubusercontent.com/AbsVahter/ontoTRPG/main/crown_and_skull/crown_and_skull.ttl#giving_hero_coin
:giving_hero_coin rdf:type owl:NamedIndividual ;
                  rdfs:label "Giving hero coin to other player"@en ;
                  gen:Actor gen:player ;
                  gen:cost "1" ;
                  gen:resource :hero_coin ;
                  gen:set :hero_coin ;
                  gen:target "other player" ;
                  gen:valueNumeric 1 .


###  https://raw.githubusercontent.com/AbsVahter/ontoTRPG/main/crown_and_skull/crown_and_skull.ttl#halving_fall_damage
:halving_fall_damage rdf:type owl:NamedIndividual ;
                     rdfs:label "Half damage taken in long falls"@en .


###  https://raw.githubusercontent.com/AbsVahter/ontoTRPG/main/crown_and_skull/crown_and_skull.ttl#healing
:healing rdf:type owl:NamedIndividual ;
         rdfs:comment "restore 1 crossed-off skill" ;
         rdfs:label "Healing"@en ;
         gen:modified :skills ;
         gen:prerequisiteDescription "magic, potion" ;
         gen:valueFormula "1 skill crossed -> non-crossed" .


###  https://raw.githubusercontent.com/AbsVahter/ontoTRPG/main/crown_and_skull/crown_and_skull.ttl#hero_coin
:hero_coin rdf:type owl:NamedIndividual ,
                    gen:ParameterPC ;
           rdfs:label "Hero coin"@en .


###  https://raw.githubusercontent.com/AbsVahter/ontoTRPG/main/crown_and_skull/crown_and_skull.ttl#hero_points
:hero_points rdf:type owl:NamedIndividual ,
                      gen:ParameterPC ;
             rdfs:comment """
format = (current value, earned value) ;
current value used as resource ;
earned value is always increased except for PC creation ;
"""@en ;
             rdfs:label "Hero points"@en .


###  https://raw.githubusercontent.com/AbsVahter/ontoTRPG/main/crown_and_skull/crown_and_skull.ttl#hometown
:hometown rdf:type owl:NamedIndividual ,
                   gen:ParameterPC ;
          rdfs:label "Hometown"@en .


###  https://raw.githubusercontent.com/AbsVahter/ontoTRPG/main/crown_and_skull/crown_and_skull.ttl#hometown_bonus
:hometown_bonus rdf:type owl:NamedIndividual ;
                rdfs:label "Hometown bonus for hero points"@en .


###  https://raw.githubusercontent.com/AbsVahter/ontoTRPG/main/crown_and_skull/crown_and_skull.ttl#hurry
:hurry rdf:type owl:NamedIndividual ;
       rdfs:comment "If you need to move AND do something in one turn, your haste opens up your Defenses with clumsy haste."@en ;
       rdfs:label "Hurry"@en ;
       gen:effect :move ,
                  :perform_action ;
       gen:prerequisiteDescription "move+action combo" ;
       gen:set :status_vs_haste ;
       gen:target "foes in the scene" .


###  https://raw.githubusercontent.com/AbsVahter/ontoTRPG/main/crown_and_skull/crown_and_skull.ttl#item_backpack
:item_backpack rdf:type owl:NamedIndividual ,
                        :ItemBasic ;
               rdfs:comment "Carry 2 additional items"@en ;
               rdfs:label "Backpack"@en ;
               gen:cost "6 hero points" .


###  https://raw.githubusercontent.com/AbsVahter/ontoTRPG/main/crown_and_skull/crown_and_skull.ttl#item_bandage_kit
:item_bandage_kit rdf:type owl:NamedIndividual ,
                           :ItemBasic ;
                  rdfs:comment "3 count, heal 1 crossed off skill"@en ;
                  rdfs:label "Bandage Kit"@en ,
                             "Bandage kit"@en ;
                  gen:cost "3 hero points" ;
                  gen:effect :block_status_bleed .


###  https://raw.githubusercontent.com/AbsVahter/ontoTRPG/main/crown_and_skull/crown_and_skull.ttl#item_barbed_whip
:item_barbed_whip rdf:type owl:NamedIndividual ,
                           :ItemWeapon ;
                  rdfs:comment "Induces bleed on target"@en ;
                  rdfs:label "Barbed Whip"@en ;
                  gen:cost "5 hero points" ;
                  gen:damage "1d8" .


###  https://raw.githubusercontent.com/AbsVahter/ontoTRPG/main/crown_and_skull/crown_and_skull.ttl#item_battle_axe
:item_battle_axe rdf:type owl:NamedIndividual ,
                          :ItemWeapon ;
                 rdfs:comment "Ignore 2 target DEF"@en ;
                 rdfs:label "Battle Axe"@en ;
                 gen:cost "5 hero points" ;
                 gen:damage "1d12" .


###  https://raw.githubusercontent.com/AbsVahter/ontoTRPG/main/crown_and_skull/crown_and_skull.ttl#item_bear_trap
:item_bear_trap rdf:type owl:NamedIndividual ,
                         :ItemBasic ;
                rdfs:comment "1 count, Muscle to escape"@en ;
                rdfs:label "Bear Trap"@en ;
                gen:cost "2 hero points" .


###  https://raw.githubusercontent.com/AbsVahter/ontoTRPG/main/crown_and_skull/crown_and_skull.ttl#item_blessed_water
:item_blessed_water rdf:type owl:NamedIndividual ,
                             :ItemBasic ;
                    rdfs:comment "3 uses, anathema to pure evil or the undead"@en ;
                    rdfs:label "Blessed Water"@en ;
                    gen:cost "3 hero points" .


###  https://raw.githubusercontent.com/AbsVahter/ontoTRPG/main/crown_and_skull/crown_and_skull.ttl#item_caltrops
:item_caltrops rdf:type owl:NamedIndividual ,
                        :ItemBasic ;
               rdfs:comment "3 uses, spiked floor-scatter, inflicts D4"@en ;
               rdfs:label "Caltrops"@en ;
               gen:cost "1 hero point" .


###  https://raw.githubusercontent.com/AbsVahter/ontoTRPG/main/crown_and_skull/crown_and_skull.ttl#item_cart
:item_cart rdf:type owl:NamedIndividual ,
                    :ItemLarge ;
           rdfs:comment "Holds crates and barrels filled with goods"@en ;
           rdfs:label "Cart"@en ;
           gen:cost "10 hero points" .


###  https://raw.githubusercontent.com/AbsVahter/ontoTRPG/main/crown_and_skull/crown_and_skull.ttl#item_castle
:item_castle rdf:type owl:NamedIndividual ,
                      :ItemLarge ;
             rdfs:comment "A series of keeps and towers, stone"@en ;
             rdfs:label "Castle"@en ;
             gen:cost "200 hero points" .


###  https://raw.githubusercontent.com/AbsVahter/ontoTRPG/main/crown_and_skull/crown_and_skull.ttl#item_chain_mail
:item_chain_mail rdf:type owl:NamedIndividual ,
                          :ItemArmor ;
                 rdfs:comment "Noisy"@en ;
                 rdfs:label "Chain Mail"@en ;
                 gen:cost "3 hero points" ;
                 gen:defense "+3" .


###  https://raw.githubusercontent.com/AbsVahter/ontoTRPG/main/crown_and_skull/crown_and_skull.ttl#item_chest_plate
:item_chest_plate rdf:type owl:NamedIndividual ,
                           :ItemArmor ;
                  rdfs:comment "-3 Stealth skill, cannot swim"@en ;
                  rdfs:label "Chest Plate"@en ;
                  gen:cost "5 hero points" ;
                  gen:defense "+4" .


###  https://raw.githubusercontent.com/AbsVahter/ontoTRPG/main/crown_and_skull/crown_and_skull.ttl#item_climbing_gear
:item_climbing_gear rdf:type owl:NamedIndividual ,
                             :ItemBasic ;
                    rdfs:comment "Ignore penalties on Climbing rolls"@en ;
                    rdfs:label "Climbing Gear"@en ;
                    gen:cost "1 hero point" .


###  https://raw.githubusercontent.com/AbsVahter/ontoTRPG/main/crown_and_skull/crown_and_skull.ttl#item_cloak
:item_cloak rdf:type owl:NamedIndividual ,
                     :ItemArmor ;
            rdfs:comment "+3 Stealth skill"@en ;
            rdfs:label "Cloak"@en ;
            gen:cost "1 hero point" ;
            gen:defense "+1" .


###  https://raw.githubusercontent.com/AbsVahter/ontoTRPG/main/crown_and_skull/crown_and_skull.ttl#item_cold_weather_fur
:item_cold_weather_fur rdf:type owl:NamedIndividual ,
                                :ItemBasic ;
                       rdfs:comment "Ignore penalties from normal cold or snow"@en ;
                       rdfs:label "Cold Weather Fur"@en ;
                       gen:cost "1 hero point" .


###  https://raw.githubusercontent.com/AbsVahter/ontoTRPG/main/crown_and_skull/crown_and_skull.ttl#item_craftsmans_tools
:item_craftsmans_tools rdf:type owl:NamedIndividual ,
                                :ItemBasic ;
                       rdfs:comment "Hammer, spanner, and bits for simple work"@en ;
                       rdfs:label "Craftsman’s Tools"@en ;
                       gen:cost "1 hero point" .


###  https://raw.githubusercontent.com/AbsVahter/ontoTRPG/main/crown_and_skull/crown_and_skull.ttl#item_crossbow
:item_crossbow rdf:type owl:NamedIndividual ,
                        :ItemWeapon ;
               rdfs:comment "Takes 1 round to reload"@en ;
               rdfs:label "Crossbow"@en ;
               gen:cost "5 hero points" ;
               gen:damage "1d10" .


###  https://raw.githubusercontent.com/AbsVahter/ontoTRPG/main/crown_and_skull/crown_and_skull.ttl#item_custom
:item_custom rdf:type owl:NamedIndividual ,
                      :Item ;
             rdfs:label "Custom item"@en .


###  https://raw.githubusercontent.com/AbsVahter/ontoTRPG/main/crown_and_skull/crown_and_skull.ttl#item_dagger
:item_dagger rdf:type owl:NamedIndividual ,
                      :ItemWeapon ;
             rdfs:comment "Conceal, thrown"@en ;
             rdfs:label "Dagger"@en ;
             gen:cost "1 hero point" ;
             gen:damage "1d4" .


###  https://raw.githubusercontent.com/AbsVahter/ontoTRPG/main/crown_and_skull/crown_and_skull.ttl#item_diving_gear
:item_diving_gear rdf:type owl:NamedIndividual ,
                           :ItemBasic ;
                  rdfs:comment "2 dive helms, spearguns, fins, marker buoy"@en ;
                  rdfs:label "Diving Gear"@en ;
                  gen:cost "1 hero point" .


###  https://raw.githubusercontent.com/AbsVahter/ontoTRPG/main/crown_and_skull/crown_and_skull.ttl#item_flint_and_steel
:item_flint_and_steel rdf:type owl:NamedIndividual ,
                               :ItemBasic ;
                      rdfs:comment "Camp with comfort and cozy fire"@en ;
                      rdfs:label "Flint & Steel"@en ;
                      gen:cost "1 hero point" .


###  https://raw.githubusercontent.com/AbsVahter/ontoTRPG/main/crown_and_skull/crown_and_skull.ttl#item_flint_pistol
:item_flint_pistol rdf:type owl:NamedIndividual ,
                            :ItemWeapon ;
                   rdfs:comment "Concealed, 1d6 phases to reload"@en ;
                   rdfs:label "Flint Pistol"@en ;
                   gen:cost "7 hero points" ;
                   gen:damage "1d10" .


###  https://raw.githubusercontent.com/AbsVahter/ontoTRPG/main/crown_and_skull/crown_and_skull.ttl#item_fort_garrison
:item_fort_garrison rdf:type owl:NamedIndividual ,
                             :ItemLarge ;
                    rdfs:comment "A wooden defense position with pole-fences"@en ;
                    rdfs:label "Fort or Garrison"@en ;
                    gen:cost "75 hero points" .


###  https://raw.githubusercontent.com/AbsVahter/ontoTRPG/main/crown_and_skull/crown_and_skull.ttl#item_fortress
:item_fortress rdf:type owl:NamedIndividual ,
                        :ItemLarge ;
               rdfs:comment "A massive, impregnable castle on a cliff"@en ;
               rdfs:label "Fortress"@en ;
               gen:cost "300 hero points" .


###  https://raw.githubusercontent.com/AbsVahter/ontoTRPG/main/crown_and_skull/crown_and_skull.ttl#item_great_sword
:item_great_sword rdf:type owl:NamedIndividual ,
                           :ItemWeapon ;
                  rdfs:comment "Uses 2 hands"@en ;
                  rdfs:label "Great Sword"@en ;
                  gen:cost "3 hero points" ;
                  gen:damage "1d10" .


###  https://raw.githubusercontent.com/AbsVahter/ontoTRPG/main/crown_and_skull/crown_and_skull.ttl#item_greaves
:item_greaves rdf:type owl:NamedIndividual ,
                       :ItemArmor ;
              rdfs:comment "Boots with armored shins"@en ;
              rdfs:label "Greaves"@en ;
              gen:cost "1 hero point" ;
              gen:defense "+1" .


###  https://raw.githubusercontent.com/AbsVahter/ontoTRPG/main/crown_and_skull/crown_and_skull.ttl#item_halberd
:item_halberd rdf:type owl:NamedIndividual ,
                       :ItemWeapon ;
              rdfs:comment "Long reach, halt a target’s progress"@en ;
              rdfs:label "Halberd"@en ;
              gen:cost "3 hero points" ;
              gen:damage "1d10" .


###  https://raw.githubusercontent.com/AbsVahter/ontoTRPG/main/crown_and_skull/crown_and_skull.ttl#item_helm
:item_helm rdf:type owl:NamedIndividual ,
                    :ItemArmor ;
           rdfs:comment "Draws enemy attention"@en ;
           rdfs:label "Helm"@en ;
           gen:cost "1 hero point" ;
           gen:defense "+1" .


###  https://raw.githubusercontent.com/AbsVahter/ontoTRPG/main/crown_and_skull/crown_and_skull.ttl#item_holy_symbol
:item_holy_symbol rdf:type owl:NamedIndividual ,
                           :Item ;
                  rdfs:label "Holy symbol"@en .


###  https://raw.githubusercontent.com/AbsVahter/ontoTRPG/main/crown_and_skull/crown_and_skull.ttl#item_horse
:item_horse rdf:type owl:NamedIndividual ,
                     :ItemLarge ;
            rdfs:comment "Transports 2 people at 4x walking speed"@en ;
            rdfs:label "Horse"@en ;
            gen:cost "5 hero points" .


###  https://raw.githubusercontent.com/AbsVahter/ontoTRPG/main/crown_and_skull/crown_and_skull.ttl#item_house
:item_house rdf:type owl:NamedIndividual ,
                     :ItemLarge ;
            rdfs:comment "A cozy place to live, deed for life"@en ;
            rdfs:label "House"@en ;
            gen:cost "50 hero points" .


###  https://raw.githubusercontent.com/AbsVahter/ontoTRPG/main/crown_and_skull/crown_and_skull.ttl#item_iron_chain
:item_iron_chain rdf:type owl:NamedIndividual ,
                          :ItemBasic ;
                 rdfs:comment "15’ length, all but unbreakable"@en ;
                 rdfs:label "Iron Chain"@en ;
                 gen:cost "1 hero point" .


###  https://raw.githubusercontent.com/AbsVahter/ontoTRPG/main/crown_and_skull/crown_and_skull.ttl#item_leather_vest
:item_leather_vest rdf:type owl:NamedIndividual ,
                            :ItemArmor ;
                   rdfs:comment "No protection against blunt force"@en ;
                   rdfs:label "Leather Vest"@en ;
                   gen:cost "2 hero points" ;
                   gen:defense "+2" .


###  https://raw.githubusercontent.com/AbsVahter/ontoTRPG/main/crown_and_skull/crown_and_skull.ttl#item_lockpicks
:item_lockpicks rdf:type owl:NamedIndividual ,
                         :ItemBasic ;
                rdfs:comment "Cannot pick locks without these tools"@en ;
                rdfs:label "Lockpicks"@en ;
                gen:cost "1 hero point" .


###  https://raw.githubusercontent.com/AbsVahter/ontoTRPG/main/crown_and_skull/crown_and_skull.ttl#item_long_bow
:item_long_bow rdf:type owl:NamedIndividual ,
                        :ItemWeapon ;
               rdfs:comment "On max damage, fire again"@en ;
               rdfs:label "Long Bow"@en ;
               gen:cost "3 hero points" ;
               gen:damage "1d8" .


###  https://raw.githubusercontent.com/AbsVahter/ontoTRPG/main/crown_and_skull/crown_and_skull.ttl#item_long_sword
:item_long_sword rdf:type owl:NamedIndividual ,
                          :ItemWeapon ;
                 rdfs:comment "If max damage, roll again"@en ;
                 rdfs:label "Long Sword"@en ;
                 gen:cost "2 hero points" ;
                 gen:damage "1d8" .


###  https://raw.githubusercontent.com/AbsVahter/ontoTRPG/main/crown_and_skull/crown_and_skull.ttl#item_mast_ship
:item_mast_ship rdf:type owl:NamedIndividual ,
                         :ItemLarge ;
                rdfs:comment "Crew of 3 required, 2 masts, huge hold"@en ;
                rdfs:label "Mast Ship"@en ;
                gen:cost "35 hero points" .


###  https://raw.githubusercontent.com/AbsVahter/ontoTRPG/main/crown_and_skull/crown_and_skull.ttl#item_mining_kit
:item_mining_kit rdf:type owl:NamedIndividual ,
                          :ItemBasic ;
                 rdfs:comment "Exploring or excavation times cut in half"@en ;
                 rdfs:label "Mining Kit"@en ;
                 gen:cost "1 hero point" .


###  https://raw.githubusercontent.com/AbsVahter/ontoTRPG/main/crown_and_skull/crown_and_skull.ttl#item_musket
:item_musket rdf:type owl:NamedIndividual ,
                      :ItemWeapon ;
             rdfs:comment "Heard for miles, 1d6 phases to reload"@en ;
             rdfs:label "Musket"@en ;
             gen:cost "7 hero points" ;
             gen:damage "1d12" .


###  https://raw.githubusercontent.com/AbsVahter/ontoTRPG/main/crown_and_skull/crown_and_skull.ttl#item_oil_flask
:item_oil_flask rdf:type owl:NamedIndividual ,
                         :ItemBasic ;
                rdfs:comment "3 count, flammable liquid, glass phial"@en ;
                rdfs:label "Oil Flask"@en ;
                gen:cost "1 hero point" .


###  https://raw.githubusercontent.com/AbsVahter/ontoTRPG/main/crown_and_skull/crown_and_skull.ttl#item_pick_hammer
:item_pick_hammer rdf:type owl:NamedIndividual ,
                           :ItemWeapon ;
                  rdfs:comment "Reduce target armor by 1 per hit"@en ;
                  rdfs:label "Pick Hammer"@en ;
                  gen:cost "2 hero points" ;
                  gen:damage "1d6" .


###  https://raw.githubusercontent.com/AbsVahter/ontoTRPG/main/crown_and_skull/crown_and_skull.ttl#item_powder_kit
:item_powder_kit rdf:type owl:NamedIndividual ,
                          :ItemBasic ;
                 rdfs:comment "1 Firearm never empty, ruined if wet"@en ;
                 rdfs:label "Powder Kit"@en ;
                 gen:cost "3 hero points" .


###  https://raw.githubusercontent.com/AbsVahter/ontoTRPG/main/crown_and_skull/crown_and_skull.ttl#item_rope
:item_rope rdf:type owl:NamedIndividual ,
                    :ItemBasic ;
           rdfs:comment "50’ length, breaks on crit fail usage"@en ;
           rdfs:label "Rope"@en ;
           gen:cost "1 hero point" .


###  https://raw.githubusercontent.com/AbsVahter/ontoTRPG/main/crown_and_skull/crown_and_skull.ttl#item_sack_of_bearings
:item_sack_of_bearings rdf:type owl:NamedIndividual ,
                                :ItemBasic ;
                       rdfs:comment "A pouch of 3 dozen metal balls"@en ;
                       rdfs:label "Sack of Bearings"@en ;
                       gen:cost "1 hero point" .


###  https://raw.githubusercontent.com/AbsVahter/ontoTRPG/main/crown_and_skull/crown_and_skull.ttl#item_scale_vest
:item_scale_vest rdf:type owl:NamedIndividual ,
                          :ItemArmor ;
                 rdfs:comment "Rare/requires expert blacksmith"@en ;
                 rdfs:label "Scale Vest"@en ;
                 gen:cost "3 hero points" ;
                 gen:defense "+3" .


###  https://raw.githubusercontent.com/AbsVahter/ontoTRPG/main/crown_and_skull/crown_and_skull.ttl#item_scimitar
:item_scimitar rdf:type owl:NamedIndividual ,
                        :ItemWeapon ;
               rdfs:comment "On max damage, attack another target"@en ;
               rdfs:label "Scimitar"@en ;
               gen:cost "5 hero points" ;
               gen:damage "1d8" .


###  https://raw.githubusercontent.com/AbsVahter/ontoTRPG/main/crown_and_skull/crown_and_skull.ttl#item_scribes_kit
:item_scribes_kit rdf:type owl:NamedIndividual ,
                           :ItemBasic ;
                  rdfs:comment "Parchment book, charcoal sticks"@en ;
                  rdfs:label "Scribe’s Kit"@en ;
                  gen:cost "1 hero point" .


###  https://raw.githubusercontent.com/AbsVahter/ontoTRPG/main/crown_and_skull/crown_and_skull.ttl#item_short_bow
:item_short_bow rdf:type owl:NamedIndividual ,
                         :ItemWeapon ;
                rdfs:comment "Conceal, use point blank"@en ;
                rdfs:label "Short Bow"@en ;
                gen:cost "1 hero point" ;
                gen:damage "1d6" .


###  https://raw.githubusercontent.com/AbsVahter/ontoTRPG/main/crown_and_skull/crown_and_skull.ttl#item_short_sword
:item_short_sword rdf:type owl:NamedIndividual ,
                           :ItemWeapon ;
                  rdfs:comment "Use with no hindrance in tight spaces"@en ;
                  rdfs:label "Short Sword"@en ;
                  gen:cost "1 hero point" ;
                  gen:damage "1d6" .


###  https://raw.githubusercontent.com/AbsVahter/ontoTRPG/main/crown_and_skull/crown_and_skull.ttl#item_small_boat
:item_small_boat rdf:type owl:NamedIndividual ,
                          :ItemLarge ;
                 rdfs:comment "Holds 4 people, barely seaworthy, sneaky"@en ;
                 rdfs:label "Small Boat"@en ;
                 gen:cost "15 hero points" .


###  https://raw.githubusercontent.com/AbsVahter/ontoTRPG/main/crown_and_skull/crown_and_skull.ttl#item_snare_kit
:item_snare_kit rdf:type owl:NamedIndividual ,
                         :ItemBasic ;
                rdfs:comment "3 count, catch small animals"@en ;
                rdfs:label "Snare Kit"@en ;
                gen:cost "1 hero point" .


###  https://raw.githubusercontent.com/AbsVahter/ontoTRPG/main/crown_and_skull/crown_and_skull.ttl#item_spear
:item_spear rdf:type owl:NamedIndividual ,
                     :ItemWeapon ;
            rdfs:comment "Thrown, long reach"@en ;
            rdfs:label "Spear"@en ;
            gen:cost "2 hero points" ;
            gen:damage "1d8" .


###  https://raw.githubusercontent.com/AbsVahter/ontoTRPG/main/crown_and_skull/crown_and_skull.ttl#item_spiked_flail
:item_spiked_flail rdf:type owl:NamedIndividual ,
                            :ItemWeapon ;
                   rdfs:comment "Double damage if used mounted"@en ;
                   rdfs:label "Spiked Flail"@en ;
                   gen:cost "3 hero points" ;
                   gen:damage "1d10" .


###  https://raw.githubusercontent.com/AbsVahter/ontoTRPG/main/crown_and_skull/crown_and_skull.ttl#item_steel_shield
:item_steel_shield rdf:type owl:NamedIndividual ,
                            :ItemArmor ;
                   rdfs:comment "Absorb 3 hits before attrition"@en ;
                   rdfs:label "Steel Shield"@en ;
                   gen:cost "5 hero points" ;
                   gen:defense "+2" .


###  https://raw.githubusercontent.com/AbsVahter/ontoTRPG/main/crown_and_skull/crown_and_skull.ttl#item_studded_mace
:item_studded_mace rdf:type owl:NamedIndividual ,
                            :ItemWeapon ;
                   rdfs:comment "If max damage, stun target 3 phases"@en ;
                   rdfs:label "Studded Mace"@en ;
                   gen:cost "2 hero points" ;
                   gen:damage "1d8" .


###  https://raw.githubusercontent.com/AbsVahter/ontoTRPG/main/crown_and_skull/crown_and_skull.ttl#item_torches
:item_torches rdf:type owl:NamedIndividual ,
                       :ItemBasic ;
              rdfs:comment "3 count, snap-light, burns for 1 scene"@en ;
              rdfs:label "Torches"@en ;
              gen:cost "1 hero point" .


###  https://raw.githubusercontent.com/AbsVahter/ontoTRPG/main/crown_and_skull/crown_and_skull.ttl#item_tower_shield
:item_tower_shield rdf:type owl:NamedIndividual ,
                            :ItemArmor ;
                   rdfs:comment "Clumsy, ignore attrition from arrows"@en ;
                   rdfs:label "Tower Shield"@en ;
                   gen:cost "5 hero points" ;
                   gen:defense "+3" .


###  https://raw.githubusercontent.com/AbsVahter/ontoTRPG/main/crown_and_skull/crown_and_skull.ttl#item_wagon
:item_wagon rdf:type owl:NamedIndividual ,
                     :ItemLarge ;
            rdfs:comment "Transports like a cart, at horse speed"@en ;
            rdfs:label "Wagon"@en ;
            gen:cost "20 hero points" .


###  https://raw.githubusercontent.com/AbsVahter/ontoTRPG/main/crown_and_skull/crown_and_skull.ttl#item_walking_staff
:item_walking_staff rdf:type owl:NamedIndividual ,
                             :ItemWeapon ;
                    rdfs:comment "Handy for all kinds of things"@en ;
                    rdfs:label "Walking Staff"@en ;
                    gen:cost "1 hero point" ;
                    gen:damage "1d4" .


###  https://raw.githubusercontent.com/AbsVahter/ontoTRPG/main/crown_and_skull/crown_and_skull.ttl#item_war_hammer
:item_war_hammer rdf:type owl:NamedIndividual ,
                          :ItemWeapon ;
                 rdfs:comment "If 7+ dmg, stun for 1d6 phases"@en ;
                 rdfs:label "War Hammer"@en ;
                 gen:cost "3 hero points" ;
                 gen:damage "1d10" .


###  https://raw.githubusercontent.com/AbsVahter/ontoTRPG/main/crown_and_skull/crown_and_skull.ttl#item_war_wagon
:item_war_wagon rdf:type owl:NamedIndividual ,
                         :ItemLarge ;
                rdfs:comment "An armored wagon for siege"@en ;
                rdfs:label "War Wagon"@en ;
                gen:cost "25 hero points" .


###  https://raw.githubusercontent.com/AbsVahter/ontoTRPG/main/crown_and_skull/crown_and_skull.ttl#item_wood_axe
:item_wood_axe rdf:type owl:NamedIndividual ,
                        :ItemWeapon ;
               rdfs:comment "Thrown, double damage on wood"@en ;
               rdfs:label "Wood Axe"@en ;
               gen:cost "1 hero point" ;
               gen:damage "1d6" .


###  https://raw.githubusercontent.com/AbsVahter/ontoTRPG/main/crown_and_skull/crown_and_skull.ttl#item_wood_shield
:item_wood_shield rdf:type owl:NamedIndividual ,
                           :ItemArmor ;
                  rdfs:comment "Absorb 2 hits before attrition"@en ;
                  rdfs:label "Wood Shield"@en ;
                  gen:cost "3 hero points" ;
                  gen:defense "+1" .


###  https://raw.githubusercontent.com/AbsVahter/ontoTRPG/main/crown_and_skull/crown_and_skull.ttl#lady_walcrest
:lady_walcrest rdf:type owl:NamedIndividual ,
                        gen:Creature ;
               rdfs:comment "The most widely respected fi gure in Rivergate is a venerable Baroness: heir to the Walcrest empire, Lady Ezmerelda Walcrest. Well into her 70s, she has seen and survived it all, but held true to the old alliances and standards of the town. All city policy is approved and executed by her and her council of advisors."@en ;
               rdfs:label "Lady Walcrest"@en .


###  https://raw.githubusercontent.com/AbsVahter/ontoTRPG/main/crown_and_skull/crown_and_skull.ttl#limitation_companion_clumsy
:limitation_companion_clumsy rdf:type owl:NamedIndividual ,
                                      :LimitationCompanion ;
                             rdfs:comment "This companion is almost never stealthy, hidden, or silent. The group’s sneaking or stealth efforts are afflicted by a -3 penalty."@en ;
                             rdfs:label "Clumsy"@en .


###  https://raw.githubusercontent.com/AbsVahter/ontoTRPG/main/crown_and_skull/crown_and_skull.ttl#limitation_companion_feral
:limitation_companion_feral rdf:type owl:NamedIndividual ,
                                     :LimitationCompanion ;
                            rdfs:comment "Will not stop attacking until all immediate foes are slain or subdued."@en ;
                            rdfs:label "Feral"@en .


###  https://raw.githubusercontent.com/AbsVahter/ontoTRPG/main/crown_and_skull/crown_and_skull.ttl#limitation_companion_frightened
:limitation_companion_frightened rdf:type owl:NamedIndividual ,
                                          :LimitationCompanion ;
                                 rdfs:comment "On a roll of 4 or less, or in special circumstances, this companion will flee, vanishing for 1D4 days."@en ;
                                 rdfs:label "Frightened"@en .


###  https://raw.githubusercontent.com/AbsVahter/ontoTRPG/main/crown_and_skull/crown_and_skull.ttl#limitation_companion_impulsive
:limitation_companion_impulsive rdf:type owl:NamedIndividual ,
                                         :LimitationCompanion ;
                                rdfs:comment "When battle is joined, this companion rolls its best skill. On a failed roll, it makes its own opening decision, using the hero’s phase."@en ;
                                rdfs:label "Impulsive"@en .


###  https://raw.githubusercontent.com/AbsVahter/ontoTRPG/main/crown_and_skull/crown_and_skull.ttl#limitation_companion_trophy
:limitation_companion_trophy rdf:type owl:NamedIndividual ,
                                      :LimitationCompanion ;
                             rdfs:comment "This companion is sought after by shadowy folk, collectors, jailers, or those who simply hate it."@en ;
                             rdfs:label "Trophy"@en .


###  https://raw.githubusercontent.com/AbsVahter/ontoTRPG/main/crown_and_skull/crown_and_skull.ttl#limitation_item_breakable
:limitation_item_breakable rdf:type owl:NamedIndividual ,
                                    :LimitationItem ;
                           rdfs:comment "On a critical fail usage, minimum damage roll, or special GM-noticed circumstances, this equipment just goes to pieces."@en ;
                           rdfs:label "Breakable"@en .


###  https://raw.githubusercontent.com/AbsVahter/ontoTRPG/main/crown_and_skull/crown_and_skull.ttl#limitation_item_garish
:limitation_item_garish rdf:type owl:NamedIndividual ,
                                 :LimitationItem ;
                        rdfs:comment "The appearance with this gear is over the top, ugly, or off-putting to most. This will draw enemy ire, embarrass you, or embolden foes."@en ;
                        rdfs:label "Garish"@en .


###  https://raw.githubusercontent.com/AbsVahter/ontoTRPG/main/crown_and_skull/crown_and_skull.ttl#limitation_item_heavy
:limitation_item_heavy rdf:type owl:NamedIndividual ,
                                :LimitationItem ;
                       rdfs:comment "This equipment is bulky, occupying 2 item inventory."@en ;
                       rdfs:label "Heavy"@en .


###  https://raw.githubusercontent.com/AbsVahter/ontoTRPG/main/crown_and_skull/crown_and_skull.ttl#limitation_item_sought_after
:limitation_item_sought_after rdf:type owl:NamedIndividual ,
                                       :LimitationItem ;
                              rdfs:comment "There are nefarious folk seeking this gear."@en ;
                              rdfs:label "Sought after"@en .


###  https://raw.githubusercontent.com/AbsVahter/ontoTRPG/main/crown_and_skull/crown_and_skull.ttl#limitation_item_stolen
:limitation_item_stolen rdf:type owl:NamedIndividual ,
                                 :LimitationItem ;
                        rdfs:comment "The owner of this gear, or forces of law, will hunt you down."@en ;
                        rdfs:label "Stolen"@en .


###  https://raw.githubusercontent.com/AbsVahter/ontoTRPG/main/crown_and_skull/crown_and_skull.ttl#limitation_item_wonky
:limitation_item_wonky rdf:type owl:NamedIndividual ,
                                :LimitationItem ;
                       rdfs:comment "This gear has silly or unexpected malfunctions the GM will referee as needed."@en ;
                       rdfs:label "Wonky"@en .


###  https://raw.githubusercontent.com/AbsVahter/ontoTRPG/main/crown_and_skull/crown_and_skull.ttl#limitation_spell_campfire_magic
:limitation_spell_campfire_magic rdf:type owl:NamedIndividual ,
                                          :LimitationSpell ;
                                 rdfs:comment "Can only be cast in a safe place."@en ;
                                 rdfs:label "Campfire magic"@en .


###  https://raw.githubusercontent.com/AbsVahter/ontoTRPG/main/crown_and_skull/crown_and_skull.ttl#limitation_spell_cannot_be_customized
:limitation_spell_cannot_be_customized rdf:type owl:NamedIndividual ,
                                                :LimitationSpell ;
                                       rdfs:comment "This spell is minimalistic, only available in its first-learned form, never to be changed."@en ;
                                       rdfs:label "Cannot be customized"@en .


###  https://raw.githubusercontent.com/AbsVahter/ontoTRPG/main/crown_and_skull/crown_and_skull.ttl#limitation_spell_cannot_be_targeted
:limitation_spell_cannot_be_targeted rdf:type owl:NamedIndividual ,
                                              :LimitationSpell ;
                                     rdfs:comment "Spell always flies wild. Use dice for direction, or randomly select from available targets."@en ;
                                     rdfs:label "Cannot be targeted"@en .


###  https://raw.githubusercontent.com/AbsVahter/ontoTRPG/main/crown_and_skull/crown_and_skull.ttl#limitation_spell_costs_attrition
:limitation_spell_costs_attrition rdf:type owl:NamedIndividual ,
                                           :LimitationSpell ;
                                  rdfs:comment "Sustain 1 attrition with each cast."@en ;
                                  rdfs:label "Costs attrition to cast"@en .


###  https://raw.githubusercontent.com/AbsVahter/ontoTRPG/main/crown_and_skull/crown_and_skull.ttl#limitation_spell_costs_material
:limitation_spell_costs_material rdf:type owl:NamedIndividual ,
                                          :LimitationSpell ;
                                 rdfs:comment "When cast, mark off 1 item in your inventory as destroyed... a powerful reagent like a crystal or crushed bone."@en ;
                                 rdfs:label "Costs material to cast"@en .


###  https://raw.githubusercontent.com/AbsVahter/ontoTRPG/main/crown_and_skull/crown_and_skull.ttl#limitation_spell_druidic
:limitation_spell_druidic rdf:type owl:NamedIndividual ,
                                   :LimitationSpell ;
                          rdfs:comment "Cannot be cast if the caster wears or is touching any metal."@en ;
                          rdfs:label "Druidic"@en .


###  https://raw.githubusercontent.com/AbsVahter/ontoTRPG/main/crown_and_skull/crown_and_skull.ttl#limitation_spell_exhausting
:limitation_spell_exhausting rdf:type owl:NamedIndividual ,
                                      :LimitationSpell ;
                             rdfs:comment "No magic can be used for 1 round after cast."@en ;
                             rdfs:label "Exhausting"@en .


###  https://raw.githubusercontent.com/AbsVahter/ontoTRPG/main/crown_and_skull/crown_and_skull.ttl#limitation_spell_ineffable
:limitation_spell_ineffable rdf:type owl:NamedIndividual ,
                                     :LimitationSpell ;
                            rdfs:comment "This magic is primal, and can’t be recorded for others to use on scrolls, weapons, rings, or wands of any sort."@en ;
                            rdfs:label "Ineffable"@en .


###  https://raw.githubusercontent.com/AbsVahter/ontoTRPG/main/crown_and_skull/crown_and_skull.ttl#limitation_spell_infernal
:limitation_spell_infernal rdf:type owl:NamedIndividual ,
                                    :LimitationSpell ;
                           rdfs:comment "Calls on brimstone and demons."@en ;
                           rdfs:label "Infernal spell"@en .


###  https://raw.githubusercontent.com/AbsVahter/ontoTRPG/main/crown_and_skull/crown_and_skull.ttl#limitation_spell_infernal_powers
:limitation_spell_infernal_powers rdf:type owl:NamedIndividual ,
                                           :LimitationSpell ;
                                  rdfs:comment "Calls on brimstone and demons. When cast, roll Magic to maintain control. If failing, roll on the Infernal Magic table."@en ;
                                  rdfs:label "Uses infernal powers"@en .


###  https://raw.githubusercontent.com/AbsVahter/ontoTRPG/main/crown_and_skull/crown_and_skull.ttl#limitation_spell_linked_to_object
:limitation_spell_linked_to_object rdf:type owl:NamedIndividual ,
                                            :LimitationSpell ;
                                   rdfs:comment "The spell manifests with or through an object. If that object is destroyed or stolen, the spell is lost."@en ;
                                   rdfs:label "Linked to physical object"@en .


###  https://raw.githubusercontent.com/AbsVahter/ontoTRPG/main/crown_and_skull/crown_and_skull.ttl#limitation_spell_madness
:limitation_spell_madness rdf:type owl:NamedIndividual ,
                                   :LimitationSpell ;
                          rdfs:comment "Each time this spell is cast, roll your Magic skill. On failure, take the Crazy flaw until your next rest."@en ;
                          rdfs:label "Madness"@en .


###  https://raw.githubusercontent.com/AbsVahter/ontoTRPG/main/crown_and_skull/crown_and_skull.ttl#limitation_spell_must_be_sustained
:limitation_spell_must_be_sustained rdf:type owl:NamedIndividual ,
                                             :LimitationSpell ;
                                    rdfs:comment "This spell ends if the caster is hit or takes any other action while the spell is active."@en ;
                                    rdfs:label "Must be sustained"@en .


###  https://raw.githubusercontent.com/AbsVahter/ontoTRPG/main/crown_and_skull/crown_and_skull.ttl#limitation_spell_nullified_by
:limitation_spell_nullified_by rdf:type owl:NamedIndividual ,
                                        :LimitationSpell ;
                               rdfs:comment "Has no effect on a specific type of target or target property."@en ;
                               rdfs:label "Nullified by"@en .


###  https://raw.githubusercontent.com/AbsVahter/ontoTRPG/main/crown_and_skull/crown_and_skull.ttl#limitation_spell_outdoors_only
:limitation_spell_outdoors_only rdf:type owl:NamedIndividual ,
                                         :LimitationSpell ;
                                rdfs:comment "Elemental forces are required to cast."@en ;
                                rdfs:label "Only works outdoors"@en .


###  https://raw.githubusercontent.com/AbsVahter/ontoTRPG/main/crown_and_skull/crown_and_skull.ttl#limitation_spell_painful
:limitation_spell_painful rdf:type owl:NamedIndividual ,
                                   :LimitationSpell ;
                          rdfs:comment "After this spell is cast, the user can only make a move on their next turn... i.e., no actions."@en ;
                          rdfs:label "Painful"@en .


###  https://raw.githubusercontent.com/AbsVahter/ontoTRPG/main/crown_and_skull/crown_and_skull.ttl#limitation_spell_red_speech
:limitation_spell_red_speech rdf:type owl:NamedIndividual ,
                                      :LimitationSpell ;
                             rdfs:comment "This spell can only be cast with booming, shouted words. This limitation prohibits the use of Silent Spell."@en ;
                             rdfs:label "Red Speech"@en .


###  https://raw.githubusercontent.com/AbsVahter/ontoTRPG/main/crown_and_skull/crown_and_skull.ttl#limitation_spell_ritual
:limitation_spell_ritual rdf:type owl:NamedIndividual ,
                                  :LimitationSpell ;
                         rdfs:comment "This spell can only be cast with 1D4 uninterrupted rounds of successful Magic skill rolls."@en ;
                         rdfs:label "Ritual"@en .


###  https://raw.githubusercontent.com/AbsVahter/ontoTRPG/main/crown_and_skull/crown_and_skull.ttl#limitation_spell_specific_target_type
:limitation_spell_specific_target_type rdf:type owl:NamedIndividual ,
                                                :LimitationSpell ;
                                       rdfs:comment "Can be anything. Be as specific as possible."@en ;
                                       rdfs:label "Only works on specific target type"@en .


###  https://raw.githubusercontent.com/AbsVahter/ontoTRPG/main/crown_and_skull/crown_and_skull.ttl#limitation_spell_two_phase_cast
:limitation_spell_two_phase_cast rdf:type owl:NamedIndividual ,
                                          :LimitationSpell ;
                                 rdfs:comment "Effect takes place at the end of the caster’s second phase spent casting. If hit in that time, the count starts over. If rolling to cast, the roll must be made twice consecutively."@en ;
                                 rdfs:label "Takes 2 phases to cast"@en .


###  https://raw.githubusercontent.com/AbsVahter/ontoTRPG/main/crown_and_skull/crown_and_skull.ttl#limitation_spell_unstable
:limitation_spell_unstable rdf:type owl:NamedIndividual ,
                                    :LimitationSpell ;
                           rdfs:comment "A wobbly, barely-contained magic. When cast, roll Magic to maintain control. If failing, roll on the Unstable Magic table."@en ;
                           rdfs:label "Unstable"@en ,
                                      "Unstable spell"@en .


###  https://raw.githubusercontent.com/AbsVahter/ontoTRPG/main/crown_and_skull/crown_and_skull.ttl#lineage
:lineage rdf:type owl:NamedIndividual ,
                  gen:ParameterPC ;
         rdfs:comment "narrative parameter"@en ;
         rdfs:label "Lineage"@en .


###  https://raw.githubusercontent.com/AbsVahter/ontoTRPG/main/crown_and_skull/crown_and_skull.ttl#lineage_elf
:lineage_elf rdf:type owl:NamedIndividual ,
                      :Lineage ;
             rdfs:comment "Elven folk have a knack for the magical..."@en ;
             rdfs:label "Elven lineage"@en .


###  https://raw.githubusercontent.com/AbsVahter/ontoTRPG/main/crown_and_skull/crown_and_skull.ttl#lineage_frog
:lineage_frog rdf:type owl:NamedIndividual ,
                       :Lineage ;
              rdfs:comment "Frog-kin are honor-bound, trapped in a violent empire..."@en ;
              rdfs:label "Frog lineage"@en .


###  https://raw.githubusercontent.com/AbsVahter/ontoTRPG/main/crown_and_skull/crown_and_skull.ttl#lineage_human
:lineage_human rdf:type owl:NamedIndividual ,
                        :Lineage ;
               rdfs:comment "Humankind are a versatile folk..."@en ;
               rdfs:label "Humankind lineage"@en .


###  https://raw.githubusercontent.com/AbsVahter/ontoTRPG/main/crown_and_skull/crown_and_skull.ttl#lineage_proudfoot
:lineage_proudfoot rdf:type owl:NamedIndividual ,
                            :Lineage ;
                   rdfs:comment "Proudfoots are feastwise inventors..."@en ;
                   rdfs:label "Proudfoot lineage"@en .


###  https://raw.githubusercontent.com/AbsVahter/ontoTRPG/main/crown_and_skull/crown_and_skull.ttl#lineage_stout
:lineage_stout rdf:type owl:NamedIndividual ,
                        :Lineage ;
               rdfs:comment "Stout Folk are usually built like tanks..."@en ;
               rdfs:label "Stout lineage"@en .


###  https://raw.githubusercontent.com/AbsVahter/ontoTRPG/main/crown_and_skull/crown_and_skull.ttl#lord_loyce
:lord_loyce rdf:type owl:NamedIndividual ,
                     gen:Creature ;
            rdfs:comment "This is a mysterious fi gure known as Lord Royce, said by doomsayers to be ‘he who would drink the world.’"@en ;
            rdfs:label "Lord Loyce"@en .


###  https://raw.githubusercontent.com/AbsVahter/ontoTRPG/main/crown_and_skull/crown_and_skull.ttl#losing_control
:losing_control rdf:type owl:NamedIndividual ;
                rdfs:label "Losing control"@en ;
                gen:Actor gen:master ;
                gen:effectOption :losing_control_flesh_attrition_and_magic_block ,
                                 :losing_control_flesh_attrition_and_stun ,
                                 :losing_control_focus_on_caster ,
                                 :losing_control_opposite_effect .


###  https://raw.githubusercontent.com/AbsVahter/ontoTRPG/main/crown_and_skull/crown_and_skull.ttl#losing_control_flesh_attrition_and_magic_block
:losing_control_flesh_attrition_and_magic_block rdf:type owl:NamedIndividual ;
                                                rdfs:label "Losing control: flesh attrition and magic block"@en ;
                                                gen:Actor gen:master ;
                                                gen:effect :attrition_flesh ,
                                                           :status_magic_block ;
                                                gen:target "caster of wild magic" .


###  https://raw.githubusercontent.com/AbsVahter/ontoTRPG/main/crown_and_skull/crown_and_skull.ttl#losing_control_flesh_attrition_and_stun
:losing_control_flesh_attrition_and_stun rdf:type owl:NamedIndividual ;
                                         rdfs:label "Losing control: flesh attrition and stun"@en ;
                                         gen:Actor gen:master ;
                                         gen:effect :attrition_flesh ,
                                                    :status_stun ;
                                         gen:target "caster of wild magic" ;
                                         gen:valueFormula "stun duration = 1 round" .


###  https://raw.githubusercontent.com/AbsVahter/ontoTRPG/main/crown_and_skull/crown_and_skull.ttl#losing_control_focus_on_caster
:losing_control_focus_on_caster rdf:type owl:NamedIndividual ;
                                rdfs:comment "Fizzles and sparks cause nearby enemies to focus on the caster"@en ;
                                rdfs:label "Losing control: focus of enemies on caster"@en ;
                                gen:Actor gen:master ;
                                gen:set :status_enemy_focus ;
                                gen:target "caster of wild magic" .


###  https://raw.githubusercontent.com/AbsVahter/ontoTRPG/main/crown_and_skull/crown_and_skull.ttl#losing_control_opposite_effect
:losing_control_opposite_effect rdf:type owl:NamedIndividual ;
                                rdfs:comment "Desired effect is achieved, but in an opposite form."@en ;
                                rdfs:label "Losing control: opposite effect"@en ;
                                gen:Actor gen:master ;
                                gen:modified :set_spell .


###  https://raw.githubusercontent.com/AbsVahter/ontoTRPG/main/crown_and_skull/crown_and_skull.ttl#magic_advancements
:magic_advancements rdf:type owl:NamedIndividual ,
                             gen:ParameterPC ;
                    rdfs:comment "format = [list of abilities]"@en ;
                    rdfs:label "Magic advancements"@en .


###  https://raw.githubusercontent.com/AbsVahter/ontoTRPG/main/crown_and_skull/crown_and_skull.ttl#magic_subclass
:magic_subclass rdf:type owl:NamedIndividual ,
                         gen:ParameterPC ;
                rdfs:label "Magic subclass"@en .


###  https://raw.githubusercontent.com/AbsVahter/ontoTRPG/main/crown_and_skull/crown_and_skull.ttl#maximize_roll
:maximize_roll rdf:type owl:NamedIndividual ;
               rdfs:label "Maximize roll"@en ;
               gen:Actor gen:player ;
               gen:modified :damage_roll ,
                            gen:Check ;
               gen:valueFormula "reroll roll enterily" .


###  https://raw.githubusercontent.com/AbsVahter/ontoTRPG/main/crown_and_skull/crown_and_skull.ttl#miracle
:miracle rdf:type owl:NamedIndividual ;
         rdfs:comment "Divine will manifests in unexpected ways. Upon a successful request for a miracle, the faithful must offer some explanation of their hopes. The GM will then take the reins, offering the divine intervention as they see fit."@en ;
         rdfs:label "Miracle"@en ;
         gen:Actor gen:party .


###  https://raw.githubusercontent.com/AbsVahter/ontoTRPG/main/crown_and_skull/crown_and_skull.ttl#move
:move rdf:type owl:NamedIndividual ;
      rdfs:label "Move"@en ;
      gen:modified gen:position ;
      gen:valueFormula "Move elsewhere in the scene, about 6” table space. A small ‘sidestep’ move is allowed without using one’s phase." .


###  https://raw.githubusercontent.com/AbsVahter/ontoTRPG/main/crown_and_skull/crown_and_skull.ttl#north_holds
:north_holds rdf:type owl:NamedIndividual ,
                      gen:Location ;
             rdfs:comment "This vast, diverse landscape is filled with cultures, secrets, and dangers for you to explore."@en ;
             rdfs:label "The North Holds"@en ;
             gen:included :gardenburrow ,
                          :rivergate ,
                          :slimshire .


###  https://raw.githubusercontent.com/AbsVahter/ontoTRPG/main/crown_and_skull/crown_and_skull.ttl#path_of_magic
:path_of_magic rdf:type owl:NamedIndividual ;
               rdfs:comment "More comprehensive progression for the magic user"@en ;
               rdfs:label "Path of magic"@en ;
               gen:Actor gen:player ;
               gen:effectOption :path_of_magic_antimagic ,
                                :path_of_magic_divine ,
                                :path_of_magic_wizard .


###  https://raw.githubusercontent.com/AbsVahter/ontoTRPG/main/crown_and_skull/crown_and_skull.ttl#path_of_magic_antimagic
:path_of_magic_antimagic rdf:type owl:NamedIndividual ;
                         rdfs:comment "This method seeks to nullify, cancel, or remove magic rather than channel it. To learn any of the abilities listed here, the practitioner must have access to magical research facilities, no matter their style or path. Antimagic is a closely guarded secret, and not easily learned."@en ;
                         rdfs:label "Antimagic path"@en ;
                         gen:Actor gen:player ;
                         gen:cost "1 hero point per level" ;
                         gen:input :hero_points ;
                         gen:inputOption :SkillAntimagic ;
                         gen:prerequisiteDescription "(earned hero points >= 15)" ;
                         gen:resource :hero_points ;
                         gen:setAdditive :skills .


###  https://raw.githubusercontent.com/AbsVahter/ontoTRPG/main/crown_and_skull/crown_and_skull.ttl#path_of_magic_divine
:path_of_magic_divine rdf:type owl:NamedIndividual ;
                      rdfs:comment "Wizards and their kind draw power by comprehension, intuition, and methodology. The user of divine magic, by contrast, places their trust in higher beings... offering themselves as mere conduits for deifi c blessings and miracles. The means of this transfer of power is a complete mystery. This mystery has a name: faith."@en ;
                      rdfs:label "Path of divine magic"@en ;
                      gen:Actor gen:player ;
                      gen:included :path_of_magic_divine_faith_instead_of_magic ,
                                   :path_of_magic_divine_holy_symbol_advancement ,
                                   :path_of_magic_divine_lord ,
                                   :path_of_magic_holy ;
                      gen:input :equipment ,
                                :item_holy_symbol ,
                                :skill_faith ;
                      gen:prerequisiteDescription "(faith > 2) and (deity) and (holy symbol in equipment)" .


###  https://raw.githubusercontent.com/AbsVahter/ontoTRPG/main/crown_and_skull/crown_and_skull.ttl#path_of_magic_divine_faith_instead_of_magic
:path_of_magic_divine_faith_instead_of_magic rdf:type owl:NamedIndividual ;
                                             rdfs:label "Path of divine magic: using faith skill instead of magic"@en ;
                                             gen:modified :check_skill ;
                                             gen:prerequisite :skill_magic ;
                                             gen:valueFormula "magic skill -> faith skill" ;
                                             gen:valueObject :skill_faith .


###  https://raw.githubusercontent.com/AbsVahter/ontoTRPG/main/crown_and_skull/crown_and_skull.ttl#path_of_magic_divine_holy_symbol_advancement
:path_of_magic_divine_holy_symbol_advancement rdf:type owl:NamedIndividual ;
                                              rdfs:comment "purchased at any time"@en ;
                                              rdfs:label "Path of divine magic: advancement for holy symbol"@en ;
                                              gen:cost "3 hero points" ;
                                              gen:input :item_holy_symbol ;
                                              gen:inputOption :MagicAdvancementHolySymbol ;
                                              gen:prerequisiteDescription "(holy symbol in equipment) and (number of advancements <= 2)" ;
                                              gen:resource :hero_points ;
                                              gen:setAdditive :spells ;
                                              gen:valueFormula "spells += selected advancement" .


###  https://raw.githubusercontent.com/AbsVahter/ontoTRPG/main/crown_and_skull/crown_and_skull.ttl#path_of_magic_divine_lord
:path_of_magic_divine_lord rdf:type owl:NamedIndividual ;
                           rdfs:comment "You will be awarded a stronghold, abbey, or holy site as your own, and proclaimed Divine Lord of that area. This title will earn you land, equipment stores, a few loyal servants, and invitations from various dignitaries."@en ;
                           rdfs:label "Path of Divine Lord"@en ;
                           gen:after :path_of_magic_holy ;
                           gen:input :hero_points ;
                           gen:prerequisiteDescription "earned hero points >= 50" .


###  https://raw.githubusercontent.com/AbsVahter/ontoTRPG/main/crown_and_skull/crown_and_skull.ttl#path_of_magic_holy
:path_of_magic_holy rdf:type owl:NamedIndividual ;
                    rdfs:comment "This is a way of life that leaves no room for selfishness, compromise, or earthly concerns. The player is encouraged to role play this way of life."@en ;
                    rdfs:label "The holy Path"@en ;
                    gen:Actor gen:player ;
                    gen:included :path_of_magic_holy_high_priest ,
                                 :path_of_magic_holy_pray ,
                                 :path_of_magic_holy_safe_heaven ;
                    gen:input :hero_points ;
                    gen:prerequisiteDescription "earned hero points >= 15" .


###  https://raw.githubusercontent.com/AbsVahter/ontoTRPG/main/crown_and_skull/crown_and_skull.ttl#path_of_magic_holy_high_priest
:path_of_magic_holy_high_priest rdf:type owl:NamedIndividual ;
                                rdfs:comment "Once you walk the path, the next abbey or place of worship you visit will include a High Priest to take you in as a loyal aspirant. You will be asked to make a solemn vow to this person, and offer your life to their service."@en ;
                                rdfs:label "The holy Path: a High Priest"@en .


###  https://raw.githubusercontent.com/AbsVahter/ontoTRPG/main/crown_and_skull/crown_and_skull.ttl#path_of_magic_holy_pray
:path_of_magic_holy_pray rdf:type owl:NamedIndividual ,
                                  gen:Check ;
                         rdfs:label "The holy Path: Pray"@en ;
                         gen:basedOn :check_skill ;
                         gen:checkSuccess :miracle ;
                         gen:duration "1d4 rounds" ;
                         gen:input :equipment ,
                                   :item_holy_symbol ;
                         gen:prerequisite :skill_faith ;
                         gen:prerequisiteDescription "(deity) and (holy symbol in equipment)" .


###  https://raw.githubusercontent.com/AbsVahter/ontoTRPG/main/crown_and_skull/crown_and_skull.ttl#path_of_magic_holy_safe_heaven
:path_of_magic_holy_safe_heaven rdf:type owl:NamedIndividual ;
                                rdfs:comment "In exchange for your service thus promised, you and your allies can always treat holy sites as places of rest and safety, even in enemy territory. A humble shrine can become a fortress."@en ;
                                rdfs:label "The holy Path: Safe Haven"@en .


###  https://raw.githubusercontent.com/AbsVahter/ontoTRPG/main/crown_and_skull/crown_and_skull.ttl#path_of_magic_wizard
:path_of_magic_wizard rdf:type owl:NamedIndividual ;
                      rdfs:comment "A wizard is a rare and misunderstood thing... a child of the elements, a dimension-strider, a being whose innate nature is magical for good, ill, or both. Though always old and wizened in appearance, wizards have strangely ‘young’ souls... sometimes forgetful of their own origins, purpose, or even name."@en ;
                      rdfs:label "Path of Wizard"@en ;
                      gen:Actor gen:player ;
                      gen:included :path_of_magic_wizard_advancement ,
                                   :path_of_magic_wizard_bargain ,
                                   :path_of_magic_wizard_selection_of_subclass ,
                                   :path_of_magic_wizard_tether ;
                      gen:modified gen:pc ;
                      gen:prerequisite :flaw_ancient .


###  https://raw.githubusercontent.com/AbsVahter/ontoTRPG/main/crown_and_skull/crown_and_skull.ttl#path_of_magic_wizard_advancement
:path_of_magic_wizard_advancement rdf:type owl:NamedIndividual ;
                                  rdfs:label "Wizard: advancement"@en ;
                                  gen:after :path_of_magic_wizard_selection_of_subclass ;
                                  gen:cost "cost of magic advancement" ;
                                  gen:input :tier ;
                                  gen:inputOption :MagicAdvancement ;
                                  gen:prerequisite :rest ;
                                  gen:prerequisiteDescription "(tier = 1) or (initial number of magic advancements of (tier - 1) > (4 - tier))" ;
                                  gen:resource :hero_points ;
                                  gen:setAdditive :magic_advancements .


###  https://raw.githubusercontent.com/AbsVahter/ontoTRPG/main/crown_and_skull/crown_and_skull.ttl#path_of_magic_wizard_bargain
:path_of_magic_wizard_bargain rdf:type owl:NamedIndividual ;
                              rdfs:label "Path of Wizard: making a bargain"@en ;
                              gen:included :contacting_arcanum ,
                                           :tattooing_bargain ;
                              gen:setAdditive :tattoos .


###  https://raw.githubusercontent.com/AbsVahter/ontoTRPG/main/crown_and_skull/crown_and_skull.ttl#path_of_magic_wizard_during_action
:path_of_magic_wizard_during_action rdf:type owl:NamedIndividual ;
                                    rdfs:label "Making a bargain during action"@en ;
                                    gen:input :rest ;
                                    gen:modified :path_of_magic_wizard_advancement ;
                                    gen:valueFormula "may be granted an advancement during action scenes" .


###  https://raw.githubusercontent.com/AbsVahter/ontoTRPG/main/crown_and_skull/crown_and_skull.ttl#path_of_magic_wizard_overspend
:path_of_magic_wizard_overspend rdf:type owl:NamedIndividual ;
                                rdfs:label "Making a bargain with overspend advancement"@en ;
                                gen:modified :path_of_magic_wizard_advancement ;
                                gen:valueFormula "(cost of magic advancement) - 3" .


###  https://raw.githubusercontent.com/AbsVahter/ontoTRPG/main/crown_and_skull/crown_and_skull.ttl#path_of_magic_wizard_selection_of_subclass
:path_of_magic_wizard_selection_of_subclass rdf:type owl:NamedIndividual ;
                                            rdfs:label "Wizard: path selection"@en ;
                                            gen:inputOption :Wizard ;
                                            gen:set :magic_subclass .


###  https://raw.githubusercontent.com/AbsVahter/ontoTRPG/main/crown_and_skull/crown_and_skull.ttl#path_of_magic_wizard_tether
:path_of_magic_wizard_tether rdf:type owl:NamedIndividual ;
                             rdfs:label "Path of Wizard: forming a tether"@en ;
                             gen:included :tattooing_tether ,
                                          :tether_service ,
                                          :word_is_bond ;
                             gen:setAdditive :tattoos .


###  https://raw.githubusercontent.com/AbsVahter/ontoTRPG/main/crown_and_skull/crown_and_skull.ttl#perform_action
:perform_action rdf:type owl:NamedIndividual ;
                rdfs:comment "Make an attack, use a skill, cast a spell or perform one discreet action. This takes your entire phase."@en ;
                rdfs:label "Perform an Action"@en ;
                gen:effectOption :attack_of_enemy ,
                                 :check_skill ,
                                 :set_damage ,
                                 :wild_magic .


###  https://raw.githubusercontent.com/AbsVahter/ontoTRPG/main/crown_and_skull/crown_and_skull.ttl#phase_action
:phase_action rdf:type owl:NamedIndividual ;
              rdfs:label "Action on phase"@en ;
              gen:after :phase_choose ;
              gen:effectOption :hurry ,
                               :move ,
                               :perform_action ;
              gen:prerequisiteDescription "any time enemies and heroes share a phase, heroes go first" .


###  https://raw.githubusercontent.com/AbsVahter/ontoTRPG/main/crown_and_skull/crown_and_skull.ttl#phase_choose
:phase_choose rdf:type owl:NamedIndividual ;
              rdfs:comment """
Generally, players will agree on which phase is best, especially after a few battles inform their decision. What phase a character chooses can be changed, but not mid-combat. Players can also choose the same phase.
For enemies GM chooses phases accordingly with character's statistic.
"""@en ;
              rdfs:label "Choosing a Phase"@en ;
              gen:prerequisiteDescription "(foes acts in phases (1, 3, 5)) and (number of actions = count of phases of creature)" ;
              gen:set :phase_of_character ;
              gen:valueFormula "1..5" .


###  https://raw.githubusercontent.com/AbsVahter/ontoTRPG/main/crown_and_skull/crown_and_skull.ttl#phase_of_character
:phase_of_character rdf:type owl:NamedIndividual ,
                             gen:ParameterCreature ;
                    rdfs:label "Phase of character"@en .


###  https://raw.githubusercontent.com/AbsVahter/ontoTRPG/main/crown_and_skull/crown_and_skull.ttl#phases_and_rounds
:phases_and_rounds rdf:type owl:NamedIndividual ;
                   rdfs:comment "Think of phases as cool moments in an action scene. A collection of these moments is called a round. Which phase a hero takes action is a meaningful choice for timing and strategy."@en ;
                   rdfs:label "Phases and Rounds"@en ;
                   gen:after :setting_scene ;
                   gen:included :death_of_pc ,
                                :phase_action ,
                                :phase_choose .


###  https://raw.githubusercontent.com/AbsVahter/ontoTRPG/main/crown_and_skull/crown_and_skull.ttl#recovery
:recovery rdf:type owl:NamedIndividual ;
          rdfs:comment "After each scene in play, once safety is found and no enemies or timers are incoming, regain 1 equipment or skill."@en ;
          rdfs:label "Recovery"@en ;
          gen:after :phases_and_rounds ;
          gen:modified :equipment ,
                       :skills ;
          gen:valueFormula "1 (equipment or skill) crossed -> non-crossed" .


###  https://raw.githubusercontent.com/AbsVahter/ontoTRPG/main/crown_and_skull/crown_and_skull.ttl#renown
:renown rdf:type owl:NamedIndividual ;
        rdfs:comment "Renown is the inevitable result of heroic action, acknowledged by folk of the realm and GM alike as deeds."@en ;
        rdfs:label "Renown"@en ;
        gen:Actor gen:master ;
        gen:setAdditive :deeds ;
        gen:valueNumeric 1 .


###  https://raw.githubusercontent.com/AbsVahter/ontoTRPG/main/crown_and_skull/crown_and_skull.ttl#repair
:repair rdf:type owl:NamedIndividual ;
        rdfs:comment "repair 1 crossed-off equipment"@en ;
        rdfs:label "Repair"@en ;
        gen:modified :equipment ;
        gen:valueFormula "1 equipment crossed -> non-crossed" .


###  https://raw.githubusercontent.com/AbsVahter/ontoTRPG/main/crown_and_skull/crown_and_skull.ttl#repair_failed
:repair_failed rdf:type owl:NamedIndividual ;
               rdfs:comment "On a failure, the armor is destroyed."@en ;
               rdfs:label "Failed repair"@en ;
               gen:setAdditive :equipment ;
               gen:valueFormula "destroy item in process of repair" .


###  https://raw.githubusercontent.com/AbsVahter/ontoTRPG/main/crown_and_skull/crown_and_skull.ttl#reroll
:reroll rdf:type owl:NamedIndividual ;
        rdfs:label "Reroll"@en ;
        gen:Actor gen:player ;
        gen:modified :damage_roll ,
                     gen:Check ;
        gen:valueFormula "reroll roll enterily" .


###  https://raw.githubusercontent.com/AbsVahter/ontoTRPG/main/crown_and_skull/crown_and_skull.ttl#rest
:rest rdf:type owl:NamedIndividual ;
      rdfs:comment "Regain a combined 1D4 of equipment and skills with a night’s rest in safety."@en ;
      rdfs:label "Rest"@en ;
      gen:effectOption :spending_hero_points ;
      gen:modified :equipment ,
                   :skills ;
      gen:valueFormula "1d4 (equipment or skill) crossed -> non-crossed" .


###  https://raw.githubusercontent.com/AbsVahter/ontoTRPG/main/crown_and_skull/crown_and_skull.ttl#ring_anvil_light
:ring_anvil_light rdf:type owl:NamedIndividual ,
                           :Item ;
                  rdfs:label "Ring of the Anvil's Light"@en .


###  https://raw.githubusercontent.com/AbsVahter/ontoTRPG/main/crown_and_skull/crown_and_skull.ttl#ring_skull
:ring_skull rdf:type owl:NamedIndividual ,
                     :Item ;
            rdfs:label "Ring of the Skull"@en .


###  https://raw.githubusercontent.com/AbsVahter/ontoTRPG/main/crown_and_skull/crown_and_skull.ttl#rivergate
:rivergate rdf:type owl:NamedIndividual ,
                    gen:Location ;
           rdfs:comment "At the geographic center point of The North Holds is the port city of Rivergate. This central location has made the ruling elite here wealthy, trading with the Stormkeeper dwarves and the abundant farms south of the River Thenne. Now that Ruinmoor has gone quiet, though, Rivergate is in crisis. To call this town home, you’ll be working for desperate nobles, escorting merchant barges, or exploring the fallen walls of ancient monasteries. Rivergate is the busy hub of mankind, with all its intrigue and peril."@en ;
           rdfs:label "Rivergate, Bustling Trade City"@en ;
           gen:included :frothy_mare ,
                        :thenneport_docks .


###  https://raw.githubusercontent.com/AbsVahter/ontoTRPG/main/crown_and_skull/crown_and_skull.ttl#rivergate_residents
:rivergate_residents rdf:type owl:NamedIndividual ;
                     rdfs:label "Residents of Rivergate"@en ;
                     gen:Actor :lady_walcrest ;
                     gen:Location :rivergate .


###  https://raw.githubusercontent.com/AbsVahter/ontoTRPG/main/crown_and_skull/crown_and_skull.ttl#rivergate_threat
:rivergate_threat rdf:type owl:NamedIndividual ;
                  rdfs:comment "Mysterious archers have been harassing travelers and residents alike, leaving none alive to identify them. A murmur of fear is spreading..."@en ;
                  rdfs:label "Threat at Rivergate"@en ;
                  gen:Location :rivergate .


###  https://raw.githubusercontent.com/AbsVahter/ontoTRPG/main/crown_and_skull/crown_and_skull.ttl#selene
:selene rdf:type owl:NamedIndividual ,
                 gen:Creature ;
        rdfs:comment "An elder hunter and forest warden, Selene is widely known as the oldest elf in this region. She was making camp here before there was a town at all, and knows every nook and cranny of the Oakenwood and beyond. She is a descendent of the third royal line of Thryn, enjoying all the privileges of a Baroness but choosing a humble life."@en ;
        rdfs:label "Selene"@en .


###  https://raw.githubusercontent.com/AbsVahter/ontoTRPG/main/crown_and_skull/crown_and_skull.ttl#set_bonus_reward
:set_bonus_reward rdf:type owl:NamedIndividual ;
                  rdfs:label "Bonus reward for hero points"@en ;
                  gen:after :set_hero_points ;
                  gen:prerequisiteDescription "per 10 hero points" ;
                  gen:set :hometown_bonus .


###  https://raw.githubusercontent.com/AbsVahter/ontoTRPG/main/crown_and_skull/crown_and_skull.ttl#set_damage
:set_damage rdf:type owl:NamedIndividual ;
            rdfs:label "Set damage to enemy"@en ;
            gen:Actor gen:player ;
            gen:input :damage_penalty ,
                      :damage_roll ,
                      :stat_def_enemy ;
            gen:setAdditive :stat_hp ;
            gen:target "enemy" ;
            gen:valueFormula "(defense of enemy) + (damage penalty) - (damage roll)" .


###  https://raw.githubusercontent.com/AbsVahter/ontoTRPG/main/crown_and_skull/crown_and_skull.ttl#set_flaw
:set_flaw rdf:type owl:NamedIndividual ;
          rdfs:label "Set flaw"@en ;
          gen:inputOption :FlawBasic ;
          gen:prerequisiteDescription "number of flaws <= 4" ;
          gen:setAdditive :flaws .


###  https://raw.githubusercontent.com/AbsVahter/ontoTRPG/main/crown_and_skull/crown_and_skull.ttl#set_hero_coin
:set_hero_coin rdf:type owl:NamedIndividual ;
               rdfs:label "Awarding hero coin to player"@en ;
               gen:Actor gen:master ;
               gen:prerequisiteDescription "acts of heroism or astounding play" ;
               gen:set :hero_coin ;
               gen:valueNumeric 1 .


###  https://raw.githubusercontent.com/AbsVahter/ontoTRPG/main/crown_and_skull/crown_and_skull.ttl#set_hero_points
:set_hero_points rdf:type owl:NamedIndividual ;
                 rdfs:label "Awarding hero points"@en ;
                 gen:Actor gen:master ;
                 gen:setAdditive :hero_points .


###  https://raw.githubusercontent.com/AbsVahter/ontoTRPG/main/crown_and_skull/crown_and_skull.ttl#set_hometown
:set_hometown rdf:type owl:NamedIndividual ;
              rdfs:label "Choose a hometown"@en ;
              gen:Actor gen:party ;
              gen:inputOption :gardenburrow ,
                              :rivergate ,
                              :slimshire ;
              gen:set :hometown .


###  https://raw.githubusercontent.com/AbsVahter/ontoTRPG/main/crown_and_skull/crown_and_skull.ttl#set_spell
:set_spell rdf:type owl:NamedIndividual .


###  https://raw.githubusercontent.com/AbsVahter/ontoTRPG/main/crown_and_skull/crown_and_skull.ttl#set_status_afraid
:set_status_afraid rdf:type owl:NamedIndividual ;
                   rdfs:label "Start be afraid"@en ;
                   gen:set :status_afraid .


###  https://raw.githubusercontent.com/AbsVahter/ontoTRPG/main/crown_and_skull/crown_and_skull.ttl#set_status_bleed
:set_status_bleed rdf:type owl:NamedIndividual ;
                  rdfs:label "Start bleed"@en ;
                  gen:set :status_bleed .


###  https://raw.githubusercontent.com/AbsVahter/ontoTRPG/main/crown_and_skull/crown_and_skull.ttl#set_status_burning
:set_status_burning rdf:type owl:NamedIndividual ;
                    rdfs:label "Start burning"@en ;
                    gen:prerequisiteDescription "ignition by fire attacks or effects" ;
                    gen:set :status_burning .


###  https://raw.githubusercontent.com/AbsVahter/ontoTRPG/main/crown_and_skull/crown_and_skull.ttl#set_status_close_to_death
:set_status_close_to_death rdf:type owl:NamedIndividual ;
                           rdfs:label "Set status Close to death"@en ;
                           gen:input :equipment ,
                                     :skills ;
                           gen:prerequisiteDescription "(no non-damaged equipment to get equipment attrition) or (no non-crossed skill to get skill attrition)" ;
                           gen:set :status_close_to_death ;
                           gen:target "target of attrition" .


###  https://raw.githubusercontent.com/AbsVahter/ontoTRPG/main/crown_and_skull/crown_and_skull.ttl#set_status_corrosion
:set_status_corrosion rdf:type owl:NamedIndividual ;
                      rdfs:label "Start corrosion"@en ;
                      gen:set :status_corrosion .


###  https://raw.githubusercontent.com/AbsVahter/ontoTRPG/main/crown_and_skull/crown_and_skull.ttl#set_status_freezing
:set_status_freezing rdf:type owl:NamedIndividual ;
                     rdfs:label "Start freezing"@en ;
                     gen:blocked :status_overheated ;
                     gen:prerequisiteDescription "4 rounds of deep cold" ;
                     gen:set :status_freezing .


###  https://raw.githubusercontent.com/AbsVahter/ontoTRPG/main/crown_and_skull/crown_and_skull.ttl#set_status_grappled
:set_status_grappled rdf:type owl:NamedIndividual ;
                     rdfs:label "Set grapple status"@en ;
                     gen:set :status_grapple ;
                     gen:target "enemy" .


###  https://raw.githubusercontent.com/AbsVahter/ontoTRPG/main/crown_and_skull/crown_and_skull.ttl#set_status_overheated
:set_status_overheated rdf:type owl:NamedIndividual ;
                       rdfs:label "Start overheated status"@en ;
                       gen:blocked :status_freezing ;
                       gen:prerequisiteDescription "2 rounds of extreme heat" ;
                       gen:set :status_overheated .


###  https://raw.githubusercontent.com/AbsVahter/ontoTRPG/main/crown_and_skull/crown_and_skull.ttl#set_status_stun
:set_status_stun rdf:type owl:NamedIndividual ;
                 rdfs:label "Set stun status"@en ;
                 gen:set :status_stun .


###  https://raw.githubusercontent.com/AbsVahter/ontoTRPG/main/crown_and_skull/crown_and_skull.ttl#set_status_stun_brawling
:set_status_stun_brawling rdf:type owl:NamedIndividual ;
                          rdfs:label "Set stun status by brawling"@en ;
                          gen:set :status_stun_brawling ;
                          gen:target "enemy" .


###  https://raw.githubusercontent.com/AbsVahter/ontoTRPG/main/crown_and_skull/crown_and_skull.ttl#set_status_stun_by_brutal_attrition
:set_status_stun_by_brutal_attrition rdf:type owl:NamedIndividual ;
                                     rdfs:label "Set stun because of maximum roll on Brutal Attrition"@en ;
                                     gen:prerequisiteDescription "brutal attrition roll = 6" ;
                                     gen:set :status_stun .


###  https://raw.githubusercontent.com/AbsVahter/ontoTRPG/main/crown_and_skull/crown_and_skull.ttl#setting_scene
:setting_scene rdf:type owl:NamedIndividual ;
               rdfs:label "Setting the Scene"@en ;
               gen:Actor gen:master .


###  https://raw.githubusercontent.com/AbsVahter/ontoTRPG/main/crown_and_skull/crown_and_skull.ttl#skill_animal_training
:skill_animal_training rdf:type owl:NamedIndividual ,
                                :SkillBasic ;
                       rdfs:comment "Charm or induce an animal companion to perform simple actions. Can only be used with one animal at a time."@en ;
                       rdfs:label "Animal training skill"@en .


###  https://raw.githubusercontent.com/AbsVahter/ontoTRPG/main/crown_and_skull/crown_and_skull.ttl#skill_armorer
:skill_armorer rdf:type owl:NamedIndividual ,
                        :SkillBasic ;
               rdfs:comment "In arm’s length of an ally, roll this skill to repair 1 damaged armor item in their inventory. On a failure, the armor is destroyed."@en ;
               rdfs:label "Armorer skill"@en .


###  https://raw.githubusercontent.com/AbsVahter/ontoTRPG/main/crown_and_skull/crown_and_skull.ttl#skill_brawling
:skill_brawling rdf:type owl:NamedIndividual ,
                         :SkillBasic ;
                rdfs:comment "Fight with fists and feet. Two uses: 1) Roll the skill to grapple or stun a foe for 1 round. 2) Use a D6 when attacking without a weapon."@en ;
                rdfs:label "Brawling skill"@en .


###  https://raw.githubusercontent.com/AbsVahter/ontoTRPG/main/crown_and_skull/crown_and_skull.ttl#skill_breakfall
:skill_breakfall rdf:type owl:NamedIndividual ,
                          :SkillBasic ;
                 rdfs:comment "Half damage taken in long falls if this skill rolled successfully."@en ;
                 rdfs:label "Breakfall skill"@en .


###  https://raw.githubusercontent.com/AbsVahter/ontoTRPG/main/crown_and_skull/crown_and_skull.ttl#skill_climber
:skill_climber rdf:type owl:NamedIndividual ,
                        :SkillBasic ;
               rdfs:comment "Climb any reasonable surface with texture, holds, or crevasses."@en ;
               rdfs:label "Climber skill"@en .


###  https://raw.githubusercontent.com/AbsVahter/ontoTRPG/main/crown_and_skull/crown_and_skull.ttl#skill_companion_attack
:skill_companion_attack rdf:type owl:NamedIndividual ,
                                 :SkillCompanion ;
                        rdfs:comment "Roll damage with natural weapons."@en ;
                        rdfs:label "Attack"@en .


###  https://raw.githubusercontent.com/AbsVahter/ontoTRPG/main/crown_and_skull/crown_and_skull.ttl#skill_companion_carry
:skill_companion_carry rdf:type owl:NamedIndividual ,
                                :SkillCompanion ;
                       rdfs:comment "This companion can carry its weight or less with ease."@en ;
                       rdfs:label "Carry"@en .


###  https://raw.githubusercontent.com/AbsVahter/ontoTRPG/main/crown_and_skull/crown_and_skull.ttl#skill_companion_endure
:skill_companion_endure rdf:type owl:NamedIndividual ,
                                 :SkillCompanion ;
                        rdfs:comment "This companion gains a +1 protective attrition against a lethal hit."@en ;
                        rdfs:label "Endure"@en .


###  https://raw.githubusercontent.com/AbsVahter/ontoTRPG/main/crown_and_skull/crown_and_skull.ttl#skill_companion_find
:skill_companion_find rdf:type owl:NamedIndividual ,
                               :SkillCompanion ;
                      rdfs:comment "Locate a person or object in 1D4 rounds."@en ;
                      rdfs:label "Find"@en .


###  https://raw.githubusercontent.com/AbsVahter/ontoTRPG/main/crown_and_skull/crown_and_skull.ttl#skill_companion_frighten
:skill_companion_frighten rdf:type owl:NamedIndividual ,
                                   :SkillCompanion ;
                          rdfs:comment "With a roll, scare a foe into hesitating for 1 round."@en ;
                          rdfs:label "Frighten"@en .


###  https://raw.githubusercontent.com/AbsVahter/ontoTRPG/main/crown_and_skull/crown_and_skull.ttl#skill_companion_hunt
:skill_companion_hunt rdf:type owl:NamedIndividual ,
                               :SkillCompanion ;
                      rdfs:comment "Once per day, this companion can feed a group with its efforts."@en ;
                      rdfs:label "Hunt"@en .


###  https://raw.githubusercontent.com/AbsVahter/ontoTRPG/main/crown_and_skull/crown_and_skull.ttl#skill_companion_pin_down
:skill_companion_pin_down rdf:type owl:NamedIndividual ,
                                   :SkillCompanion ;
                          rdfs:comment "Roll to pounce on a foe and pin it. Versus rolls encouraged."@en ;
                          rdfs:label "Pin Down"@en .


###  https://raw.githubusercontent.com/AbsVahter/ontoTRPG/main/crown_and_skull/crown_and_skull.ttl#skill_companion_protect
:skill_companion_protect rdf:type owl:NamedIndividual ,
                                  :SkillCompanion ;
                         rdfs:comment "The companion clings to its charge, taking damage when possible."@en ;
                         rdfs:label "Protect"@en .


###  https://raw.githubusercontent.com/AbsVahter/ontoTRPG/main/crown_and_skull/crown_and_skull.ttl#skill_companion_report
:skill_companion_report rdf:type owl:NamedIndividual ,
                                 :SkillCompanion ;
                        rdfs:comment "In 1D4 rounds, scout the area and report back in simple terms."@en ;
                        rdfs:label "Report"@en .


###  https://raw.githubusercontent.com/AbsVahter/ontoTRPG/main/crown_and_skull/crown_and_skull.ttl#skill_companion_retrieve
:skill_companion_retrieve rdf:type owl:NamedIndividual ,
                                   :SkillCompanion ;
                          rdfs:comment "Roll to recover an object of equal or smaller mass."@en ;
                          rdfs:label "Retrieve"@en .


###  https://raw.githubusercontent.com/AbsVahter/ontoTRPG/main/crown_and_skull/crown_and_skull.ttl#skill_companion_stand_watch
:skill_companion_stand_watch rdf:type owl:NamedIndividual ,
                                      :SkillCompanion ;
                             rdfs:comment "This companion reliably keeps guard, alerting at any event."@en ;
                             rdfs:label "Stand Watch"@en .


###  https://raw.githubusercontent.com/AbsVahter/ontoTRPG/main/crown_and_skull/crown_and_skull.ttl#skill_companion_taunt
:skill_companion_taunt rdf:type owl:NamedIndividual ,
                                :SkillCompanion ;
                       rdfs:comment "With a roll, require a foe to attack for 1 round."@en ;
                       rdfs:label "Taunt"@en .


###  https://raw.githubusercontent.com/AbsVahter/ontoTRPG/main/crown_and_skull/crown_and_skull.ttl#skill_companion_track
:skill_companion_track rdf:type owl:NamedIndividual ,
                                :SkillCompanion ;
                       rdfs:comment "Roll to reliably follow a designated quarry for 1 round."@en ;
                       rdfs:label "Track"@en .


###  https://raw.githubusercontent.com/AbsVahter/ontoTRPG/main/crown_and_skull/crown_and_skull.ttl#skill_courtier
:skill_courtier rdf:type owl:NamedIndividual ,
                         :SkillBasic ;
                rdfs:comment "Roll to outwit bureaucrats or royalty."@en ;
                rdfs:label "Courtier skill"@en .


###  https://raw.githubusercontent.com/AbsVahter/ontoTRPG/main/crown_and_skull/crown_and_skull.ttl#skill_disguise
:skill_disguise rdf:type owl:NamedIndividual ,
                         :SkillBasic ;
                rdfs:comment "Take on alternate identities. More difficult with acquaintances."@en ;
                rdfs:label "Disguise skill"@en .


###  https://raw.githubusercontent.com/AbsVahter/ontoTRPG/main/crown_and_skull/crown_and_skull.ttl#skill_evade
:skill_evade rdf:type owl:NamedIndividual ,
                      :SkillBasic ;
             rdfs:comment "Used to avoid attacks that armor cannot protect against."@en ;
             rdfs:label "Evade skill"@en .


###  https://raw.githubusercontent.com/AbsVahter/ontoTRPG/main/crown_and_skull/crown_and_skull.ttl#skill_faith
:skill_faith rdf:type owl:NamedIndividual ,
                      :SkillBasic ;
             rdfs:comment "The ability to call forth miracles with prayer (see Divine Magic)."@en ,
                          "format = (maximum value, current value, temporal value)"@en ,
                          "temporal value >= current value"@en ;
             rdfs:label "Faith skill"@en .


###  https://raw.githubusercontent.com/AbsVahter/ontoTRPG/main/crown_and_skull/crown_and_skull.ttl#skill_forage
:skill_forage rdf:type owl:NamedIndividual ,
                       :SkillBasic ;
              rdfs:comment "A skill used to find plants in the Herbalists’ Guide."@en ;
              rdfs:label "Forage skill"@en .


###  https://raw.githubusercontent.com/AbsVahter/ontoTRPG/main/crown_and_skull/crown_and_skull.ttl#skill_gambling
:skill_gambling rdf:type owl:NamedIndividual ,
                         :SkillBasic ;
                rdfs:comment "Cheat or overcome casino games with devious attention."@en ;
                rdfs:label "Gambling skill"@en .


###  https://raw.githubusercontent.com/AbsVahter/ontoTRPG/main/crown_and_skull/crown_and_skull.ttl#skill_hunting
:skill_hunting rdf:type owl:NamedIndividual ,
                        :SkillBasic ;
               rdfs:comment "Acquire food in natural environments, enough for a group."@en ;
               rdfs:label "Hunting skill"@en .


###  https://raw.githubusercontent.com/AbsVahter/ontoTRPG/main/crown_and_skull/crown_and_skull.ttl#skill_investigate
:skill_investigate rdf:type owl:NamedIndividual ,
                            :SkillBasic ;
                   rdfs:comment "Uncover hidden information, history or subtle facts."@en ;
                   rdfs:label "Investigate skill"@en .


###  https://raw.githubusercontent.com/AbsVahter/ontoTRPG/main/crown_and_skull/crown_and_skull.ttl#skill_jump
:skill_jump rdf:type owl:NamedIndividual ,
                     :SkillBasic ;
            rdfs:comment "Leap with uncanny agility, out-jumping the untrained by 3-fold."@en ;
            rdfs:label "Jump skill"@en .


###  https://raw.githubusercontent.com/AbsVahter/ontoTRPG/main/crown_and_skull/crown_and_skull.ttl#skill_knowledge
:skill_knowledge rdf:type owl:NamedIndividual ,
                          :SkillBasic ;
                 rdfs:comment "Roll to recall details on a single topic or area of expertise."@en ;
                 rdfs:label "Knowledge skill"@en .


###  https://raw.githubusercontent.com/AbsVahter/ontoTRPG/main/crown_and_skull/crown_and_skull.ttl#skill_languages
:skill_languages rdf:type owl:NamedIndividual ,
                          :SkillBasic ;
                 rdfs:comment "Be fluent with a successful roll. Only spend here for languages outside what would be normal for your folk to speak."@en ;
                 rdfs:label "Languages skill"@en .


###  https://raw.githubusercontent.com/AbsVahter/ontoTRPG/main/crown_and_skull/crown_and_skull.ttl#skill_linguist
:skill_linguist rdf:type owl:NamedIndividual ,
                         :SkillBasic ;
                rdfs:comment "Discern lost or unknown language, glyphs, or writing."@en ;
                rdfs:label "Linguist skill"@en .


###  https://raw.githubusercontent.com/AbsVahter/ontoTRPG/main/crown_and_skull/crown_and_skull.ttl#skill_lockpicking
:skill_lockpicking rdf:type owl:NamedIndividual ,
                            :SkillBasic ;
                   rdfs:comment "Disable non-magical locking devices with tools."@en ;
                   rdfs:label "Lockpicking skill"@en .


###  https://raw.githubusercontent.com/AbsVahter/ontoTRPG/main/crown_and_skull/crown_and_skull.ttl#skill_magic
:skill_magic rdf:type owl:NamedIndividual ,
                      :SkillBasic ;
             rdfs:comment "Used to contain infernal or unstable magic, or as a resistance to spells. Also used for wild magic and anti-magic."@en ;
             rdfs:label "Magic skill"@en .


###  https://raw.githubusercontent.com/AbsVahter/ontoTRPG/main/crown_and_skull/crown_and_skull.ttl#skill_medical
:skill_medical rdf:type owl:NamedIndividual ,
                        :SkillBasic ;
               rdfs:comment "Recover a crossed-off skill on yourself or an ally, with a touch. A failed roll renders that skill recoverable only by rest."@en ;
               rdfs:label "Medical skill"@en .


###  https://raw.githubusercontent.com/AbsVahter/ontoTRPG/main/crown_and_skull/crown_and_skull.ttl#skill_mining
:skill_mining rdf:type owl:NamedIndividual ,
                       :SkillBasic ;
              rdfs:comment "Navigate or excavate underground with perfect direction and skill."@en ;
              rdfs:label "Mining skill"@en .


###  https://raw.githubusercontent.com/AbsVahter/ontoTRPG/main/crown_and_skull/crown_and_skull.ttl#skill_muscle
:skill_muscle rdf:type owl:NamedIndividual ,
                       :SkillBasic ;
              rdfs:comment "You have a knack for leverage, a powerful grip, and raw strength. Roll this skill to bend bars, lift the unliftable, or brace against wind."@en ;
              rdfs:label "Muscle skill"@en .


###  https://raw.githubusercontent.com/AbsVahter/ontoTRPG/main/crown_and_skull/crown_and_skull.ttl#skill_oratory
:skill_oratory rdf:type owl:NamedIndividual ,
                        :SkillBasic ;
               rdfs:comment "Fascinate or deceive with stories, bravado and sheer charisma."@en ;
               rdfs:label "Oratory skill"@en .


###  https://raw.githubusercontent.com/AbsVahter/ontoTRPG/main/crown_and_skull/crown_and_skull.ttl#skill_pickpocket
:skill_pickpocket rdf:type owl:NamedIndividual ,
                           :SkillBasic ;
                  rdfs:comment "Acquire small or simple items on unsuspecting targets."@en ;
                  rdfs:label "Pickpocket skill"@en .


###  https://raw.githubusercontent.com/AbsVahter/ontoTRPG/main/crown_and_skull/crown_and_skull.ttl#skill_profession
:skill_profession rdf:type owl:NamedIndividual ,
                           :SkillBasic ;
                  rdfs:comment "Any working skill or commerce skill, its tools and ways."@en ;
                  rdfs:label "Profession skill"@en .


###  https://raw.githubusercontent.com/AbsVahter/ontoTRPG/main/crown_and_skull/crown_and_skull.ttl#skill_repair
:skill_repair rdf:type owl:NamedIndividual ,
                       :SkillBasic ;
              rdfs:comment "Mend a damaged weapon or item. Not usable on armor. A failed roll destroys the item. “I think I dropped a piece...”"@en ;
              rdfs:label "Repair skill"@en .


###  https://raw.githubusercontent.com/AbsVahter/ontoTRPG/main/crown_and_skull/crown_and_skull.ttl#skill_resist
:skill_resist rdf:type owl:NamedIndividual ,
                       :SkillBasic ;
              rdfs:comment "You are hearty. Roll to ignore extreme cold, poison, or too many mugs of ale. Hold your breath or fight back harmful magic with Resist."@en ;
              rdfs:label "Resist skill"@en .


###  https://raw.githubusercontent.com/AbsVahter/ontoTRPG/main/crown_and_skull/crown_and_skull.ttl#skill_riding
:skill_riding rdf:type owl:NamedIndividual ,
                       :SkillBasic ;
              rdfs:comment "Perform daring maneuvers on horseback without penalties."@en ;
              rdfs:label "Riding skill"@en .


###  https://raw.githubusercontent.com/AbsVahter/ontoTRPG/main/crown_and_skull/crown_and_skull.ttl#skill_roll_penalty
:skill_roll_penalty rdf:type owl:NamedIndividual ;
                    rdfs:label "Penalty to skill roll"@en ;
                    gen:valueFormula "zero by default" .


###  https://raw.githubusercontent.com/AbsVahter/ontoTRPG/main/crown_and_skull/crown_and_skull.ttl#skill_running
:skill_running rdf:type owl:NamedIndividual ,
                        :SkillBasic ;
               rdfs:comment "Run double the distance of others, outrun pursuers in the open."@en ;
               rdfs:label "Running skill"@en .


###  https://raw.githubusercontent.com/AbsVahter/ontoTRPG/main/crown_and_skull/crown_and_skull.ttl#skill_sailing
:skill_sailing rdf:type owl:NamedIndividual ,
                        :SkillBasic ;
               rdfs:comment "Operate marine vessels, with appropriate crew."@en ;
               rdfs:label "Sailing skill"@en .


###  https://raw.githubusercontent.com/AbsVahter/ontoTRPG/main/crown_and_skull/crown_and_skull.ttl#skill_scholar
:skill_scholar rdf:type owl:NamedIndividual ,
                        :SkillBasic ;
               rdfs:comment "Achieve renown in a specific topic. You are published."@en ;
               rdfs:label "Scholar skill"@en .


###  https://raw.githubusercontent.com/AbsVahter/ontoTRPG/main/crown_and_skull/crown_and_skull.ttl#skill_scout
:skill_scout rdf:type owl:NamedIndividual ,
                      :SkillBasic ;
             rdfs:comment "Find all kinds of clues, information, or traps in the immediate area."@en ;
             rdfs:label "Scout skill"@en .


###  https://raw.githubusercontent.com/AbsVahter/ontoTRPG/main/crown_and_skull/crown_and_skull.ttl#skill_shield_fighting
:skill_shield_fighting rdf:type owl:NamedIndividual ,
                                :SkillBasic ;
                       rdfs:comment "When using a shield, roll this skill instead of Defense. Additionally, add the Defense bonus of your shield to this skill."@en ;
                       rdfs:label "Shield fighting skill"@en ;
                       gen:input :equipment ;
                       gen:modified :threshold_defense ;
                       gen:prerequisiteDescription "worn shield" ;
                       gen:valueFormula "formula: max(defense, shield fighting skill + shield defense) - (penalty to defense)" ;
                       gen:valueObject gen:valueFormula .


###  https://raw.githubusercontent.com/AbsVahter/ontoTRPG/main/crown_and_skull/crown_and_skull.ttl#skill_skinning
:skill_skinning rdf:type owl:NamedIndividual ,
                         :SkillBasic ;
                rdfs:comment "Harvest a slain beast for pelt or hide in 1D4 rounds."@en ;
                rdfs:label "Skinning skill"@en .


###  https://raw.githubusercontent.com/AbsVahter/ontoTRPG/main/crown_and_skull/crown_and_skull.ttl#skill_spell_research
:skill_spell_research rdf:type owl:NamedIndividual ,
                               :SkillBasic ;
                      rdfs:comment "Roll to study spells with time and materials in a safe place. Gain 1 hero point per day invested thus, spendable only on spells."@en ;
                      rdfs:label "Spell research skill"@en .


###  https://raw.githubusercontent.com/AbsVahter/ontoTRPG/main/crown_and_skull/crown_and_skull.ttl#skill_stealth
:skill_stealth rdf:type owl:NamedIndividual ,
                        :SkillBasic ;
               rdfs:comment "Go unnoticed when moving. Easier if perfectly still or hidden."@en ;
               rdfs:label "Stealth skill"@en .


###  https://raw.githubusercontent.com/AbsVahter/ontoTRPG/main/crown_and_skull/crown_and_skull.ttl#skill_streetwise
:skill_streetwise rdf:type owl:NamedIndividual ,
                           :SkillBasic ;
                  rdfs:comment "You know shady people and back-alley secrets."@en ;
                  rdfs:label "Streetwise skill"@en .


###  https://raw.githubusercontent.com/AbsVahter/ontoTRPG/main/crown_and_skull/crown_and_skull.ttl#skill_survival
:skill_survival rdf:type owl:NamedIndividual ,
                         :SkillBasic ;
                rdfs:comment "If your heart is hit, a lethal injury, roll this skill instantly (it will be crossed off). On a success, you fight off death’s embrace for 1 round. Also rolled when refusing to rest and pushing onward after lack of sleep."@en ;
                rdfs:label "Survival skill"@en ;
                gen:modified :death_of_pc .


###  https://raw.githubusercontent.com/AbsVahter/ontoTRPG/main/crown_and_skull/crown_and_skull.ttl#skill_swimming
:skill_swimming rdf:type owl:NamedIndividual ,
                         :SkillBasic ;
                rdfs:comment "Swim twice as far as others. Stay underwater twice as long."@en ;
                rdfs:label "Swimming skill"@en .


###  https://raw.githubusercontent.com/AbsVahter/ontoTRPG/main/crown_and_skull/crown_and_skull.ttl#skill_take_aim
:skill_take_aim rdf:type owl:NamedIndividual ,
                         :SkillBasic ;
                rdfs:comment "Add a die of your attack type on the next attack you make."@en ;
                rdfs:label "Take aim skill"@en .


###  https://raw.githubusercontent.com/AbsVahter/ontoTRPG/main/crown_and_skull/crown_and_skull.ttl#skill_tracking
:skill_tracking rdf:type owl:NamedIndividual ,
                         :SkillBasic ;
                rdfs:comment "Find obscured foes in the wild."@en ;
                rdfs:label "Tracking skill"@en .


###  https://raw.githubusercontent.com/AbsVahter/ontoTRPG/main/crown_and_skull/crown_and_skull.ttl#skill_trading
:skill_trading rdf:type owl:NamedIndividual ,
                        :SkillBasic ;
               rdfs:comment "Get more value out of trade despite hagglers, bad leverage, distractions or scammers."@en ;
               rdfs:label "Trading skill"@en .


###  https://raw.githubusercontent.com/AbsVahter/ontoTRPG/main/crown_and_skull/crown_and_skull.ttl#skills
:skills rdf:type owl:NamedIndividual ,
                 gen:ParameterPC ;
        rdfs:comment "format = {skill: {level: 3..18; status: non-crossed, crossed, recoverable only by rest}}"@en ;
        rdfs:label "Skills"@en .


###  https://raw.githubusercontent.com/AbsVahter/ontoTRPG/main/crown_and_skull/crown_and_skull.ttl#skull
:skull rdf:type owl:NamedIndividual ;
       rdfs:comment "Those who choose the SKULL will join no order, swear allegiance to no one, and walk the world as a masterless rogue. They will spare no method or dark power to see their deeds done. They trust their own wisdom over the laws of kingdoms or motives of kings. Free to choose their own path, they will be honored by others who stand defiant, self-contained." ;
       rdfs:label "Skull"@en ;
       gen:included :skull_gain_ring ,
                    :skull_gaining_hero_points ,
                    :skull_select_equipment ,
                    :skull_select_skill ,
                    :skull_set_flaw .


###  https://raw.githubusercontent.com/AbsVahter/ontoTRPG/main/crown_and_skull/crown_and_skull.ttl#skull_gain_ring
:skull_gain_ring rdf:type owl:NamedIndividual ;
                 rdfs:label "Skull: gaining Ring of the Skull"@en ;
                 gen:Actor gen:player ;
                 gen:setAdditive :equipment ;
                 gen:valueObject :ring_skull .


###  https://raw.githubusercontent.com/AbsVahter/ontoTRPG/main/crown_and_skull/crown_and_skull.ttl#skull_gaining_hero_points
:skull_gaining_hero_points rdf:type owl:NamedIndividual ;
                           rdfs:label "Skull: gaining hero points"@en ;
                           gen:Actor gen:master ;
                           gen:setAdditive :hero_points ;
                           gen:valueNumeric 9 .


###  https://raw.githubusercontent.com/AbsVahter/ontoTRPG/main/crown_and_skull/crown_and_skull.ttl#skull_select_equipment
:skull_select_equipment rdf:type owl:NamedIndividual ;
                        rdfs:label "Skull: choosing equipment"@en ;
                        gen:Actor gen:player ;
                        gen:inputOption :ItemSkull ;
                        gen:setAdditive :equipment ;
                        gen:valueFormula "1 item" .


###  https://raw.githubusercontent.com/AbsVahter/ontoTRPG/main/crown_and_skull/crown_and_skull.ttl#skull_select_skill
:skull_select_skill rdf:type owl:NamedIndividual ;
                    rdfs:label "Skull: choosing skill"@en ;
                    gen:Actor gen:player ;
                    gen:inputOption :SkillSkull ;
                    gen:setAdditive :skills ;
                    gen:valueFormula "1 skull skill with level 9" ;
                    gen:valueNumeric 9 .


###  https://raw.githubusercontent.com/AbsVahter/ontoTRPG/main/crown_and_skull/crown_and_skull.ttl#skull_set_flaw
:skull_set_flaw rdf:type owl:NamedIndividual ;
                rdfs:label "Skull: set Ronin flaw"@en ;
                gen:Actor gen:player ;
                gen:setAdditive :flaws ;
                gen:valueObject :flaw_ronin .


###  https://raw.githubusercontent.com/AbsVahter/ontoTRPG/main/crown_and_skull/crown_and_skull.ttl#slimshire
:slimshire rdf:type owl:NamedIndividual ,
                    gen:Location ;
           rdfs:comment "The coming of the ‘White Bird’ and The Holy Order has grown this town, once a wide spot in the road to Hakburg, to new heights. Ruling here is Lord Pickins, and times have been good. Such fortune has attracted the destructive attention of goblins from the Shadow Glades, Orc raiders from the deep desert, and even the darkly dreaming infl uence of a mysterious entity generally referred to as ‘the eye in the well.’ To call this town home, you will be confronting vampiric cults, fi ghting goblin skirmishers, or working to secure allies in the war with the Orcs."@en ;
           rdfs:label "Slimshire, High Plains Outpost"@en ;
           gen:included :bee_spoke ,
                        :dunsel_and_kid .


###  https://raw.githubusercontent.com/AbsVahter/ontoTRPG/main/crown_and_skull/crown_and_skull.ttl#slimshire_threat
:slimshire_threat rdf:type owl:NamedIndividual ;
                  rdfs:comment "As Slimshire has reached the apogee of its prosperity though, a dark force has emboldened goblins from the Shadow Glades and orc raiders from the remnants of Dalric’s Wall. To make things worse, Lord Pickins has been seen less and less of late, cloistered with his ailing daughter Kay, who, according to rumor, has been afflicted with a vampiric sickness."@en ;
                  rdfs:label "Threat at Slimshire"@en ;
                  gen:Location :slimshire .


###  https://raw.githubusercontent.com/AbsVahter/ontoTRPG/main/crown_and_skull/crown_and_skull.ttl#spell_arcane_lock
:spell_arcane_lock rdf:type owl:NamedIndividual ,
                            :Spell ;
                   rdfs:comment "A glyph used to permanently seal a door"@en ;
                   rdfs:label "Arcane Lock"@en ;
                   gen:cost "3 hero points" .


###  https://raw.githubusercontent.com/AbsVahter/ontoTRPG/main/crown_and_skull/crown_and_skull.ttl#spell_armor
:spell_armor rdf:type owl:NamedIndividual ,
                      :Spell ;
             rdfs:comment "Add +3 Defense"@en ;
             rdfs:label "Armor"@en ;
             gen:cost "3 hero points" .


###  https://raw.githubusercontent.com/AbsVahter/ontoTRPG/main/crown_and_skull/crown_and_skull.ttl#spell_consequence_infernal_charred
:spell_consequence_infernal_charred rdf:type owl:NamedIndividual ,
                                             :SpellConsequenceInfernal ;
                                    rdfs:comment "Terrible burn... reduce skill inventory by 1 permanently."@en ;
                                    rdfs:label "Charred"@en .


###  https://raw.githubusercontent.com/AbsVahter/ontoTRPG/main/crown_and_skull/crown_and_skull.ttl#spell_consequence_infernal_devilish
:spell_consequence_infernal_devilish rdf:type owl:NamedIndividual ,
                                              :SpellConsequenceInfernal ;
                                     rdfs:comment "Your appearance slightly changes: a hint of horns, a glow to the eyes, black fingernails, crab-claw fingers, or scaly skin."@en ;
                                     rdfs:label "Devilish"@en .


###  https://raw.githubusercontent.com/AbsVahter/ontoTRPG/main/crown_and_skull/crown_and_skull.ttl#spell_consequence_infernal_hellrift
:spell_consequence_infernal_hellrift rdf:type owl:NamedIndividual ,
                                              :SpellConsequenceInfernal ;
                                     rdfs:comment "A powerful baron of hell appears, furious. It has 20 HP, actions on phases 2 and 4, and does D12 sword damage."@en ;
                                     rdfs:label "Hellrift"@en .


###  https://raw.githubusercontent.com/AbsVahter/ontoTRPG/main/crown_and_skull/crown_and_skull.ttl#spell_consequence_infernal_hellstone
:spell_consequence_infernal_hellstone rdf:type owl:NamedIndividual ,
                                               :SpellConsequenceInfernal ;
                                      rdfs:comment "A mass of smoldering rock falls from above! It smashes a random area in 1D6 phases, inflicting 2 attrition on those below."@en ;
                                      rdfs:label "Hellstone"@en .


###  https://raw.githubusercontent.com/AbsVahter/ontoTRPG/main/crown_and_skull/crown_and_skull.ttl#spell_consequence_infernal_imps
:spell_consequence_infernal_imps rdf:type owl:NamedIndividual ,
                                          :SpellConsequenceInfernal ;
                                 rdfs:comment "2D6 1 HP imps materialize and attack you. They do not make rolls, fly about like bats, and inflict 1 attrition per bite."@en ;
                                 rdfs:label "Imps"@en .


###  https://raw.githubusercontent.com/AbsVahter/ontoTRPG/main/crown_and_skull/crown_and_skull.ttl#spell_consequence_infernal_inert
:spell_consequence_infernal_inert rdf:type owl:NamedIndividual ,
                                           :SpellConsequenceInfernal ;
                                  rdfs:comment "Nothing happens, save a wisp of smoke."@en ;
                                  rdfs:label "Inert"@en .


###  https://raw.githubusercontent.com/AbsVahter/ontoTRPG/main/crown_and_skull/crown_and_skull.ttl#spell_consequence_infernal_pain
:spell_consequence_infernal_pain rdf:type owl:NamedIndividual ,
                                          :SpellConsequenceInfernal ;
                                 rdfs:comment "Heat and sparks sear your flesh for 1 item attrition."@en ;
                                 rdfs:label "Pain"@en .


###  https://raw.githubusercontent.com/AbsVahter/ontoTRPG/main/crown_and_skull/crown_and_skull.ttl#spell_consequence_infernal_smoke_cloud
:spell_consequence_infernal_smoke_cloud rdf:type owl:NamedIndividual ,
                                                 :SpellConsequenceInfernal ;
                                        rdfs:comment "A large cloud of opaque smoke surrounds you."@en ;
                                        rdfs:label "Smoke Cloud"@en .


###  https://raw.githubusercontent.com/AbsVahter/ontoTRPG/main/crown_and_skull/crown_and_skull.ttl#spell_consequence_unstable_dud
:spell_consequence_unstable_dud rdf:type owl:NamedIndividual ,
                                         :SpellConsequenceUnstable ;
                                rdfs:comment "The cast fails, and expends itself."@en ;
                                rdfs:label "A dud"@en .


###  https://raw.githubusercontent.com/AbsVahter/ontoTRPG/main/crown_and_skull/crown_and_skull.ttl#spell_consequence_unstable_echo
:spell_consequence_unstable_echo rdf:type owl:NamedIndividual ,
                                          :SpellConsequenceUnstable ;
                                 rdfs:comment "A searing, loud noise erupts, heard for miles."@en ;
                                 rdfs:label "Echo"@en .


###  https://raw.githubusercontent.com/AbsVahter/ontoTRPG/main/crown_and_skull/crown_and_skull.ttl#spell_consequence_unstable_erosion
:spell_consequence_unstable_erosion rdf:type owl:NamedIndividual ,
                                             :SpellConsequenceUnstable ;
                                    rdfs:comment "The spell itself is damaged. Roll to add a new limitation."@en ;
                                    rdfs:label "Erosion"@en .


###  https://raw.githubusercontent.com/AbsVahter/ontoTRPG/main/crown_and_skull/crown_and_skull.ttl#spell_consequence_unstable_forgetful
:spell_consequence_unstable_forgetful rdf:type owl:NamedIndividual ,
                                               :SpellConsequenceUnstable ;
                                      rdfs:comment "You forget how to cast this spell for 1D4 days. For each of those days, roll Investigation to try and remember."@en ;
                                      rdfs:label "Forgetful"@en .


###  https://raw.githubusercontent.com/AbsVahter/ontoTRPG/main/crown_and_skull/crown_and_skull.ttl#spell_consequence_unstable_psychic_spike
:spell_consequence_unstable_psychic_spike rdf:type owl:NamedIndividual ,
                                                   :SpellConsequenceUnstable ;
                                          rdfs:comment "Your mind reels from failed magic. Take a -3 penalty to your Magic skill until your next rest."@en ;
                                          rdfs:label "Psychic Spike"@en .


###  https://raw.githubusercontent.com/AbsVahter/ontoTRPG/main/crown_and_skull/crown_and_skull.ttl#spell_consequence_unstable_spellblast
:spell_consequence_unstable_spellblast rdf:type owl:NamedIndividual ,
                                                :SpellConsequenceUnstable ;
                                       rdfs:comment "Explosion! Absorb 2 attrition. The blast is large, reaching to ‘near’ distance."@en ;
                                       rdfs:label "Spellblast"@en .


###  https://raw.githubusercontent.com/AbsVahter/ontoTRPG/main/crown_and_skull/crown_and_skull.ttl#spell_consequence_unstable_stable
:spell_consequence_unstable_stable rdf:type owl:NamedIndividual ,
                                            :SpellConsequenceUnstable ;
                                   rdfs:comment "Your spell casts normally, with no unstable aspects."@en ;
                                   rdfs:label "Stable"@en .


###  https://raw.githubusercontent.com/AbsVahter/ontoTRPG/main/crown_and_skull/crown_and_skull.ttl#spell_consequence_unstable_wild_shot
:spell_consequence_unstable_wild_shot rdf:type owl:NamedIndividual ,
                                               :SpellConsequenceUnstable ;
                                      rdfs:comment "The spell fires at a random target or area, including allies."@en ;
                                      rdfs:label "Wild Shot"@en .


###  https://raw.githubusercontent.com/AbsVahter/ontoTRPG/main/crown_and_skull/crown_and_skull.ttl#spell_courage
:spell_courage rdf:type owl:NamedIndividual ,
                        :Spell ;
               rdfs:comment "Ignore fear or intimidation"@en ;
               rdfs:label "Courage"@en ;
               gen:cost "3 hero points" .


###  https://raw.githubusercontent.com/AbsVahter/ontoTRPG/main/crown_and_skull/crown_and_skull.ttl#spell_custom
:spell_custom rdf:type owl:NamedIndividual ,
                       :Spell ;
              rdfs:label "Custom spell"@en .


###  https://raw.githubusercontent.com/AbsVahter/ontoTRPG/main/crown_and_skull/crown_and_skull.ttl#spell_dream_spike
:spell_dream_spike rdf:type owl:NamedIndividual ,
                            :Spell ;
                   rdfs:comment "Stun an intelligent foe"@en ;
                   rdfs:label "Dream Spike"@en ;
                   gen:cost "3 hero points" .


###  https://raw.githubusercontent.com/AbsVahter/ontoTRPG/main/crown_and_skull/crown_and_skull.ttl#spell_far_seer
:spell_far_seer rdf:type owl:NamedIndividual ,
                         :Spell ;
                rdfs:comment "See your position from high above"@en ;
                rdfs:label "Far-Seer"@en ;
                gen:cost "3 hero points" .


###  https://raw.githubusercontent.com/AbsVahter/ontoTRPG/main/crown_and_skull/crown_and_skull.ttl#spell_fireblast
:spell_fireblast rdf:type owl:NamedIndividual ,
                          :Spell ;
                 rdfs:comment "Explosive fire from the caster’s hands"@en ;
                 rdfs:label "Fireblast"@en ;
                 gen:cost "3 hero points" .


###  https://raw.githubusercontent.com/AbsVahter/ontoTRPG/main/crown_and_skull/crown_and_skull.ttl#spell_ghost_blade
:spell_ghost_blade rdf:type owl:NamedIndividual ,
                            :Spell ;
                   rdfs:comment "Hit 1D2 targets with arcane knives"@en ;
                   rdfs:label "Ghost Blade"@en ;
                   gen:cost "3 hero points" .


###  https://raw.githubusercontent.com/AbsVahter/ontoTRPG/main/crown_and_skull/crown_and_skull.ttl#spell_healing_light
:spell_healing_light rdf:type owl:NamedIndividual ,
                              :Spell ;
                     rdfs:comment "Heal a skill attrition with a touch"@en ;
                     rdfs:label "Healing Light"@en ;
                     gen:cost "3 hero points" .


###  https://raw.githubusercontent.com/AbsVahter/ontoTRPG/main/crown_and_skull/crown_and_skull.ttl#spell_invisible_wall
:spell_invisible_wall rdf:type owl:NamedIndividual ,
                               :Spell ;
                      rdfs:comment "A 20’ wide force field, 4 attrition/10 Def"@en ;
                      rdfs:label "Invisible Wall"@en ;
                      gen:cost "3 hero points" .


###  https://raw.githubusercontent.com/AbsVahter/ontoTRPG/main/crown_and_skull/crown_and_skull.ttl#spell_levitation
:spell_levitation rdf:type owl:NamedIndividual ,
                           :Spell ;
                  rdfs:comment "Hover up to 6 feet above ground"@en ;
                  rdfs:label "Levitation"@en ;
                  gen:cost "3 hero points" .


###  https://raw.githubusercontent.com/AbsVahter/ontoTRPG/main/crown_and_skull/crown_and_skull.ttl#spell_mages_cloak
:spell_mages_cloak rdf:type owl:NamedIndividual ,
                            :Spell ;
                   rdfs:comment "Enchant a cape. Its wearer is targeted last"@en ;
                   rdfs:label "Mage’s Cloak"@en ;
                   gen:cost "3 hero points" .


###  https://raw.githubusercontent.com/AbsVahter/ontoTRPG/main/crown_and_skull/crown_and_skull.ttl#spell_piercing_blade
:spell_piercing_blade rdf:type owl:NamedIndividual ,
                               :Spell ;
                      rdfs:comment "Enchant a weapon. It is deadly"@en ;
                      rdfs:label "Piercing Blade"@en ;
                      gen:cost "3 hero points" .


###  https://raw.githubusercontent.com/AbsVahter/ontoTRPG/main/crown_and_skull/crown_and_skull.ttl#spell_purify
:spell_purify rdf:type owl:NamedIndividual ,
                       :Spell ;
              rdfs:comment "Free a target of all afflictions"@en ;
              rdfs:label "Purify"@en ;
              gen:cost "3 hero points" .


###  https://raw.githubusercontent.com/AbsVahter/ontoTRPG/main/crown_and_skull/crown_and_skull.ttl#spell_sprint
:spell_sprint rdf:type owl:NamedIndividual ,
                       :Spell ;
              rdfs:comment "Grant double move speed"@en ;
              rdfs:label "Sprint"@en ;
              gen:cost "3 hero points" .


###  https://raw.githubusercontent.com/AbsVahter/ontoTRPG/main/crown_and_skull/crown_and_skull.ttl#spell_stormcaller
:spell_stormcaller rdf:type owl:NamedIndividual ,
                            :Spell ;
                   rdfs:comment "Conjure a type of weather when outdoors"@en ;
                   rdfs:label "Stormcaller"@en ;
                   gen:cost "3 hero points" .


###  https://raw.githubusercontent.com/AbsVahter/ontoTRPG/main/crown_and_skull/crown_and_skull.ttl#spell_summon_vermin
:spell_summon_vermin rdf:type owl:NamedIndividual ,
                              :Spell ;
                     rdfs:comment "Attract a swarm of local pests"@en ;
                     rdfs:label "Summon Vermin"@en ;
                     gen:cost "3 hero points" .


###  https://raw.githubusercontent.com/AbsVahter/ontoTRPG/main/crown_and_skull/crown_and_skull.ttl#spell_telekineticus
:spell_telekineticus rdf:type owl:NamedIndividual ,
                              :Spell ;
                     rdfs:comment "Move small objects in your immediate area"@en ;
                     rdfs:label "Telekineticus"@en ;
                     gen:cost "3 hero points" .


###  https://raw.githubusercontent.com/AbsVahter/ontoTRPG/main/crown_and_skull/crown_and_skull.ttl#spell_vanish
:spell_vanish rdf:type owl:NamedIndividual ,
                       :Spell ;
              rdfs:comment "Become invisible"@en ;
              rdfs:label "Vanish"@en ;
              gen:cost "5 hero points" .


###  https://raw.githubusercontent.com/AbsVahter/ontoTRPG/main/crown_and_skull/crown_and_skull.ttl#spell_vines
:spell_vines rdf:type owl:NamedIndividual ,
                      :Spell ;
             rdfs:comment "Call up vines that grab passers-through"@en ;
             rdfs:label "Vines"@en ;
             gen:cost "3 hero points" .


###  https://raw.githubusercontent.com/AbsVahter/ontoTRPG/main/crown_and_skull/crown_and_skull.ttl#spell_waterbreath
:spell_waterbreath rdf:type owl:NamedIndividual ,
                            :Spell ;
                   rdfs:comment "Breathe underwater with ease"@en ;
                   rdfs:label "Waterbreath"@en ;
                   gen:cost "3 hero points" .


###  https://raw.githubusercontent.com/AbsVahter/ontoTRPG/main/crown_and_skull/crown_and_skull.ttl#spells
:spells rdf:type owl:NamedIndividual ,
                 gen:ParameterPC ;
        rdfs:comment "format = {spell: number of casts}"@en ;
        rdfs:label "Spells"@en .


###  https://raw.githubusercontent.com/AbsVahter/ontoTRPG/main/crown_and_skull/crown_and_skull.ttl#spending_hero_coin
:spending_hero_coin rdf:type owl:NamedIndividual ;
                    rdfs:label "Spending hero coin"@en ;
                    gen:Actor gen:player ;
                    gen:cost "1" ;
                    gen:effectOption :maximize_roll ,
                                     :reroll ;
                    gen:resource :hero_coin .


###  https://raw.githubusercontent.com/AbsVahter/ontoTRPG/main/crown_and_skull/crown_and_skull.ttl#spending_hero_points
:spending_hero_points rdf:type owl:NamedIndividual ;
                      rdfs:comment "A milestone moment for any character."@en ;
                      rdfs:label "Spending hero points"@en ;
                      gen:Actor gen:player ;
                      gen:included :upgrade_skill ;
                      gen:modified gen:pc ;
                      gen:prerequisiteDescription "can only be spent when resting in a safe place with required facilities or services" ;
                      gen:resource :hero_points .


###  https://raw.githubusercontent.com/AbsVahter/ontoTRPG/main/crown_and_skull/crown_and_skull.ttl#stat_atk
:stat_atk rdf:type owl:NamedIndividual ,
                   gen:ParameterEnemy ;
          rdfs:label "Attack stat"@en .


###  https://raw.githubusercontent.com/AbsVahter/ontoTRPG/main/crown_and_skull/crown_and_skull.ttl#stat_def_enemy
:stat_def_enemy rdf:type owl:NamedIndividual ,
                         gen:ParameterEnemy ;
                rdfs:label "Defense stat of enemy"@en .


###  https://raw.githubusercontent.com/AbsVahter/ontoTRPG/main/crown_and_skull/crown_and_skull.ttl#stat_def_pc
:stat_def_pc rdf:type owl:NamedIndividual ,
                      gen:ParameterPC ;
             rdfs:label "Defense stat of PC"@en ;
             gen:input :equipment ;
             gen:valueFormula "min (6 + (defense value of worn armor); 18)" .


###  https://raw.githubusercontent.com/AbsVahter/ontoTRPG/main/crown_and_skull/crown_and_skull.ttl#stat_hp
:stat_hp rdf:type owl:NamedIndividual ,
                  gen:ParameterDynamic ,
                  gen:ParameterEnemy ;
         rdfs:label "Hit points of enemy"@en .


###  https://raw.githubusercontent.com/AbsVahter/ontoTRPG/main/crown_and_skull/crown_and_skull.ttl#stat_tactics
:stat_tactics rdf:type owl:NamedIndividual ,
                       gen:ParameterEnemy ;
              rdfs:label "Number of actions of enemy per round"@en .


###  https://raw.githubusercontent.com/AbsVahter/ontoTRPG/main/crown_and_skull/crown_and_skull.ttl#status_afraid
:status_afraid rdf:type owl:NamedIndividual ,
                        gen:Status ;
               rdfs:comment "Terrified by extreme horrors, you lose your wits and are forced to use your phase to flee the source of your fear."@en ;
               rdfs:label "Afraid"@en ;
               gen:blocked :hurry ,
                           :perform_action ;
               gen:duration "rolled timer" .


###  https://raw.githubusercontent.com/AbsVahter/ontoTRPG/main/crown_and_skull/crown_and_skull.ttl#status_bleed
:status_bleed rdf:type owl:NamedIndividual ,
                       gen:Status ;
              rdfs:label "Bleed"@en ;
              gen:duration "1d4 rounds" ;
              gen:effect :attrition_flesh .


###  https://raw.githubusercontent.com/AbsVahter/ontoTRPG/main/crown_and_skull/crown_and_skull.ttl#status_burning
:status_burning rdf:type owl:NamedIndividual ,
                         gen:Status ;
                rdfs:label "Burning"@en ;
                gen:duration "1d4 rounds" ;
                gen:effect :attrition_equipment ,
                           :attrition_flesh ;
                gen:valueFormula "every round" .


###  https://raw.githubusercontent.com/AbsVahter/ontoTRPG/main/crown_and_skull/crown_and_skull.ttl#status_close_to_death
:status_close_to_death rdf:type owl:NamedIndividual ,
                                gen:Status ;
                       rdfs:label "Close to death"@en .


###  https://raw.githubusercontent.com/AbsVahter/ontoTRPG/main/crown_and_skull/crown_and_skull.ttl#status_corrosion
:status_corrosion rdf:type owl:NamedIndividual ,
                           gen:Status ;
                  rdfs:comment "Acid, rust, or specifi c types of venom can erode equipment, even if somewhat uncommon in terrain. Acidic ‘drips’ are the most frequently encountered, often found on the ceilings of underground places."@en ;
                  rdfs:label "Corrosion"@en ;
                  gen:duration "1d4 rounds" ;
                  gen:effect :attrition_equipment .


###  https://raw.githubusercontent.com/AbsVahter/ontoTRPG/main/crown_and_skull/crown_and_skull.ttl#status_enemy_focus
:status_enemy_focus rdf:type owl:NamedIndividual ,
                             gen:Status ;
                    rdfs:label "In focus of nearby enemies"@en .


###  https://raw.githubusercontent.com/AbsVahter/ontoTRPG/main/crown_and_skull/crown_and_skull.ttl#status_exhausting
:status_exhausting rdf:type owl:NamedIndividual ,
                            gen:Status ;
                   rdfs:label "Exhausting status"@en .


###  https://raw.githubusercontent.com/AbsVahter/ontoTRPG/main/crown_and_skull/crown_and_skull.ttl#status_freezing
:status_freezing rdf:type owl:NamedIndividual ,
                          gen:Status ;
                 rdfs:comment "Deep cold will numb the fingers and slow the mind without furs or winter clothes."@en ;
                 rdfs:label "Freezing"@en ;
                 gen:duration "until you warm up" ;
                 gen:set :damage_penalty ,
                         :skill_roll_penalty ;
                 gen:valueNumeric 5 .


###  https://raw.githubusercontent.com/AbsVahter/ontoTRPG/main/crown_and_skull/crown_and_skull.ttl#status_grapple
:status_grapple rdf:type owl:NamedIndividual ,
                         gen:Status ;
                rdfs:label "Grappled"@en ;
                gen:duration "1 round" .


###  https://raw.githubusercontent.com/AbsVahter/ontoTRPG/main/crown_and_skull/crown_and_skull.ttl#status_immobilized_by_magic
:status_immobilized_by_magic rdf:type owl:NamedIndividual ,
                                      gen:Status ;
                             rdfs:label "Immobilized by magic"@en ,
                                        "Start be immobilized by magic"@en ;
                             gen:blocked :move ;
                             gen:prerequisiteDescription "appropriate effect of spell" ;
                             gen:set :status_immobilized_by_magic .


###  https://raw.githubusercontent.com/AbsVahter/ontoTRPG/main/crown_and_skull/crown_and_skull.ttl#status_immobilized_by_material_forces
:status_immobilized_by_material_forces rdf:type owl:NamedIndividual ,
                                                gen:Status ;
                                       rdfs:label "Immobilized by material forces"@en ,
                                                  "Start be immobilized by material forces"@en ;
                                       gen:blocked :move ;
                                       gen:prerequisiteDescription "material causes" ;
                                       gen:set :status_immobilized_by_material_forces .


###  https://raw.githubusercontent.com/AbsVahter/ontoTRPG/main/crown_and_skull/crown_and_skull.ttl#status_magic_block
:status_magic_block rdf:type owl:NamedIndividual ,
                             gen:Status ;
                    rdfs:label "Under effect of magic block"@en ;
                    gen:blocked :set_spell ;
                    gen:duration "1d4 rounds" .


###  https://raw.githubusercontent.com/AbsVahter/ontoTRPG/main/crown_and_skull/crown_and_skull.ttl#status_overheated
:status_overheated rdf:type owl:NamedIndividual ,
                            gen:Status ;
                   rdfs:comment "Extreme heat causes a heavy-limbed exhaustion."@en ;
                   rdfs:label "Overheated"@en ;
                   gen:blocked :hurry ;
                   gen:duration "until you cool off" ;
                   gen:set :damage_penalty ,
                           :skill_roll_penalty ;
                   gen:valueNumeric 5 .


###  https://raw.githubusercontent.com/AbsVahter/ontoTRPG/main/crown_and_skull/crown_and_skull.ttl#status_stun
:status_stun rdf:type owl:NamedIndividual ,
                      gen:Status ;
             rdfs:comment "If stunned, you are conscious but concussed, unable to act, barely able to stand."@en ;
             rdfs:label "Under stun effect"@en ;
             gen:duration "1d4 rounds" .


###  https://raw.githubusercontent.com/AbsVahter/ontoTRPG/main/crown_and_skull/crown_and_skull.ttl#status_stun_brawling
:status_stun_brawling rdf:type owl:NamedIndividual ,
                               gen:Status ;
                      rdfs:comment "If stunned, you are conscious but concussed, unable to act, barely able to stand."@en ;
                      rdfs:label "Under stun effect by brawling"@en ;
                      gen:duration "1 round" .


###  https://raw.githubusercontent.com/AbsVahter/ontoTRPG/main/crown_and_skull/crown_and_skull.ttl#status_tether_service_is_not_given
:status_tether_service_is_not_given rdf:type owl:NamedIndividual ,
                                             gen:Status ;
                                    rdfs:comment "If service isn’t given, the tattoo will burn with pain, but cannot kill wizard"@en ;
                                    rdfs:label "Called service by tether is not given"@en ;
                                    gen:duration "until the wizard complies service" ;
                                    gen:prerequisiteDescription "service isn't given" ;
                                    gen:setAdditive :skills ;
                                    gen:valueFormula "(1d4 per round) skill non-crossed -> crossed" .


###  https://raw.githubusercontent.com/AbsVahter/ontoTRPG/main/crown_and_skull/crown_and_skull.ttl#status_vs_haste
:status_vs_haste rdf:type owl:NamedIndividual ,
                          gen:Status ;
                 rdfs:label "Bonus against haste target"@en ;
                 gen:duration "1 round" ;
                 gen:setAdditive :defense_penalty ;
                 gen:valueNumeric 5 .


###  https://raw.githubusercontent.com/AbsVahter/ontoTRPG/main/crown_and_skull/crown_and_skull.ttl#suede_and_saddle
:suede_and_saddle rdf:type owl:NamedIndividual ,
                           gen:Location ;
                  rdfs:comment "Gardenburrow features a women’s social club for food, drink, and reprieve. Any female character may stay here free, gathering information or restocking basic supplies at no charge. The only male allowed in these walls is a bumbling cook named Scooby."@en ;
                  rdfs:label "The Suede & Saddle"@en .


###  https://raw.githubusercontent.com/AbsVahter/ontoTRPG/main/crown_and_skull/crown_and_skull.ttl#tattooing_bargain
:tattooing_bargain rdf:type owl:NamedIndividual ;
                   rdfs:comment "A ‘bargain’ tattoo is seen as a dark omen by many magic users, townspeople, and nobles. If detected, it will cause unfavorable responses from such folk. There may even be schools of magical study or certain academic locations that will deny entry if the tattoo is seen."@en ,
                                "Tattoo ‘contains’ the acquired advancement. If it is destroyed or lost (with a loss of limb, for example) the advancement will be lost."@en ;
                   rdfs:label "Tattooing by bargain"@en ;
                   gen:after :contacting_arcanum ;
                   gen:duration "1d4 rounds" ;
                   gen:input :magic_advancements ;
                   gen:prerequisiteDescription "(no other actions may be taken) and (the wizard will grunt and strain with agony, staying quiet only with Resist rolls)" ;
                   gen:setAdditive :tattoos ;
                   gen:valueFormula "tattoo contains the acquired advancement" .


###  https://raw.githubusercontent.com/AbsVahter/ontoTRPG/main/crown_and_skull/crown_and_skull.ttl#tattooing_tether
:tattooing_tether rdf:type owl:NamedIndividual ;
                  rdfs:comment "If the tattoo is destroyed or removed by limb loss, the tether will be broken, but its master may be displeased and appear or pursue for retribution."@en ,
                               "The tether is a deal struck over future service. Thus, the master requires assurances that this debt will not be welched or avoided. The tether tattoo enforces this agreement."@en ;
                  rdfs:label "Tattooing by tether"@en ;
                  gen:after :word_is_bond ;
                  gen:setAdditive :tattoos .


###  https://raw.githubusercontent.com/AbsVahter/ontoTRPG/main/crown_and_skull/crown_and_skull.ttl#tattoos
:tattoos rdf:type owl:NamedIndividual ,
                  gen:ParameterPC ;
         rdfs:comment "format = [list of {tattoo: linked magic advancement}]"@en ;
         rdfs:label "Tattoos"@en .


###  https://raw.githubusercontent.com/AbsVahter/ontoTRPG/main/crown_and_skull/crown_and_skull.ttl#template_adventurer
:template_adventurer rdf:type owl:NamedIndividual ,
                              gen:TemplatePC ;
                     rdfs:comment "You are a nomad, a hunter, a road-walker. You thrive in the ruins and wilderness, seeking treasures and truths."@en ;
                     rdfs:label "Adventurer"@en .


###  https://raw.githubusercontent.com/AbsVahter/ontoTRPG/main/crown_and_skull/crown_and_skull.ttl#template_cleric
:template_cleric rdf:type owl:NamedIndividual ,
                          gen:TemplatePC ;
                 rdfs:comment "Yours is the holy path. You represent a higher power, divine will, and the greater good that watches over living things."@en ;
                 rdfs:label "Cleric"@en .


###  https://raw.githubusercontent.com/AbsVahter/ontoTRPG/main/crown_and_skull/crown_and_skull.ttl#template_hoodlum
:template_hoodlum rdf:type owl:NamedIndividual ,
                           gen:TemplatePC ;
                  rdfs:comment "You are a dubious character... a shadow-dweller. You dabble in the forbidden, the lawless, and the truly free. Your fate is yours alone."@en ;
                  rdfs:label "Hoodlum"@en .


###  https://raw.githubusercontent.com/AbsVahter/ontoTRPG/main/crown_and_skull/crown_and_skull.ttl#template_sage
:template_sage rdf:type owl:NamedIndividual ,
                        gen:TemplatePC ;
               rdfs:comment "You are a learned researcher; keeper of books; mind of science, history, and the arcane. The writing desk is your home, but adventure calls."@en ;
               rdfs:label "Sage"@en .


###  https://raw.githubusercontent.com/AbsVahter/ontoTRPG/main/crown_and_skull/crown_and_skull.ttl#template_smith
:template_smith rdf:type owl:NamedIndividual ,
                         gen:TemplatePC ;
                rdfs:comment "You are a hearty worker of materials and tools. The daily grind of making wares must wait, though, as the wide world beckons."@en ;
                rdfs:label "Smith"@en .


###  https://raw.githubusercontent.com/AbsVahter/ontoTRPG/main/crown_and_skull/crown_and_skull.ttl#template_soldier
:template_soldier rdf:type owl:NamedIndividual ,
                           gen:TemplatePC ;
                  rdfs:comment "You specialize in weapons and armor. On adventures and quests, your allies look to you to take a beating and see foes dispatched."@en ;
                  rdfs:label "Soldier"@en .


###  https://raw.githubusercontent.com/AbsVahter/ontoTRPG/main/crown_and_skull/crown_and_skull.ttl#tether_service
:tether_service rdf:type owl:NamedIndividual ;
                rdfs:label "Called service by tether"@en ;
                gen:after :tattooing_tether ;
                gen:duration "1d4 rounds" ;
                gen:effect :status_tether_service_is_not_given ,
                           :tether_service_is_rendered ;
                gen:prerequisiteDescription "the servant must begin to comply service" .


###  https://raw.githubusercontent.com/AbsVahter/ontoTRPG/main/crown_and_skull/crown_and_skull.ttl#tether_service_is_rendered
:tether_service_is_rendered rdf:type owl:NamedIndividual ;
                            rdfs:label "Called service by tether is rendered"@en ;
                            gen:prerequisiteDescription "service is rendered" ;
                            gen:setAdditive :tattoos ;
                            gen:valueFormula "linked tattoo disappers" .


###  https://raw.githubusercontent.com/AbsVahter/ontoTRPG/main/crown_and_skull/crown_and_skull.ttl#thenneport_docks
:thenneport_docks rdf:type owl:NamedIndividual ,
                           gen:Location ;
                  rdfs:comment "The complex of piers, moorings and cranes in Rivergate is a wonder of The North Holds. All manner of barges, fishing boats and rivercraft gather here to load and unload cargo, conscript crew, and arrange expeditions to every corner of the world. So much wealth moves through these ports, there is an abundance of ‘red cloak’ guards present at all times. These city soldiers sport 10-foot spears, and they are some of the finest fighters in The Holds."@en ;
                  rdfs:label "Thenneport Docks"@en .


###  https://raw.githubusercontent.com/AbsVahter/ontoTRPG/main/crown_and_skull/crown_and_skull.ttl#threshold_defense
:threshold_defense rdf:type owl:NamedIndividual ;
                   rdfs:label "Threshold for defense roll"@en ;
                   gen:input :defense_penalty ,
                             :stat_def_pc ;
                   gen:valueFormula "defense - (penalty to defense)" .


###  https://raw.githubusercontent.com/AbsVahter/ontoTRPG/main/crown_and_skull/crown_and_skull.ttl#threshold_flat
:threshold_flat rdf:type owl:NamedIndividual ;
                rdfs:label "Threshold for flat roll"@en ;
                gen:valueFormula "target or opposed roll" .


###  https://raw.githubusercontent.com/AbsVahter/ontoTRPG/main/crown_and_skull/crown_and_skull.ttl#threshold_skill
:threshold_skill rdf:type owl:NamedIndividual ;
                 rdfs:label "Threshold for skill roll"@en ;
                 gen:input :Skill ,
                           :skill_roll_penalty ;
                 gen:valueFormula "skill value - (skill roll penalty)" .


###  https://raw.githubusercontent.com/AbsVahter/ontoTRPG/main/crown_and_skull/crown_and_skull.ttl#threshold_wild_magic
:threshold_wild_magic rdf:type owl:NamedIndividual ;
                      rdfs:label "Wild magic threshold"@en ;
                      gen:input :skill_magic ,
                                :spell_custom ;
                      gen:valueFormula "(magic skill) - (spell value in hero points)" .


###  https://raw.githubusercontent.com/AbsVahter/ontoTRPG/main/crown_and_skull/crown_and_skull.ttl#tier
:tier rdf:type owl:NamedIndividual .


###  https://raw.githubusercontent.com/AbsVahter/ontoTRPG/main/crown_and_skull/crown_and_skull.ttl#transitions_and_table_talk
:transitions_and_table_talk rdf:type owl:NamedIndividual ;
                            rdfs:label "Transitions and Table Talk"@en ;
                            gen:after :recovery ;
                            gen:effectOption :setting_scene .


###  https://raw.githubusercontent.com/AbsVahter/ontoTRPG/main/crown_and_skull/crown_and_skull.ttl#upgrade_skill
:upgrade_skill rdf:type owl:NamedIndividual ;
               rdfs:label "Upgrade skill"@en ;
               gen:Actor gen:player ;
               gen:cost "1 point per 1 skill level" ;
               gen:inputOption :Skill ;
               gen:resource :hero_points ;
               gen:setAdditive :skills .


###  https://raw.githubusercontent.com/AbsVahter/ontoTRPG/main/crown_and_skull/crown_and_skull.ttl#wild_magic
:wild_magic rdf:type owl:NamedIndividual ,
                     gen:Check ;
            rdfs:label "Conjuring a Wild Spell"@en ;
            gen:Actor gen:player ;
            gen:basedOn :check_skill ;
            gen:checkFailure :losing_control ;
            gen:checkSuccess :set_spell ;
            gen:checkThreshold :threshold_wild_magic ;
            gen:duration "1 turn" ;
            gen:input :spell_custom ;
            gen:prerequisite :skill_magic ;
            gen:prerequisiteDescription "magic skill > spell value in hero points" .


###  https://raw.githubusercontent.com/AbsVahter/ontoTRPG/main/crown_and_skull/crown_and_skull.ttl#wizard_ancient_one
:wizard_ancient_one rdf:type owl:NamedIndividual ,
                             :Wizard ;
                    rdfs:comment "The deepest secrets of magic take centuries to unlock. By magical means, you have prolonged your life long enough to reach the most obscure levels of spell-craft."@en ;
                    rdfs:label "Ancient one"@en .


###  https://raw.githubusercontent.com/AbsVahter/ontoTRPG/main/crown_and_skull/crown_and_skull.ttl#wizard_demonologist
:wizard_demonologist rdf:type owl:NamedIndividual ,
                              :Wizard ;
                     rdfs:comment "You see power in the infernal, certain that the darkness can be made a servant. This darkness you perilously tap for your power, always an inch from the wrath of inhuman evils."@en ;
                     rdfs:label "Demonologist"@en .


###  https://raw.githubusercontent.com/AbsVahter/ontoTRPG/main/crown_and_skull/crown_and_skull.ttl#wizard_starfallen
:wizard_starfallen rdf:type owl:NamedIndividual ,
                            :Wizard ;
                   rdfs:comment "Some wizards are not born... they fall from the stars. These beings are envoys of hidden gods, incarnations of world-guardians, or a living coalescence of nature’s arcane spirit."@en ;
                   rdfs:label "Starfallen"@en .


###  https://raw.githubusercontent.com/AbsVahter/ontoTRPG/main/crown_and_skull/crown_and_skull.ttl#word_is_bond
:word_is_bond rdf:type owl:NamedIndividual ;
              rdfs:comment "A tether is an oath to a magic being. In return for power promised, the wizard MUST answer a future call for service. As such, tethers can only be made with intelligent creatures that can speak. Usually, such an offer benefi ts the master more than the servant."@en ;
              rdfs:label "Word is bond"@en ;
              gen:effectOption :path_of_magic_wizard_during_action ,
                               :path_of_magic_wizard_overspend .


###  https://raw.githubusercontent.com/AbsVahter/ontoTRPG/main/ontoGeneral.ttl#Check
gen:Check rdf:type owl:NamedIndividual .


###  https://raw.githubusercontent.com/AbsVahter/ontoTRPG/main/ontoGeneral.ttl#TemplatePC
gen:TemplatePC rdf:type owl:NamedIndividual .


###  https://raw.githubusercontent.com/AbsVahter/ontoTRPG/main/ontoGeneral.ttl#effect
gen:effect rdf:type owl:NamedIndividual .


###  https://raw.githubusercontent.com/AbsVahter/ontoTRPG/main/ontoGeneral.ttl#prerequisiteDescription
gen:prerequisiteDescription rdf:type owl:NamedIndividual .


###  https://raw.githubusercontent.com/AbsVahter/ontoTRPG/main/ontoGeneral.ttl#target
gen:target rdf:type owl:NamedIndividual .


###  https://raw.githubusercontent.com/AbsVahter/ontoTRPG/main/ontoGeneral.ttl#valueFormula
gen:valueFormula rdf:type owl:NamedIndividual .


#################################################################
#    Annotations
#################################################################

:Ability rdfs:label "Ability"@en .


:Attrition rdfs:comment "Attrition is a term for the reduction of your character’s resources when hit by hazards and attacks."@en ;
           rdfs:label "Attrition"@en .


:Companion rdfs:label "Companion"@en .


:CoreAbility rdfs:label "Core ability"@en .


:EffectCompanion rdfs:label "Companion effect"@en .


:EffectItem rdfs:label "Gear effect"@en .


:EffectSpell rdfs:label "Spell effect"@en .


:FlawBasic rdfs:label "Basic flaw"@en .


:Item rdfs:comment "effect after or during use"@en ,
                   "format = (base, list of effects and limitations, cost)"@en ;
      rdfs:label "Item"@en .


:ItemArmor rdfs:label "Armor"@en .


:ItemBasic rdfs:label "Basic item"@en .


:ItemCrown rdfs:label "Crown item"@en .


:ItemSkull rdfs:label "Skull item"@en .


:ItemWeapon rdfs:label "Weapon"@en .


:LimitationCompanion rdfs:label "Companion limitation"@en .


:LimitationItem rdfs:label "Gear limitation"@en .


:LimitationSpell rdfs:label "Spell limitation"@en .


:Lineage rdfs:comment "Lineage does not include mechanical aspects, as each population is vast and diverse."@en ;
         rdfs:label "Lineage"@en .


:MagicAdvancement rdfs:label "Magic advancement"@en .


:MagicAdvancementHolySymbol rdfs:label "Magic advancement for holy symbol"@en .


:SetAdditiveEquipment rdfs:label "Current equipment's correction"@en .


:SetAdditiveSkill rdfs:label "Current skill list's correction"@en .


:Skill rdfs:label "Skill"@en .


:SkillAntimagic rdfs:label "Antimagic skill"@en .


:SkillBasic rdfs:label "Basic skill"@en .


:SkillCompanion rdfs:label "Companion skill"@en .


:SkillCrown rdfs:label "Crown skill"@en .


:SkillSkull rdfs:label "Skull skill"@en .


:Spell rdfs:comment "By default: somatics, 1d6 phases duration, 1d6 effect, touch range, single target."@en ;
       rdfs:label "Spell"@en .


:SpellConsequenceInfernal rdfs:label "Infernal magic consequence"@en .


:SpellConsequenceUnstable rdfs:label "Unstable magic consequence"@en .


:Wizard rdfs:label "Wizard"@en .


:tier rdfs:label "Tier"@en .


gen:TemplatePC rdfs:label "PC template"@en .


gen:game_play gen:included :crown_or_skull ,
                           :encounter ,
                           :giving_hero_coin ,
                           :path_of_magic ,
                           :renown ,
                           :rest ,
                           :set_flaw ,
                           :set_hero_coin ,
                           :set_hero_points ,
                           gen:Check .


gen:game_preparation gen:included :character_creation ,
                                  :set_hometown .


###  Generated by the OWL API (version 4.5.29.2024-05-13T12:11:03Z) https://github.com/owlcs/owlapi
