<?xml version="1.0"?>
<rdf:RDF xmlns="http://www.semanticweb.org/nerpa/ontologies/2023/6/untitled-ontology-101/"
     xml:base="http://www.semanticweb.org/nerpa/ontologies/2023/6/untitled-ontology-101/"
     xmlns:owl="http://www.w3.org/2002/07/owl#"
     xmlns:rdf="http://www.w3.org/1999/02/22-rdf-syntax-ns#"
     xmlns:xml="http://www.w3.org/XML/1998/namespace"
     xmlns:xsd="http://www.w3.org/2001/XMLSchema#"
     xmlns:rdfs="http://www.w3.org/2000/01/rdf-schema#"
     xmlns:schema="http://schema.org/"
     xmlns:pzo2101="https://raw.githubusercontent.com/AbsVahter/trpgontologies/main/pathfinder/2ed/pzo2101.rdf#"
     xmlns:pzo90145="https://raw.githubusercontent.com/AbsVahter/trpgontologies/main/pathfinder/2ed/pzo90145.rdf#"
     xmlns:pf2_general="https://raw.githubusercontent.com/AbsVahter/trpgontologies/main/pathfinder/2ed/pf2_general.rdf#"
     xmlns:pzo9000-25e="https://raw.githubusercontent.com/AbsVahter/trpgontologies/main/pathfinder/2ed/pzo9000-25e.rdf#">
    <owl:Ontology rdf:about="https://raw.githubusercontent.com/AbsVahter/trpgontologies/main/pathfinder/2ed/pzo90145.rdf">
        <owl:imports rdf:resource="https://raw.githubusercontent.com/AbsVahter/trpgontologies/main/pathfinder/2ed/pzo9000-25e.rdf"/>
    </owl:Ontology>
    


    <!-- 
    ///////////////////////////////////////////////////////////////////////////////////////
    //
    // Annotation properties
    //
    ///////////////////////////////////////////////////////////////////////////////////////
     -->

    


    <!-- https://raw.githubusercontent.com/AbsVahter/trpgontologies/main/pathfinder/2ed/pf2_general.rdf#art_depicts -->

    <owl:AnnotationProperty rdf:about="https://raw.githubusercontent.com/AbsVahter/trpgontologies/main/pathfinder/2ed/pf2_general.rdf#art_depicts"/>
    


    <!-- 
    ///////////////////////////////////////////////////////////////////////////////////////
    //
    // Object Properties
    //
    ///////////////////////////////////////////////////////////////////////////////////////
     -->

    


    <!-- https://raw.githubusercontent.com/AbsVahter/trpgontologies/main/pathfinder/2ed/pzo90145.rdf#event_after_event -->

    <owl:ObjectProperty rdf:about="https://raw.githubusercontent.com/AbsVahter/trpgontologies/main/pathfinder/2ed/pzo90145.rdf#event_after_event">
        <owl:inverseOf rdf:resource="https://raw.githubusercontent.com/AbsVahter/trpgontologies/main/pathfinder/2ed/pzo90145.rdf#event_to_event"/>
    </owl:ObjectProperty>
    


    <!-- https://raw.githubusercontent.com/AbsVahter/trpgontologies/main/pathfinder/2ed/pzo90145.rdf#event_to_event -->

    <owl:ObjectProperty rdf:about="https://raw.githubusercontent.com/AbsVahter/trpgontologies/main/pathfinder/2ed/pzo90145.rdf#event_to_event">
        <rdfs:domain rdf:resource="https://raw.githubusercontent.com/AbsVahter/trpgontologies/main/pathfinder/2ed/pzo9000-25e.rdf#Event"/>
        <rdfs:range rdf:resource="https://raw.githubusercontent.com/AbsVahter/trpgontologies/main/pathfinder/2ed/pzo9000-25e.rdf#Event"/>
    </owl:ObjectProperty>
    


    <!-- https://raw.githubusercontent.com/AbsVahter/trpgontologies/main/pathfinder/2ed/pzo90145.rdf#event_with_resource -->

    <owl:ObjectProperty rdf:about="https://raw.githubusercontent.com/AbsVahter/trpgontologies/main/pathfinder/2ed/pzo90145.rdf#event_with_resource">
        <owl:inverseOf rdf:resource="https://raw.githubusercontent.com/AbsVahter/trpgontologies/main/pathfinder/2ed/pzo90145.rdf#resource_for_event"/>
        <rdfs:domain rdf:resource="https://raw.githubusercontent.com/AbsVahter/trpgontologies/main/pathfinder/2ed/pzo9000-25e.rdf#Event"/>
        <rdfs:range rdf:resource="https://raw.githubusercontent.com/AbsVahter/trpgontologies/main/pathfinder/2ed/pzo2101.rdf#Resource"/>
    </owl:ObjectProperty>
    


    <!-- https://raw.githubusercontent.com/AbsVahter/trpgontologies/main/pathfinder/2ed/pzo90145.rdf#motive_has_target_resource -->

    <owl:ObjectProperty rdf:about="https://raw.githubusercontent.com/AbsVahter/trpgontologies/main/pathfinder/2ed/pzo90145.rdf#motive_has_target_resource">
        <owl:inverseOf rdf:resource="https://raw.githubusercontent.com/AbsVahter/trpgontologies/main/pathfinder/2ed/pzo90145.rdf#resource_is_target_for_motive"/>
        <rdfs:domain rdf:resource="https://raw.githubusercontent.com/AbsVahter/trpgontologies/main/pathfinder/2ed/pzo9000-25e.rdf#Motive"/>
        <rdfs:range rdf:resource="https://raw.githubusercontent.com/AbsVahter/trpgontologies/main/pathfinder/2ed/pzo2101.rdf#Resource"/>
    </owl:ObjectProperty>
    


    <!-- https://raw.githubusercontent.com/AbsVahter/trpgontologies/main/pathfinder/2ed/pzo90145.rdf#resource_for_event -->

    <owl:ObjectProperty rdf:about="https://raw.githubusercontent.com/AbsVahter/trpgontologies/main/pathfinder/2ed/pzo90145.rdf#resource_for_event"/>
    


    <!-- https://raw.githubusercontent.com/AbsVahter/trpgontologies/main/pathfinder/2ed/pzo90145.rdf#resource_is_target_for_motive -->

    <owl:ObjectProperty rdf:about="https://raw.githubusercontent.com/AbsVahter/trpgontologies/main/pathfinder/2ed/pzo90145.rdf#resource_is_target_for_motive"/>
    


    <!-- 
    ///////////////////////////////////////////////////////////////////////////////////////
    //
    // Data properties
    //
    ///////////////////////////////////////////////////////////////////////////////////////
     -->

    


    <!-- https://raw.githubusercontent.com/AbsVahter/trpgontologies/main/pathfinder/2ed/pzo90145.rdf#event_date -->

    <owl:DatatypeProperty rdf:about="https://raw.githubusercontent.com/AbsVahter/trpgontologies/main/pathfinder/2ed/pzo90145.rdf#event_date">
        <rdfs:domain rdf:resource="https://raw.githubusercontent.com/AbsVahter/trpgontologies/main/pathfinder/2ed/pzo9000-25e.rdf#Event"/>
    </owl:DatatypeProperty>
    


    <!-- 
    ///////////////////////////////////////////////////////////////////////////////////////
    //
    // Classes
    //
    ///////////////////////////////////////////////////////////////////////////////////////
     -->

    


    <!-- https://raw.githubusercontent.com/AbsVahter/trpgontologies/main/pathfinder/2ed/pzo2101.rdf#Resource -->

    <owl:Class rdf:about="https://raw.githubusercontent.com/AbsVahter/trpgontologies/main/pathfinder/2ed/pzo2101.rdf#Resource"/>
    


    <!-- https://raw.githubusercontent.com/AbsVahter/trpgontologies/main/pathfinder/2ed/pzo2101.rdf#Resource_Artifact -->

    <owl:Class rdf:about="https://raw.githubusercontent.com/AbsVahter/trpgontologies/main/pathfinder/2ed/pzo2101.rdf#Resource_Artifact">
        <rdfs:subClassOf rdf:resource="https://raw.githubusercontent.com/AbsVahter/trpgontologies/main/pathfinder/2ed/pzo2101.rdf#Resource"/>
    </owl:Class>
    


    <!-- https://raw.githubusercontent.com/AbsVahter/trpgontologies/main/pathfinder/2ed/pzo90145.rdf#Event_Chapter_2_The_Ruined_Citadel -->

    <owl:Class rdf:about="https://raw.githubusercontent.com/AbsVahter/trpgontologies/main/pathfinder/2ed/pzo90145.rdf#Event_Chapter_2_The_Ruined_Citadel">
        <rdfs:subClassOf rdf:resource="https://raw.githubusercontent.com/AbsVahter/trpgontologies/main/pathfinder/2ed/pzo9000-25e.rdf#Event"/>
        <rdfs:comment>The heroes travel to Hellknight Hill and explore the ruined citadel that sits atop it. Therein, they might meet a few new friends, and they’ll certainly clash with plenty of new enemies before they can rescue a tribe of imperiled goblins.</rdfs:comment>
    </owl:Class>
    


    <!-- https://raw.githubusercontent.com/AbsVahter/trpgontologies/main/pathfinder/2ed/pzo90145.rdf#Event_Chapter_3_The_Citadel_Below -->

    <owl:Class rdf:about="https://raw.githubusercontent.com/AbsVahter/trpgontologies/main/pathfinder/2ed/pzo90145.rdf#Event_Chapter_3_The_Citadel_Below">
        <rdfs:subClassOf rdf:resource="https://raw.githubusercontent.com/AbsVahter/trpgontologies/main/pathfinder/2ed/pzo9000-25e.rdf#Event"/>
        <rdfs:comment>The heroes descend beneath Citadel Altaerein, where they find something sinister: an isolated group of cultists called the Cinderclaws, who herald a more serious threat from their brethren below.</rdfs:comment>
    </owl:Class>
    


    <!-- https://raw.githubusercontent.com/AbsVahter/trpgontologies/main/pathfinder/2ed/pzo90145.rdf#Event_History -->

    <owl:Class rdf:about="https://raw.githubusercontent.com/AbsVahter/trpgontologies/main/pathfinder/2ed/pzo90145.rdf#Event_History">
        <rdfs:subClassOf rdf:resource="https://raw.githubusercontent.com/AbsVahter/trpgontologies/main/pathfinder/2ed/pzo9000-25e.rdf#Event"/>
    </owl:Class>
    


    <!-- https://raw.githubusercontent.com/AbsVahter/trpgontologies/main/pathfinder/2ed/pzo90145.rdf#Event_Chapter_1_The_Council~s_Chosen -->

    <owl:Class rdf:about="https://raw.githubusercontent.com/AbsVahter/trpgontologies/main/pathfinder/2ed/pzo90145.rdf#Event_Chapter_1_The_Council~s_Chosen">
        <rdfs:subClassOf rdf:resource="https://raw.githubusercontent.com/AbsVahter/trpgontologies/main/pathfinder/2ed/pzo9000-25e.rdf#Event"/>
        <rdfs:comment>The Age of Ashes Adventure Path begins with a routine town council meeting in the storied town of Breachill. But before the PCs can learn what sort of adventure the town council might hire them for, the building ignites in a fiery crisis!</rdfs:comment>
    </owl:Class>
    


    <!-- https://raw.githubusercontent.com/AbsVahter/trpgontologies/main/pathfinder/2ed/pzo90145.rdf#Event_Chapter_4_Breachill’s_Secrets -->

    <owl:Class rdf:about="https://raw.githubusercontent.com/AbsVahter/trpgontologies/main/pathfinder/2ed/pzo90145.rdf#Event_Chapter_4_Breachill’s_Secrets">
        <rdfs:subClassOf rdf:resource="https://raw.githubusercontent.com/AbsVahter/trpgontologies/main/pathfinder/2ed/pzo9000-25e.rdf#Event"/>
        <rdfs:comment>After following a secret tunnel leading from the Hellknight citadel to the town where their saga began, the heroes must scramble to find out who in the town plots to use the keep for nefarious purposes. Clues lead the heroes to a cave complex that leads straight to the lowest level of the Hellknight citadel’s dungeons. There, they must face a powerful cultist leader and discover an ancient elven gateway before untold horrors descend upon Breachill—and perhaps all of Golarion!</rdfs:comment>
    </owl:Class>
    


    <!-- 
    ///////////////////////////////////////////////////////////////////////////////////////
    //
    // Individuals
    //
    ///////////////////////////////////////////////////////////////////////////////////////
     -->

    


    <!-- https://raw.githubusercontent.com/AbsVahter/trpgontologies/main/pathfinder/2ed/pzo2101.rdf#Gamerule_Leveling_Up -->

    <owl:NamedIndividual rdf:about="https://raw.githubusercontent.com/AbsVahter/trpgontologies/main/pathfinder/2ed/pzo2101.rdf#Gamerule_Leveling_Up"/>
    


    <!-- https://raw.githubusercontent.com/AbsVahter/trpgontologies/main/pathfinder/2ed/pzo9000-25e.rdf#NPC_Lamond_Breachton -->

    <rdf:Description rdf:about="https://raw.githubusercontent.com/AbsVahter/trpgontologies/main/pathfinder/2ed/pzo9000-25e.rdf#NPC_Lamond_Breachton">
        <owl:sameAs rdf:resource="https://raw.githubusercontent.com/AbsVahter/trpgontologies/main/pathfinder/2ed/pzo90145.rdf#NPC_Mengkare"/>
    </rdf:Description>
    


    <!-- https://raw.githubusercontent.com/AbsVahter/trpgontologies/main/pathfinder/2ed/pzo90145.rdf#NPC_Mengkare -->

    <rdf:Description rdf:about="https://raw.githubusercontent.com/AbsVahter/trpgontologies/main/pathfinder/2ed/pzo90145.rdf#NPC_Mengkare"/>
    


    <!-- https://raw.githubusercontent.com/AbsVahter/trpgontologies/main/pathfinder/2ed/pzo90145.rdf#Advice_Advancement_Track -->

    <owl:NamedIndividual rdf:about="https://raw.githubusercontent.com/AbsVahter/trpgontologies/main/pathfinder/2ed/pzo90145.rdf#Advice_Advancement_Track">
        <rdf:type rdf:resource="https://raw.githubusercontent.com/AbsVahter/trpgontologies/main/pathfinder/2ed/pzo2101.rdf#Gamerule_Advice"/>
        <pzo2101:advice_for_gamerule rdf:resource="https://raw.githubusercontent.com/AbsVahter/trpgontologies/main/pathfinder/2ed/pzo2101.rdf#Gamerule_Leveling_Up"/>
        <rdfs:comment>The PCs begin this adventure at 1st level.
The PCs should be 2nd level before they descend into Citadel Altaerein’s dungeon in Chapter 3.
The PCs should reach 3rd level after clearing two wings of the dungeon in Chapter 3.
The PCs should be 4th level before they enter the cavern complex around Alseta’s Ring.</rdfs:comment>
    </owl:NamedIndividual>
    


    <!-- https://raw.githubusercontent.com/AbsVahter/trpgontologies/main/pathfinder/2ed/pzo90145.rdf#Art_Citadel -->

    <owl:NamedIndividual rdf:about="https://raw.githubusercontent.com/AbsVahter/trpgontologies/main/pathfinder/2ed/pzo90145.rdf#Art_Citadel">
        <rdf:type rdf:resource="https://raw.githubusercontent.com/AbsVahter/trpgontologies/main/pathfinder/2ed/pf2_general.rdf#Art"/>
        <schema:image rdf:resource="https://www.worldanvil.com/uploads/images/8973a08d027526f05110bd89e565cae2.jpg"/>
    </owl:NamedIndividual>
    


    <!-- https://raw.githubusercontent.com/AbsVahter/trpgontologies/main/pathfinder/2ed/pzo90145.rdf#Art_Fire_in_Breachill -->

    <owl:NamedIndividual rdf:about="https://raw.githubusercontent.com/AbsVahter/trpgontologies/main/pathfinder/2ed/pzo90145.rdf#Art_Fire_in_Breachill">
        <rdf:type rdf:resource="https://raw.githubusercontent.com/AbsVahter/trpgontologies/main/pathfinder/2ed/pf2_general.rdf#Art"/>
        <schema:image rdf:resource="https://guildberkeley.files.wordpress.com/2019/10/hellknight-hill.jpg"/>
    </owl:NamedIndividual>
    


    <!-- https://raw.githubusercontent.com/AbsVahter/trpgontologies/main/pathfinder/2ed/pzo90145.rdf#Art_Goblin_Eater -->

    <owl:NamedIndividual rdf:about="https://raw.githubusercontent.com/AbsVahter/trpgontologies/main/pathfinder/2ed/pzo90145.rdf#Art_Goblin_Eater">
        <rdf:type rdf:resource="https://raw.githubusercontent.com/AbsVahter/trpgontologies/main/pathfinder/2ed/pf2_general.rdf#Art"/>
        <schema:image rdf:resource="https://ibb.co/gdKjyRm"/>
    </owl:NamedIndividual>
    


    <!-- https://raw.githubusercontent.com/AbsVahter/trpgontologies/main/pathfinder/2ed/pzo90145.rdf#Art_Scarlet_Triad_Logo -->

    <owl:NamedIndividual rdf:about="https://raw.githubusercontent.com/AbsVahter/trpgontologies/main/pathfinder/2ed/pzo90145.rdf#Art_Scarlet_Triad_Logo">
        <rdf:type rdf:resource="https://raw.githubusercontent.com/AbsVahter/trpgontologies/main/pathfinder/2ed/pf2_general.rdf#Art"/>
        <schema:image rdf:resource="https://ibb.co/vPx5w0R"/>
        <pf2_general:art_depicts rdf:resource="https://raw.githubusercontent.com/AbsVahter/trpgontologies/main/pathfinder/2ed/pzo90145.rdf#Community_Scarlet_Triad"/>
    </owl:NamedIndividual>
    


    <!-- https://raw.githubusercontent.com/AbsVahter/trpgontologies/main/pathfinder/2ed/pzo90145.rdf#Artifact_Orb_of_Gold_Dragonkind -->

    <owl:NamedIndividual rdf:about="https://raw.githubusercontent.com/AbsVahter/trpgontologies/main/pathfinder/2ed/pzo90145.rdf#Artifact_Orb_of_Gold_Dragonkind">
        <rdf:type rdf:resource="https://raw.githubusercontent.com/AbsVahter/trpgontologies/main/pathfinder/2ed/pzo2101.rdf#Resource_Artifact"/>
        <pzo90145:resource_for_event rdf:resource="https://raw.githubusercontent.com/AbsVahter/trpgontologies/main/pathfinder/2ed/pzo90145.rdf#Event_Dragon_Plague"/>
        <rdfs:comment>powerful artifact to dominate metallic dragons throughout Taldor, driving them to commit devastating atrocities that threw the nation into chaos</rdfs:comment>
    </owl:NamedIndividual>
    


    <!-- https://raw.githubusercontent.com/AbsVahter/trpgontologies/main/pathfinder/2ed/pzo90145.rdf#Community_Ekujae_Elves -->

    <owl:NamedIndividual rdf:about="https://raw.githubusercontent.com/AbsVahter/trpgontologies/main/pathfinder/2ed/pzo90145.rdf#Community_Ekujae_Elves">
        <rdf:type rdf:resource="https://raw.githubusercontent.com/AbsVahter/trpgontologies/main/pathfinder/2ed/pzo9000-25e.rdf#Community"/>
        <pzo9000-25e:subject_has_motive rdf:resource="https://raw.githubusercontent.com/AbsVahter/trpgontologies/main/pathfinder/2ed/pzo90145.rdf#Motive_Stop_Age_of_Ashes"/>
    </owl:NamedIndividual>
    


    <!-- https://raw.githubusercontent.com/AbsVahter/trpgontologies/main/pathfinder/2ed/pzo90145.rdf#Community_Scarlet_Triad -->

    <owl:NamedIndividual rdf:about="https://raw.githubusercontent.com/AbsVahter/trpgontologies/main/pathfinder/2ed/pzo90145.rdf#Community_Scarlet_Triad">
        <rdf:type rdf:resource="https://raw.githubusercontent.com/AbsVahter/trpgontologies/main/pathfinder/2ed/pzo9000-25e.rdf#Community"/>
        <pzo9000-25e:subject_of_event rdf:resource="https://raw.githubusercontent.com/AbsVahter/trpgontologies/main/pathfinder/2ed/pzo90145.rdf#Event_Second_Glorious_Endeavor"/>
        <rdfs:comment>The storms that wracked the world after Aroden’s death devastated Promise and forced setbacks to the Glorious Endeavor. Over the months that followed, Mengkare realized he needed to focus his attentions on protecting and guiding the Glorious Endeavor on Hermea, and thus he couldn’t spare the time to personally seek out talented and gifted humans on the mainland to recruit to the project. As a solution, he founded a group called the Scarlet Triad in 4607, drawing upon three allied mercantile concerns with ties to (and based in) the city of Katapesh. The triad’s leaders arranged for the use of chambers below the city’s so-called Red Pyramid and took on the role of curators and guides of the historic site as a front for their operations. Only the city’s leaders had an inkling of the Scarlet Triad’s true purpose, and Mengkare paid well to ensure they were satisfied enough to not probe too deeply or ask too many questions.</rdfs:comment>
    </owl:NamedIndividual>
    


    <!-- https://raw.githubusercontent.com/AbsVahter/trpgontologies/main/pathfinder/2ed/pzo90145.rdf#Event_Age_of_Ashes -->

    <owl:NamedIndividual rdf:about="https://raw.githubusercontent.com/AbsVahter/trpgontologies/main/pathfinder/2ed/pzo90145.rdf#Event_Age_of_Ashes">
        <rdf:type rdf:resource="https://raw.githubusercontent.com/AbsVahter/trpgontologies/main/pathfinder/2ed/pzo90145.rdf#Event_History"/>
        <pzo9000-25e:event_in_location rdf:resource="https://raw.githubusercontent.com/AbsVahter/trpgontologies/main/pathfinder/2ed/pzo90145.rdf#Location_Alseta~s_Ring"/>
        <pzo90145:event_to_event rdf:resource="https://raw.githubusercontent.com/AbsVahter/trpgontologies/main/pathfinder/2ed/pzo90145.rdf#Event_End_of_Age_of_Ashes_by_Ekujae_Elves"/>
        <pzo90145:event_date>{
–5293: Earthfall;
–5280: Dahak sneaks into the Material Plane via a flaw in Huntergate to revel in the post-Earthfall ruins, focusing his wrath in and around the Mwangi Expanse;
}</pzo90145:event_date>
        <rdfs:comment>Many ages have come and gone during Golarion’s long history, starting eons ago with the Age of Creation. The Age of Ashes occupies its own category, for it is an age yet to come and simultaneously an age that lasted but a heartbeat. The Ekujae elves maintain some records of the first Age of Ashes, a span of time that lasted a few short years when an incarnation of Dahak, the draconic god of destruction, ravaged a post-apocalyptic Golarion not long after Earthfall. But now, if heroes can’t stand in its way, a new Age of Ashes is set to begin!
When Earthfall struck Golarion and nearly brought about the world’s end, Dahak, the destructive god of evil dragons, took note. Amid the overwhelming devastation on both physical and spiritual levels (with continents and gods alike being destroyed), Dahak saw his chance to creep into the world without arousing the wrath of his father, Apsu. Dahak explored the metaphysical boundaries separating his realm in Hell and the world of Golarion and, after several years of searching, discovered a flaw in one of the first-constructed portals of Alseta’s Ring. Using this flaw, Dahak was able to ease a sliver of his essence through the boundaries of reality to manifest a powerful incarnation of himself in the postapocalyptic world.
By taking care to invest his manifestation with just enough power so as to avoid Apsu’s attention, Dahak’s incarnation was able to ravage the world for years, allowing the god of destruction to live and destroy vicariously through his incarnation’s actions. The results of the incarnation’s destructive power came to be known as “dragonstorms”—long-lasting events akin to thunderstorms that incorporated the five chromatic dragon breath weapons: lightning strikes, fiery tornados, freezing blasts of cold, acidic rain, and clouds of poisonous fog. Furthermore, these dragonstorms drove all dragons within them mad, reverting them to a primal frenzy as they sought each other out, adding further devastation as they violently clashed with one another.</rdfs:comment>
    </owl:NamedIndividual>
    


    <!-- https://raw.githubusercontent.com/AbsVahter/trpgontologies/main/pathfinder/2ed/pzo90145.rdf#Event_Destruction_of_Orb_of_Gold_Dragonkind -->

    <owl:NamedIndividual rdf:about="https://raw.githubusercontent.com/AbsVahter/trpgontologies/main/pathfinder/2ed/pzo90145.rdf#Event_Destruction_of_Orb_of_Gold_Dragonkind">
        <rdf:type rdf:resource="https://raw.githubusercontent.com/AbsVahter/trpgontologies/main/pathfinder/2ed/pzo90145.rdf#Event_History"/>
        <pzo9000-25e:event_with_subject rdf:resource="https://raw.githubusercontent.com/AbsVahter/trpgontologies/main/pathfinder/2ed/pzo90145.rdf#NPC_Mengkare"/>
        <pzo90145:event_after_event rdf:resource="https://raw.githubusercontent.com/AbsVahter/trpgontologies/main/pathfinder/2ed/pzo90145.rdf#Event_Mengkare~s_Path"/>
        <pzo90145:event_with_resource rdf:resource="https://raw.githubusercontent.com/AbsVahter/trpgontologies/main/pathfinder/2ed/pzo90145.rdf#Artifact_Orb_of_Gold_Dragonkind"/>
        <rdfs:comment>In 3980, Mengkare learned of a deeply troubling rumor that finally drew him out of hiding—news that a human wizard named Ilgreth had recovered the orb of gold dragonkind and had been using it to enslave dragons dwelling in and around the Five Kings Mountains. Infuriated and blinded with a need for vengeance, Mengkare foolishly challenged Ilgreth, hoping to defeat him, gain control of the orb of gold dragonkind, and keep it from human hands forever. But the orb of gold dragonkind warned Ilgreth of Mengkare’s approach. He confronted the gold dragon and, only a moment later, Mengkare became dominated by the orb of gold dragonkind for the second time in his life. Ilgreth retreated back to his hidden workshop deep within the volcano then known as Torag’s Crag and put Mengkare to work, but his plans to harness the dormant volcano’s energy collapsed when a group of powerful human heroes tracked him down and confronted him. The wizard threw his dominated dragons at the heroes, but a lucky greater dispel magic managed to counteract the dominate monster effect controlling several of the dragons, including Mengkare. The furious and shamed gold dragon seized his chance—and discovered in that moment a heretofore unknown fact of his ancestry: Mengkare was a direct descendant of the original gold dragon whose soul had been bound, eons before, into the orb of gold dragonkind. While Ilgreth had protected himself from fire, he had no defense against Mengkare’s weakness-inducing breath. Already feeble, the wizard was rendered unconscious by the blast, but this mattered little, for the breath also caught the orb of gold dragonkind in its wake. The result was instantaneous. The orb of gold dragonkind exploded, overloaded the runes Ilgreth had been carefully crafting, and set off a chain reaction: the volcano began to erupt! As devastation spread, Mengkare quickly swept up most of the shattered fragments of the destroyed orb of gold dragonkind and teleported away, back to his lair in Hermea.</rdfs:comment>
    </owl:NamedIndividual>
    


    <!-- https://raw.githubusercontent.com/AbsVahter/trpgontologies/main/pathfinder/2ed/pzo90145.rdf#Event_Dragon_Plague -->

    <owl:NamedIndividual rdf:about="https://raw.githubusercontent.com/AbsVahter/trpgontologies/main/pathfinder/2ed/pzo90145.rdf#Event_Dragon_Plague">
        <rdf:type rdf:resource="https://raw.githubusercontent.com/AbsVahter/trpgontologies/main/pathfinder/2ed/pzo90145.rdf#Event_History"/>
        <pzo9000-25e:event_with_subject rdf:resource="https://raw.githubusercontent.com/AbsVahter/trpgontologies/main/pathfinder/2ed/pzo90145.rdf#NPC_Mengkare"/>
        <pzo90145:event_date>{
1559: The dwarven city of Saggorak is founded.
2492: Orc invasion of Five Kings Mountains begins.
2507: Saggorak is blockaded by orcs.
2519: Saggorak falls after a 12-year siege.
3197: Khadon the Mighty leads effort to reclaim Five Kings Mountains from orcs.
3279: Khadon’s forces defeat the orcs at the Battle of Splitmist Pass. He then founds the empire of Tar Khadurrm.
3288: Khadon the Mighty walls off Saggorak after discovering the city to be infested with undead.
3469: Mengkare hatches in Taldor in the World’s Edge Mountains.
3660: Dragon Plague strikes Taldor.
3661: Mengkare and his parents are dominated by the orb of gold dragonkind and forced to blockade Maheto.
3667: Mengkare is banished to Axis and his parents are slain.
3672: Dragon Plague ends in Taldor.
}</pzo90145:event_date>
        <rdfs:comment>The gold dragon Mengkare hatched in 3469 ar in the eastern foothills of the World’s Edge Mountains. For the first 191 years of his life, Mengkare studied history, magic, and philosophy, tutored by his parents and, periodically, trusted scholars from across the world who were allowed to visit the lair. This idyllic life came to a devastating end in 3660, when a conspiracy of anarchists led by a cleric of Dahak used a powerful artifact called the orb of gold dragonkind to dominate metallic dragons throughout Taldor, driving them to commit devastating atrocities that threw the nation into chaos—this event came to be known as the Dragon Plague. Mengkare and his parents were among those dragons dominated by the conspirators. In time, Mengkare’s parents were killed by a group of dragonslayers, while Mengkare himself was banished to the Wastelands of Axis by the violet ray of a prismatic spray. Mengkare remained in exile on Axis for over a century, and it was during these years that his alignment shifted from lawful good to lawful neutral, and he first began to philosophize upon the nature of racial perfection.</rdfs:comment>
    </owl:NamedIndividual>
    


    <!-- https://raw.githubusercontent.com/AbsVahter/trpgontologies/main/pathfinder/2ed/pzo90145.rdf#Event_End_of_Age_of_Ashes_by_Ekujae_Elves -->

    <owl:NamedIndividual rdf:about="https://raw.githubusercontent.com/AbsVahter/trpgontologies/main/pathfinder/2ed/pzo90145.rdf#Event_End_of_Age_of_Ashes_by_Ekujae_Elves">
        <pzo9000-25e:event_from_motive rdf:resource="https://raw.githubusercontent.com/AbsVahter/trpgontologies/main/pathfinder/2ed/pzo90145.rdf#Motive_Stop_Age_of_Ashes"/>
        <pzo9000-25e:event_in_location rdf:resource="https://raw.githubusercontent.com/AbsVahter/trpgontologies/main/pathfinder/2ed/pzo90145.rdf#Location_Alseta~s_Ring"/>
        <pzo9000-25e:event_with_subject rdf:resource="https://raw.githubusercontent.com/AbsVahter/trpgontologies/main/pathfinder/2ed/pzo90145.rdf#Community_Ekujae_Elves"/>
        <pzo9000-25e:event_with_subject rdf:resource="https://raw.githubusercontent.com/AbsVahter/trpgontologies/main/pathfinder/2ed/pzo90145.rdf#NPC_Dahak"/>
        <pzo90145:event_to_event rdf:resource="https://raw.githubusercontent.com/AbsVahter/trpgontologies/main/pathfinder/2ed/pzo90145.rdf#Event_Dragon_Plague"/>
        <pzo90145:event_date>–5277</pzo90145:event_date>
        <rdfs:comment>Dahak is defeated by the Ekujae and banished, but a fragment of his power remains stuck in the “in between” of the elf gates. Backlash from his defeat spills into Alseta’s Ring and destroys the portal to Lotusgate.

Golarion was already horribly wounded, and Dahak could have eventually damaged it enough to finish the job that Earthfall started, were it not for the Ekujae elves, who had stayed behind hoping to ride out the disaster. With their partial knowledge of how the aiudara worked, these elves were able to enact a powerful ritual to defeat Dahak’s incarnation and stop the god’s devastating dragonstorms. In doing so, the elves were forced to sacrifice many of their own great heroes, a sacrifice that managed to turn Dahak’s power back in on himself, slaying the incarnation’s body and banishing its spiritual essence into the metaphysical space between portals in Alseta’s Ring. This trapped the incarnation beyond reality and without a body, but the magical backlash from the ritual blasted through the portals to destroy Lotusgate, the ring’s connection back to Kyonin. In so doing, this cut Alseta’s Ring off from the aiudara network entirely. By the time descendants of Kyonin’s elves returned to Golarion thousands of years later, Alseta’s Ring had been truly forgotten.</rdfs:comment>
    </owl:NamedIndividual>
    


    <!-- https://raw.githubusercontent.com/AbsVahter/trpgontologies/main/pathfinder/2ed/pzo90145.rdf#Event_First_Aiudara -->

    <owl:NamedIndividual rdf:about="https://raw.githubusercontent.com/AbsVahter/trpgontologies/main/pathfinder/2ed/pzo90145.rdf#Event_First_Aiudara">
        <rdf:type rdf:resource="https://raw.githubusercontent.com/AbsVahter/trpgontologies/main/pathfinder/2ed/pzo90145.rdf#Event_History"/>
        <pzo9000-25e:event_with_subject rdf:resource="https://raw.githubusercontent.com/AbsVahter/trpgontologies/main/pathfinder/2ed/pzo90145.rdf#NPC_Candlaron_the_Sculptor"/>
        <pzo90145:event_to_event rdf:resource="https://raw.githubusercontent.com/AbsVahter/trpgontologies/main/pathfinder/2ed/pzo90145.rdf#Event_Age_of_Ashes"/>
        <pzo90145:event_date>Age of Legends</pzo90145:event_date>
        <rdfs:comment>Elves arrive on Golarion. Candlaron creates the aiudara network, beginning with construction of the portals of Alseta’s Ring.

Well over 10,000 years ago, during the fabled Age of Legend, an elven hero named Candlaron the Sculptor created the very first elf gates, inspired by the gate between Golarion and Castrovel. These portals, which he called aiudara, allowed for instantaneous travel between distant locales. He linked one from the elven capital city of Iadara to a nexus of magical power many miles to the southwest, at the convergence of several thrumming magical ley lines under a remote forested hill. But he was frustrated in his attempts to form a proper hub—the portal magic of these first aiudara wouldn’t function if their destinations overlapped. As a compromise, Candlaron fashioned a circular chamber around the underground ley line nexus, then crafted five more aiudara to create a ring of portals. He named this chamber Alseta’s Ring, after the demigoddess of doorways and transitions, and similarly dedicated each of the six surrounding portals in the chamber to one of six elven divinities. Lotusgate linked back to Iadara and was dedicated to Alseta herself. Dreamgate, which linked to the western coast of Avistan, was dedicated to Desna. Duskgate, which linked to a site far to the south in Garund, was dedicated to Findeladlara, the elven goddess of architecture and art. Huntergate, which linked to the jungles of the Mwangi Expanse, was devoted to Ketephys, god of hunting and the moon. Jewelgate, which linked to a vast cavern below what would become known as the Five Kings Mountains, honored Yuelral, the elven goddess of crystals and magic. Finally, Vengegate, which linked to an island in the Steaming Sea that would one day be known as Hermea, was dedicated to Calistria.</rdfs:comment>
    </owl:NamedIndividual>
    


    <!-- https://raw.githubusercontent.com/AbsVahter/trpgontologies/main/pathfinder/2ed/pzo90145.rdf#Event_Foundation_of_Breachill -->

    <owl:NamedIndividual rdf:about="https://raw.githubusercontent.com/AbsVahter/trpgontologies/main/pathfinder/2ed/pzo90145.rdf#Event_Foundation_of_Breachill">
        <rdf:type rdf:resource="https://raw.githubusercontent.com/AbsVahter/trpgontologies/main/pathfinder/2ed/pzo90145.rdf#Event_History"/>
        <pzo9000-25e:event_in_location rdf:resource="https://raw.githubusercontent.com/AbsVahter/trpgontologies/main/pathfinder/2ed/pzo9000-25e.rdf#Settlement_Breachill"/>
        <pzo9000-25e:event_with_subject rdf:resource="https://raw.githubusercontent.com/AbsVahter/trpgontologies/main/pathfinder/2ed/pzo90145.rdf#NPC_Mengkare"/>
        <pzo90145:event_after_event rdf:resource="https://raw.githubusercontent.com/AbsVahter/trpgontologies/main/pathfinder/2ed/pzo90145.rdf#Event_Mengkare_Activated_Portal"/>
        <rdfs:comment>And so Mengkare hid the Vengegate key in his lair and dedicated himself to finding a solution to this new problem. For 2 centuries the dragon pondered, spending much of that time researching in the Perfect City on Axis. Eventually he discovered a potential solution, then spent nearly another century searching his soul and agonizing over the ramifications of what he’d learned—a potential way to not only defeat Dahak’s incarnation but also to strike a significant, perhaps even mortal, blow to the dragon god of destruction, but only at the expense of an entire civilization.
Mengkare’s discovery was of the Anima Invocation, the same ritual the Ekujae elves used so long ago to end the previous Age of Ashes and imprison Dahak’s avatar. Mengkare studied the ritual and focused on methods of expanding and improving its effects, eventually coming to the conclusion that if he could engineer a powerful enough sacrifice of a sufficient number of perfected souls, he could not only defeat the manifestation of Dahak but cause significant and lasting damage to the dragon god himself! Using the same logical arguments he’d used to retroactively justify the devastating volcanic eruption he’d triggered years before, he was able to come to terms with the most distasteful part of his plan—the sacrifice itself. If sacrificing a few thousand souls could save hundreds of thousands or more, would it not be a greater evil to do nothing and potentially consign future nations to oblivion?
Mengkare returned to Golarion in 4512 and spent the next several years finalizing his plan. Then, in 4519, he traveled to the region surrounding Alseta’s Ring, disguised as a human wizard named Lamond Breachton, and scoured Isger for people who epitomized the perfection he sought. The dragon’s initial plan was to tell these recruits the goal of his plan and use saving the world as motivation, theorizing that a like-minded group of good-hearted people would see the wisdom of his goals, but he quickly found that humans were resistant to building a society whose goal was self-sacrifice. When he realized his initial plan to create a utopia was a failure, the dragon used powerful magic to erase all traces of his attempt. He wiped the subjects’ memories, leaving them with only the barest training they’d need to survive in the remote wilderness. He extended this mind-wiping magic to cut off the citizens of the town from their loved ones, seeking to ensure his first failure would remain forgotten. He then spent a year helping the townsfolk get re-established, playing the role of a “kindly wizard who’d discovered the amnesiac citizens of a remote town and sought to save them.” In so doing, Mengkare yet again stanched his own guilt by telling himself he was acting for the greater good of humanity.
Mengkare spared no expense in this pursuit, spending a significant amount of gold from his hoard to ensure the town would thrive, helping the citizens create a supportive infrastructure before he abandoned them to their fates. The townspeople never heard from him again, but they never forgot—they named their home after him, and Breachill exists to this day, an unsuspecting remnant of Mengkare’s doomed first attempt to create a utopia.</rdfs:comment>
    </owl:NamedIndividual>
    


    <!-- https://raw.githubusercontent.com/AbsVahter/trpgontologies/main/pathfinder/2ed/pzo90145.rdf#Event_Mengkare_Activated_Portal -->

    <owl:NamedIndividual rdf:about="https://raw.githubusercontent.com/AbsVahter/trpgontologies/main/pathfinder/2ed/pzo90145.rdf#Event_Mengkare_Activated_Portal">
        <rdf:type rdf:resource="https://raw.githubusercontent.com/AbsVahter/trpgontologies/main/pathfinder/2ed/pzo90145.rdf#Event_History"/>
        <pzo9000-25e:event_in_location rdf:resource="https://raw.githubusercontent.com/AbsVahter/trpgontologies/main/pathfinder/2ed/pzo90145.rdf#Location_Alseta~s_Ring"/>
        <pzo9000-25e:event_with_subject rdf:resource="https://raw.githubusercontent.com/AbsVahter/trpgontologies/main/pathfinder/2ed/pzo90145.rdf#NPC_Mengkare"/>
        <pzo90145:event_after_event rdf:resource="https://raw.githubusercontent.com/AbsVahter/trpgontologies/main/pathfinder/2ed/pzo90145.rdf#Event_Destruction_of_Orb_of_Gold_Dragonkind"/>
        <rdfs:comment>Victory over the orb of gold dragonkind rang hollow, as Mengkare realized the volcanic eruption he had triggered had caused the loss of many lives, but he convinced himself that this was a necessary sacrifice. He devoted much of his time to studying the shards of the orb of gold dragonkind, and eventually decided that there was no way the destroyed artifact could ever be restored. Relieved that this thorn from his past had been truly vanquished, he placed the shards in his vault and spent the following years periodically traveling back to the perfect city of Axis to further research the nature of racial and spiritual perfection. In 4212, Mengkare found something amazing in a cavern deep under Hermea—an ancient and inoperable aiudara called Vengegate. Although he was initially unable to reactivate the portal, Mengkare’s considerable intellect and magical skill allowed him to determine where the portal led—a remote location on the border of Isger and Druma. Mengkare flew to the site, explored further, and discovered Alseta’s Ring. There, he also discovered the magical key needed to activate Vengegate. But when Mengkare activated the portal, he made a disturbing discovery: the incarnation of Dahak that haunted the Ring. Mengkare’s wonder at discovering the portal network and desire to reactivate the other portals in Alseta’s Ring was replaced by fear of what would occur should the incarnation of Dahak escape from its imprisonment—a resurgence of dragonstorms and the release of a cruel god’s avatar.</rdfs:comment>
    </owl:NamedIndividual>
    


    <!-- https://raw.githubusercontent.com/AbsVahter/trpgontologies/main/pathfinder/2ed/pzo90145.rdf#Event_Scarlet_Triad_as_Slave_Trader -->

    <owl:NamedIndividual rdf:about="https://raw.githubusercontent.com/AbsVahter/trpgontologies/main/pathfinder/2ed/pzo90145.rdf#Event_Scarlet_Triad_as_Slave_Trader">
        <rdf:type rdf:resource="https://raw.githubusercontent.com/AbsVahter/trpgontologies/main/pathfinder/2ed/pzo90145.rdf#Event_History"/>
        <pzo9000-25e:event_with_subject rdf:resource="https://raw.githubusercontent.com/AbsVahter/trpgontologies/main/pathfinder/2ed/pzo90145.rdf#Community_Scarlet_Triad"/>
        <pzo90145:event_after_event rdf:resource="https://raw.githubusercontent.com/AbsVahter/trpgontologies/main/pathfinder/2ed/pzo90145.rdf#Event_Second_Glorious_Endeavor"/>
        <rdfs:comment>For decades, the Scarlet Triad served as “talent scouts” for Promise, but as the Glorious Endeavor continued to gain momentum and population, the need for new blood grew less and less. By 4690, Mengkare reduced funding and support to the Scarlet Triad, reasoning that their services were increasingly unnecessary. The Triad then decided to secretly branch out into the slave trade to augment their dwindling coffers, figuring that their agents were already seeking out talented and gifted people and that even those who didn’t meet the strict requirements for inclusion into the Glorious Endeavour could still fetch a high price as slaves.
The Scarlet Triad kept this venture quiet from Mengkare with the aid of their current leader, Uri Zandivar, whose elder sister Emaliza had the dragon’s ear and a vaunted position as one of Mengkare’s 13 elected advisors—the Council of Enlightenment. With his sister’s aid, Uri prevented Mengkare from learning the truth about the Triad’s descent into the slave trade—as long as the organization continued to provide the good human stock the dragon sought and did so at reduced overhead, things ran smoothly. When Absalom outlawed slavery in 4717, the Scarlet Triad saw a significant portion of its business crash and burn, and over the past few years it has been working to branch out—most significantly into Old Cheliax’s slave trade, into the Darklands below the Five Kings Mountains (hoping to set up a new slave trade with the duergar there), and with a cult of Dahak worshippers in the Mwangi Expanse—a cult whose invasion of Breachill sets into motion the events of this Adventure Path.</rdfs:comment>
    </owl:NamedIndividual>
    


    <!-- https://raw.githubusercontent.com/AbsVahter/trpgontologies/main/pathfinder/2ed/pzo90145.rdf#Event_Second_Glorious_Endeavor -->

    <owl:NamedIndividual rdf:about="https://raw.githubusercontent.com/AbsVahter/trpgontologies/main/pathfinder/2ed/pzo90145.rdf#Event_Second_Glorious_Endeavor">
        <rdf:type rdf:resource="https://raw.githubusercontent.com/AbsVahter/trpgontologies/main/pathfinder/2ed/pzo90145.rdf#Event_History"/>
        <pzo9000-25e:event_from_motive rdf:resource="https://raw.githubusercontent.com/AbsVahter/trpgontologies/main/pathfinder/2ed/pzo90145.rdf#Motive_Defeat_Incarnation_of_Dahak"/>
        <pzo9000-25e:event_with_subject rdf:resource="https://raw.githubusercontent.com/AbsVahter/trpgontologies/main/pathfinder/2ed/pzo90145.rdf#NPC_Mengkare"/>
        <pzo90145:event_after_event rdf:resource="https://raw.githubusercontent.com/AbsVahter/trpgontologies/main/pathfinder/2ed/pzo90145.rdf#Event_Foundation_of_Breachill"/>
        <rdfs:comment>It would be decades before Mengkare began his second attempt at creating a utopia. With this second Glorious Endeavor and the founding of the utopian city of Promise, he embraced secrecy and sought to not only recruit souls but also to hand-craft them himself via selective breeding and rigorous training. But what Mengkare didn’t anticipate was that his creation of a new organization—the Scarlet Triad—would eventually set into motion a series of events that could well bring the Glorious Endeavor to its knees.</rdfs:comment>
    </owl:NamedIndividual>
    


    <!-- https://raw.githubusercontent.com/AbsVahter/trpgontologies/main/pathfinder/2ed/pzo90145.rdf#Motive_Defeat_Incarnation_of_Dahak -->

    <owl:NamedIndividual rdf:about="https://raw.githubusercontent.com/AbsVahter/trpgontologies/main/pathfinder/2ed/pzo90145.rdf#Motive_Defeat_Incarnation_of_Dahak">
        <pzo9000-25e:motive_from_event rdf:resource="https://raw.githubusercontent.com/AbsVahter/trpgontologies/main/pathfinder/2ed/pzo90145.rdf#Event_Mengkare_Activated_Portal"/>
        <pzo9000-25e:motive_has_target_subject rdf:resource="https://raw.githubusercontent.com/AbsVahter/trpgontologies/main/pathfinder/2ed/pzo90145.rdf#NPC_Dahak"/>
        <pzo9000-25e:motive_leads_to_event rdf:resource="https://raw.githubusercontent.com/AbsVahter/trpgontologies/main/pathfinder/2ed/pzo90145.rdf#Event_Foundation_of_Breachill"/>
        <pzo9000-25e:motive_of_subject rdf:resource="https://raw.githubusercontent.com/AbsVahter/trpgontologies/main/pathfinder/2ed/pzo90145.rdf#NPC_Mengkare"/>
        <rdfs:comment>The phrase “Tomorrow Must Burn” is one Mengkare often uses to justify his actions. It refers to the end goal of the Glorious Endeavor, and to Mengkare’s conviction that in order to save the future from Dahak, a short-term and hopefully controlled apocalypse in the form of sacrificing the populace of Promise will secure survival for the rest of the world. “Tomorrow must burn...” Mengkare tells himself, “...so the days thereafter can prosper.”</rdfs:comment>
    </owl:NamedIndividual>
    


    <!-- https://raw.githubusercontent.com/AbsVahter/trpgontologies/main/pathfinder/2ed/pzo90145.rdf#Motive_Dominate_Metallic_Dragon -->

    <owl:NamedIndividual rdf:about="https://raw.githubusercontent.com/AbsVahter/trpgontologies/main/pathfinder/2ed/pzo90145.rdf#Motive_Dominate_Metallic_Dragon">
        <rdf:type rdf:resource="https://raw.githubusercontent.com/AbsVahter/trpgontologies/main/pathfinder/2ed/pzo9000-25e.rdf#Motive"/>
        <pzo9000-25e:motive_leads_to_event rdf:resource="https://raw.githubusercontent.com/AbsVahter/trpgontologies/main/pathfinder/2ed/pzo90145.rdf#Event_Dragon_Plague"/>
    </owl:NamedIndividual>
    


    <!-- https://raw.githubusercontent.com/AbsVahter/trpgontologies/main/pathfinder/2ed/pzo90145.rdf#Motive_Gain_Mengkare_as_Slave -->

    <owl:NamedIndividual rdf:about="https://raw.githubusercontent.com/AbsVahter/trpgontologies/main/pathfinder/2ed/pzo90145.rdf#Motive_Gain_Mengkare_as_Slave">
        <rdf:type rdf:resource="https://raw.githubusercontent.com/AbsVahter/trpgontologies/main/pathfinder/2ed/pzo9000-25e.rdf#Motive"/>
        <pzo9000-25e:motive_from_event rdf:resource="https://raw.githubusercontent.com/AbsVahter/trpgontologies/main/pathfinder/2ed/pzo90145.rdf#Event_Scarlet_Triad_as_Slave_Trader"/>
        <pzo9000-25e:motive_has_target_subject rdf:resource="https://raw.githubusercontent.com/AbsVahter/trpgontologies/main/pathfinder/2ed/pzo90145.rdf#NPC_Mengkare"/>
        <pzo9000-25e:motive_of_subject rdf:resource="https://raw.githubusercontent.com/AbsVahter/trpgontologies/main/pathfinder/2ed/pzo90145.rdf#Community_Scarlet_Triad"/>
        <pzo90145:motive_has_target_resource rdf:resource="https://raw.githubusercontent.com/AbsVahter/trpgontologies/main/pathfinder/2ed/pzo90145.rdf#Artifact_Orb_of_Gold_Dragonkind"/>
        <rdfs:comment>In the meantime, the Scarlet Triad has become focused on a significant project—gathering up as many shards of the destroyed orb of gold dragonkind as it can, so that it can rebuild a lesser version of the orb. With the aid of strange rituals, powerful allies, and essences of Dahak himself stripped from tainted gold mined from the Mwangi Expanse where the deity’s manifestation once walked the world, the Scarlet Triad grows ever closer to something Mengkare assumed was impossible—rebuilding, at least in part, an artifact that will grant the Scarlet Triad the power to gain its most powerful slave yet: Mengkare himself.</rdfs:comment>
        <pf2_general:for_future_correction>These slavers have wholeheartedly embraced the idea of weaponizing Alseta’s Ring—eventually using it both as a method for swift travel throughout the region and as a destructive agent against the sites the ring connects to, focusing Dahak’s wrath upon those who would oppose them. Uri Zandivar believes that once they can control Mengkare via a partially reconstructed orb of gold dragonkind, the dragon will reveal the secrets of the ancient portal network and allow them to relocate their base of operations to Promise. 
For the moment, though, the Scarlet Triad must act cautiously. After all, the group is still under Mengkare’s (distracted) watch, and Uri realizes that any attempt to directly control or activate the portals of Alseta’s Ring before they’ve managed to complete repairs to the orb of gold dragonkind runs an increased risk of attracting the dragon’s attention. So instead, Uri has taken steps to ensure a Scarlet Triad presence near all five portal sites, with cover stories to justify their presence, should Mengkare grow curious. Keeping an eye on Vengegate (in Promise) and Duskgate (in southern Katapesh) is simple enough, since the Scarlet Triad already has legitimate reasons to be active in Hermea and Katapesh. By having agents established in Ravounel and Saggorak under the pretense of securing additional mercantile interests, the Scarlet Triad can watch over Dreamgate and Jewelgate (that these interests primarily involve the slave trade remains yet another secret the Triad is keeping from Mengkare). And in the Mwangi Expanse, the Triad has secured an alliance with the Cinderclaws to gain shipments of gold tainted with Dahak’s poisonous legacy. Agents have also been keeping an eye on Breachill from afar through contacts with local bookseller Voz Lirayne.
As the events of the first two adventures in Age of Ashes unfold, the PCs’ actions largely go unnoticed by the Scarlet Triad—Breachill has a long tradition of “spawning adventurers,” after all, but to date, none of them have made memorable names for themselves. Their defeat of Voz isn’t immediately noticed either, for the Triad agents have more significant tasks distracting them. However, by the time the PCs disrupt the Cinderclaws in the second adventure, Cult of Cinders, certain agents among the Scarlet Triad begin finally to take note. It falls to the gnoll Laslunn, third in command of the Scarlet Triad, to investigate what happened to Voz, and as the third adventure begins, she rightfully suspects that the PCs may be growing into a significant problem. Fortunately for the PCs, Laslunn has her own plots and keeps her knowledge about the PCs to herself, hoping that the PCs might become tools she can use to gain more power within the Triad.
When the PCs begin Age of Ashes, two of the portal keys await discovery. Scarlet Triad agents control three of the portal keys needed to use the aiudara of Alseta’s Ring. Laslunn keeps the key to Jewelgate safe, while her direct superior Ilssrah Embermead guards the key to Duskgate as she works to undermine the dwarven city of Kolvar near the ruins of Saggorak. Uri himself has secretly absconded with Vengegate’s key from Mengkare’s treasury. In keeping with the plan to maintain low profiles and mask their actual interest in Alseta’s Ring, none of these three keys have been used to infiltrate Breachill. Indeed, as Uri suspects, the way stations within all but Vengegate are likely to contain dangerous traps and hazards—for now, these factors keep Alseta’s Ring safe from infiltration via the Scarlet Triad.</pf2_general:for_future_correction>
    </owl:NamedIndividual>
    


    <!-- https://raw.githubusercontent.com/AbsVahter/trpgontologies/main/pathfinder/2ed/pzo90145.rdf#Motive_Ilgreth -->

    <owl:NamedIndividual rdf:about="https://raw.githubusercontent.com/AbsVahter/trpgontologies/main/pathfinder/2ed/pzo90145.rdf#Motive_Ilgreth">
        <rdf:type rdf:resource="https://raw.githubusercontent.com/AbsVahter/trpgontologies/main/pathfinder/2ed/pzo9000-25e.rdf#Motive"/>
        <pzo9000-25e:motive_leads_to_event rdf:resource="https://raw.githubusercontent.com/AbsVahter/trpgontologies/main/pathfinder/2ed/pzo90145.rdf#Event_Destruction_of_Orb_of_Gold_Dragonkind"/>
        <pzo9000-25e:motive_of_subject rdf:resource="https://raw.githubusercontent.com/AbsVahter/trpgontologies/main/pathfinder/2ed/pzo90145.rdf#NPC_Ilgreth"/>
        <rdfs:comment>enslave dragons</rdfs:comment>
    </owl:NamedIndividual>
    


    <!-- https://raw.githubusercontent.com/AbsVahter/trpgontologies/main/pathfinder/2ed/pzo90145.rdf#Motive_Mengkare_Pfilosophical_Quest -->

    <owl:NamedIndividual rdf:about="https://raw.githubusercontent.com/AbsVahter/trpgontologies/main/pathfinder/2ed/pzo90145.rdf#Motive_Mengkare_Pfilosophical_Quest">
        <rdf:type rdf:resource="https://raw.githubusercontent.com/AbsVahter/trpgontologies/main/pathfinder/2ed/pzo9000-25e.rdf#Motive"/>
        <pzo9000-25e:motive_from_event rdf:resource="https://raw.githubusercontent.com/AbsVahter/trpgontologies/main/pathfinder/2ed/pzo90145.rdf#Event_Dragon_Plague"/>
        <pzo9000-25e:motive_leads_to_event rdf:resource="https://raw.githubusercontent.com/AbsVahter/trpgontologies/main/pathfinder/2ed/pzo90145.rdf#Event_Mengkare~s_Path"/>
        <pzo9000-25e:motive_of_subject rdf:resource="https://raw.githubusercontent.com/AbsVahter/trpgontologies/main/pathfinder/2ed/pzo90145.rdf#NPC_Mengkare"/>
        <rdfs:comment>intrigued by humanity’s paradoxical capacity for great good and great evil</rdfs:comment>
    </owl:NamedIndividual>
    


    <!-- https://raw.githubusercontent.com/AbsVahter/trpgontologies/main/pathfinder/2ed/pzo90145.rdf#Motive_Portal_Links_across_all_Golarion -->

    <owl:NamedIndividual rdf:about="https://raw.githubusercontent.com/AbsVahter/trpgontologies/main/pathfinder/2ed/pzo90145.rdf#Motive_Portal_Links_across_all_Golarion">
        <rdf:type rdf:resource="https://raw.githubusercontent.com/AbsVahter/trpgontologies/main/pathfinder/2ed/pzo9000-25e.rdf#Motive"/>
        <pzo9000-25e:motive_leads_to_event rdf:resource="https://raw.githubusercontent.com/AbsVahter/trpgontologies/main/pathfinder/2ed/pzo90145.rdf#Event_First_Aiudara"/>
        <pzo9000-25e:motive_of_subject rdf:resource="https://raw.githubusercontent.com/AbsVahter/trpgontologies/main/pathfinder/2ed/pzo90145.rdf#NPC_Candlaron_the_Sculptor"/>
        <rdfs:comment>Well over 10,000 years ago, during the fabled Age of Legend, an elven hero named Candlaron the Sculptor created the very first elf gates, inspired by the gate between Golarion and Castrovel.</rdfs:comment>
    </owl:NamedIndividual>
    


    <!-- https://raw.githubusercontent.com/AbsVahter/trpgontologies/main/pathfinder/2ed/pzo90145.rdf#Motive_Stop_Age_of_Ashes -->

    <owl:NamedIndividual rdf:about="https://raw.githubusercontent.com/AbsVahter/trpgontologies/main/pathfinder/2ed/pzo90145.rdf#Motive_Stop_Age_of_Ashes">
        <pzo9000-25e:motive_from_event rdf:resource="https://raw.githubusercontent.com/AbsVahter/trpgontologies/main/pathfinder/2ed/pzo90145.rdf#Event_Age_of_Ashes"/>
        <pzo9000-25e:motive_has_target_subject rdf:resource="https://raw.githubusercontent.com/AbsVahter/trpgontologies/main/pathfinder/2ed/pzo90145.rdf#NPC_Dahak"/>
    </owl:NamedIndividual>
    


    <!-- https://raw.githubusercontent.com/AbsVahter/trpgontologies/main/pathfinder/2ed/pzo90145.rdf#NPC_Candlaron_the_Sculptor -->

    <owl:NamedIndividual rdf:about="https://raw.githubusercontent.com/AbsVahter/trpgontologies/main/pathfinder/2ed/pzo90145.rdf#NPC_Candlaron_the_Sculptor">
        <rdf:type rdf:resource="https://raw.githubusercontent.com/AbsVahter/trpgontologies/main/pathfinder/2ed/pzo9000-25e.rdf#NPC"/>
        <rdfs:comment>elven hero of Age of Legend</rdfs:comment>
    </owl:NamedIndividual>
    


    <!-- https://raw.githubusercontent.com/AbsVahter/trpgontologies/main/pathfinder/2ed/pzo90145.rdf#NPC_Cleric_of_Dahak -->

    <owl:NamedIndividual rdf:about="https://raw.githubusercontent.com/AbsVahter/trpgontologies/main/pathfinder/2ed/pzo90145.rdf#NPC_Cleric_of_Dahak">
        <rdf:type rdf:resource="https://raw.githubusercontent.com/AbsVahter/trpgontologies/main/pathfinder/2ed/pzo9000-25e.rdf#NPC"/>
        <pzo9000-25e:subject_has_motive rdf:resource="https://raw.githubusercontent.com/AbsVahter/trpgontologies/main/pathfinder/2ed/pzo90145.rdf#Motive_Dominate_Metallic_Dragon"/>
        <pzo9000-25e:subject_of_event rdf:resource="https://raw.githubusercontent.com/AbsVahter/trpgontologies/main/pathfinder/2ed/pzo90145.rdf#Event_Dragon_Plague"/>
    </owl:NamedIndividual>
    


    <!-- https://raw.githubusercontent.com/AbsVahter/trpgontologies/main/pathfinder/2ed/pzo90145.rdf#NPC_Dahak -->

    <owl:NamedIndividual rdf:about="https://raw.githubusercontent.com/AbsVahter/trpgontologies/main/pathfinder/2ed/pzo90145.rdf#NPC_Dahak">
        <rdf:type rdf:resource="https://raw.githubusercontent.com/AbsVahter/trpgontologies/main/pathfinder/2ed/pzo9000-25e.rdf#NPC"/>
        <pzo9000-25e:subject_of_event rdf:resource="https://raw.githubusercontent.com/AbsVahter/trpgontologies/main/pathfinder/2ed/pzo90145.rdf#Event_Age_of_Ashes"/>
        <rdfs:comment>destructive god of evil dragons</rdfs:comment>
    </owl:NamedIndividual>
    


    <!-- https://raw.githubusercontent.com/AbsVahter/trpgontologies/main/pathfinder/2ed/pzo90145.rdf#NPC_Ilgreth -->

    <owl:NamedIndividual rdf:about="https://raw.githubusercontent.com/AbsVahter/trpgontologies/main/pathfinder/2ed/pzo90145.rdf#NPC_Ilgreth">
        <rdf:type rdf:resource="https://raw.githubusercontent.com/AbsVahter/trpgontologies/main/pathfinder/2ed/pzo9000-25e.rdf#NPC"/>
        <pzo9000-25e:subject_of_event rdf:resource="https://raw.githubusercontent.com/AbsVahter/trpgontologies/main/pathfinder/2ed/pzo90145.rdf#Event_Destruction_of_Orb_of_Gold_Dragonkind"/>
        <rdfs:comment>human wizard named Ilgreth had recovered the orb of gold dragonkind and had been using it to enslave dragons</rdfs:comment>
    </owl:NamedIndividual>
    


    <!-- https://raw.githubusercontent.com/AbsVahter/trpgontologies/main/pathfinder/2ed/pzo90145.rdf#NPC_Mengkare -->

    <owl:NamedIndividual rdf:about="https://raw.githubusercontent.com/AbsVahter/trpgontologies/main/pathfinder/2ed/pzo90145.rdf#NPC_Mengkare">
        <rdf:type rdf:resource="https://raw.githubusercontent.com/AbsVahter/trpgontologies/main/pathfinder/2ed/pzo9000-25e.rdf#NPC"/>
        <rdfs:comment>gold dragon</rdfs:comment>
    </owl:NamedIndividual>
    


    <!-- https://raw.githubusercontent.com/AbsVahter/trpgontologies/main/pathfinder/2ed/pzo90145.rdf#NPC_Uri_Zandivar -->

    <owl:NamedIndividual rdf:about="https://raw.githubusercontent.com/AbsVahter/trpgontologies/main/pathfinder/2ed/pzo90145.rdf#NPC_Uri_Zandivar">
        <rdf:type rdf:resource="https://raw.githubusercontent.com/AbsVahter/trpgontologies/main/pathfinder/2ed/pzo9000-25e.rdf#NPC"/>
        <pzo9000-25e:npc_from_community rdf:resource="https://raw.githubusercontent.com/AbsVahter/trpgontologies/main/pathfinder/2ed/pzo90145.rdf#Community_Scarlet_Triad"/>
        <pzo9000-25e:subject_of_event rdf:resource="https://raw.githubusercontent.com/AbsVahter/trpgontologies/main/pathfinder/2ed/pzo90145.rdf#Event_Scarlet_Triad_as_Slave_Trader"/>
        <rdfs:comment>leader of Scarlet Triad</rdfs:comment>
    </owl:NamedIndividual>
    


    <!-- https://raw.githubusercontent.com/AbsVahter/trpgontologies/main/pathfinder/2ed/pzo90145.rdf#Settlement_Promise -->

    <owl:NamedIndividual rdf:about="https://raw.githubusercontent.com/AbsVahter/trpgontologies/main/pathfinder/2ed/pzo90145.rdf#Settlement_Promise">
        <rdf:type rdf:resource="https://raw.githubusercontent.com/AbsVahter/trpgontologies/main/pathfinder/2ed/pzo9000-25e.rdf#Settlement"/>
        <pzo9000-25e:location_for_event rdf:resource="https://raw.githubusercontent.com/AbsVahter/trpgontologies/main/pathfinder/2ed/pzo90145.rdf#Event_Second_Glorious_Endeavor"/>
        <rdfs:comment>utopian city of Promise</rdfs:comment>
    </owl:NamedIndividual>
    


    <!-- https://raw.githubusercontent.com/AbsVahter/trpgontologies/main/pathfinder/2ed/pzo90145.rdf#Art_Dahak~s_Wrath -->

    <owl:NamedIndividual rdf:about="https://raw.githubusercontent.com/AbsVahter/trpgontologies/main/pathfinder/2ed/pzo90145.rdf#Art_Dahak~s_Wrath">
        <rdf:type rdf:resource="https://raw.githubusercontent.com/AbsVahter/trpgontologies/main/pathfinder/2ed/pf2_general.rdf#Art"/>
        <schema:image rdf:resource="https://www.worldanvil.com/uploads/images/06dc5553f241bd2bb99a62a1489d5a28.jpg"/>
    </owl:NamedIndividual>
    


    <!-- https://raw.githubusercontent.com/AbsVahter/trpgontologies/main/pathfinder/2ed/pzo90145.rdf#Art_Torag~s_Crag -->

    <owl:NamedIndividual rdf:about="https://raw.githubusercontent.com/AbsVahter/trpgontologies/main/pathfinder/2ed/pzo90145.rdf#Art_Torag~s_Crag">
        <rdf:type rdf:resource="https://raw.githubusercontent.com/AbsVahter/trpgontologies/main/pathfinder/2ed/pf2_general.rdf#Art"/>
        <schema:image rdf:resource="https://ibb.co/XxsrnKN"/>
        <pf2_general:art_depicts rdf:resource="https://raw.githubusercontent.com/AbsVahter/trpgontologies/main/pathfinder/2ed/pzo90145.rdf#Location_Torag~s_Crag"/>
    </owl:NamedIndividual>
    


    <!-- https://raw.githubusercontent.com/AbsVahter/trpgontologies/main/pathfinder/2ed/pzo90145.rdf#Event_Mengkare~s_Path -->

    <owl:NamedIndividual rdf:about="https://raw.githubusercontent.com/AbsVahter/trpgontologies/main/pathfinder/2ed/pzo90145.rdf#Event_Mengkare~s_Path">
        <rdf:type rdf:resource="https://raw.githubusercontent.com/AbsVahter/trpgontologies/main/pathfinder/2ed/pzo90145.rdf#Event_History"/>
        <pzo9000-25e:event_with_subject rdf:resource="https://raw.githubusercontent.com/AbsVahter/trpgontologies/main/pathfinder/2ed/pzo90145.rdf#NPC_Mengkare"/>
        <pzo90145:event_after_event rdf:resource="https://raw.githubusercontent.com/AbsVahter/trpgontologies/main/pathfinder/2ed/pzo90145.rdf#Event_Dragon_Plague"/>
        <rdfs:comment>Mengkare returned to Golarion in 3773 and spent many years traveling the land in the guise of a human philosopher, intrigued by humanity’s paradoxical capacity for great good and great evil. Everywhere he traveled, he studied and observed. In 3819, as he wandered along the front of the Shining Crusade in Lastwall, he was approached by a fascinating woman who seemed to realize he was something more than a mere wandering philosopher. This woman was none other than Iomedae (before she ascended to divinity), a passionate and powerful crusader, and she convinced Mengkare to aid humanity in opposing the Whispering Tyrant and joining the crusade. Mengkare’s time as a crusader was short, for only 4 years later, he once again experienced humanity’s capacity for great evil when he witnessed Tar-Baphon’s defeat of Arazni. Demoralized further by what he took to be a lost cause, Mengkare quit the field of battle and left the mainland of Avistan, settling in for a hermit’s life on a remote and wilderness island in the Steaming Sea: Hermea.</rdfs:comment>
    </owl:NamedIndividual>
    


    <!-- https://raw.githubusercontent.com/AbsVahter/trpgontologies/main/pathfinder/2ed/pzo90145.rdf#Location_Alseta~s_Ring -->

    <owl:NamedIndividual rdf:about="https://raw.githubusercontent.com/AbsVahter/trpgontologies/main/pathfinder/2ed/pzo90145.rdf#Location_Alseta~s_Ring">
        <rdf:type rdf:resource="https://raw.githubusercontent.com/AbsVahter/trpgontologies/main/pathfinder/2ed/pzo9000-25e.rdf#Location"/>
        <pzo9000-25e:location_for_event rdf:resource="https://raw.githubusercontent.com/AbsVahter/trpgontologies/main/pathfinder/2ed/pzo90145.rdf#Event_First_Aiudara"/>
        <pzo9000-25e:location_inside_location rdf:resource="https://raw.githubusercontent.com/AbsVahter/trpgontologies/main/pathfinder/2ed/pzo9000-25e.rdf#Location_Isger"/>
        <pzo9000-25e:location_next_to_location rdf:resource="https://raw.githubusercontent.com/AbsVahter/trpgontologies/main/pathfinder/2ed/pzo9000-25e.rdf#Location_Citadel_Altaerein"/>
        <rdfs:comment>The ring of six aiudara located below Citadel Altaerein in Isger are known as Alseta’s Ring, and they were among the first of these magical portals created on Golarion—fashioned long ago in the Age of Legends by the elven spellcaster and hero Candlaron. He arranged these portals in a ring, placing them as close together as was possible without their individual portal energies interfering with one another. His work on these closely placed portals would prove instrumental in a breakthrough that, in the years to follow, allowed him to create aiudara hubs capable of linking between more than two locations. While Alseta’s Ring would always retain a special nostalgic place in Candlaron’s heart, the more efficient hub mechanic ensured that travel through these first aiudara was less frequent. By the time the elves fled Golarion on the eve of Earthfall, the aiudara of Alseta’s Ring had become little more than underused curiosities.</rdfs:comment>
    </owl:NamedIndividual>
    


    <!-- https://raw.githubusercontent.com/AbsVahter/trpgontologies/main/pathfinder/2ed/pzo90145.rdf#Location_Torag~s_Crag -->

    <owl:NamedIndividual rdf:about="https://raw.githubusercontent.com/AbsVahter/trpgontologies/main/pathfinder/2ed/pzo90145.rdf#Location_Torag~s_Crag">
        <rdf:type rdf:resource="https://raw.githubusercontent.com/AbsVahter/trpgontologies/main/pathfinder/2ed/pzo9000-25e.rdf#Location"/>
        <pzo9000-25e:location_for_event rdf:resource="https://raw.githubusercontent.com/AbsVahter/trpgontologies/main/pathfinder/2ed/pzo90145.rdf#Event_Destruction_of_Orb_of_Gold_Dragonkind"/>
        <rdfs:comment>volcano</rdfs:comment>
    </owl:NamedIndividual>
    


    <!-- https://raw.githubusercontent.com/AbsVahter/trpgontologies/main/pathfinder/2ed/pzo90145.rdf#Motive_Dahak~s_Wrath -->

    <owl:NamedIndividual rdf:about="https://raw.githubusercontent.com/AbsVahter/trpgontologies/main/pathfinder/2ed/pzo90145.rdf#Motive_Dahak~s_Wrath">
        <rdf:type rdf:resource="https://raw.githubusercontent.com/AbsVahter/trpgontologies/main/pathfinder/2ed/pzo9000-25e.rdf#Motive"/>
        <pzo9000-25e:motive_leads_to_event rdf:resource="https://raw.githubusercontent.com/AbsVahter/trpgontologies/main/pathfinder/2ed/pzo90145.rdf#Event_Age_of_Ashes"/>
        <pzo9000-25e:motive_of_subject rdf:resource="https://raw.githubusercontent.com/AbsVahter/trpgontologies/main/pathfinder/2ed/pzo90145.rdf#NPC_Dahak"/>
        <rdfs:comment>Dahak is destructive god of evil dragons</rdfs:comment>
    </owl:NamedIndividual>
    


    <!-- 
    ///////////////////////////////////////////////////////////////////////////////////////
    //
    // Annotations
    //
    ///////////////////////////////////////////////////////////////////////////////////////
     -->

    <rdf:Description rdf:about="https://raw.githubusercontent.com/AbsVahter/trpgontologies/main/pathfinder/2ed/pzo9000-25e.rdf#Art_Cover">
        <rdfs:comment>Kyra and Merisiel face off against an undead Hellknight guardian</rdfs:comment>
    </rdf:Description>
</rdf:RDF>



<!-- Generated by the OWL API (version 4.5.25.2023-02-15T19:15:49Z) https://github.com/owlcs/owlapi -->

